veric/semax_prog.v
@@ -53,26 +53,59 @@ Definition entry_tempenv (te: temp_env) (f: function) (vl: list val) :=
                           ++ map (fun tv => (fst tv, Vundef)) f.(fn_temps)).
 
 Definition semax_body_params_ok f : bool :=
-   andb
-        (compute_list_norepet (map (@fst _ _) (fn_params f) ++ map (@fst _ _) (fn_temps f)))
-        (compute_list_norepet (map (@fst _ _) (fn_vars f))).
+andb
+    (compute_list_norepet (map (@fst _ _) (fn_params f) ++ map (@fst _ _) (fn_temps f)))
+    (compute_list_norepet (map (@fst _ _) (fn_vars f))).
 
 Definition semax_body
-       (V: varspecs) (G: funspecs) {C: compspecs} (f: function) (spec: ident * funspec): Prop :=
-  match spec with (_, mk_funspec _ cc A P Q _ _) =>
-    forall Espec ts x, 
-      semax Espec (func_tycontext f V G nil)
-          (fun rho => P ts x rho * stackframe_of f rho)
-           (Ssequence f.(fn_body) (Sreturn None))
-          (frame_ret_assert (function_body_ret_assert (fn_return f) (Q ts x)) (stackframe_of f))
- end.
+   (V: varspecs) (G: funspecs) {C: compspecs} (f: function) (spec: ident * funspec): Prop :=
+match spec with (_, mk_funspec _ cc A P Q _ _) =>
+forall Espec ts x, 
+  semax Espec (func_tycontext f V G nil)
+      (fun rho => P ts x rho * stackframe_of f rho)
+       (Ssequence f.(fn_body) (Sreturn None))
+      (frame_ret_assert (function_body_ret_assert (fn_return f) (Q ts x)) (stackframe_of f))
+end.
 
+Definition genv_contains (ge: Genv.t fundef type) (fdecs : list (ident * fundef)) : Prop :=
+ forall id f, In (id,f) fdecs ->
+              exists b, Genv.find_symbol ge id = Some b /\ Genv.find_funct_ptr ge b = Some f.
+
+Lemma genv_prog_contains (ge:genv) fdecs: prog_contains ge fdecs = genv_contains ge fdecs.
+Proof. reflexivity. Qed.
+(*
 Definition semax_func
-         (V: varspecs) (G: funspecs) {C: compspecs} (fdecs: list (ident * fundef)) (G1: funspecs) : Prop :=
-   match_fdecs fdecs G1 /\
-  forall ge, prog_contains ge fdecs ->
-          cenv_sub cenv_cs (genv_cenv ge) ->
-          forall n, believe Espec (nofunc_tycontext V G) ge (nofunc_tycontext V G1) n.
+     (V: varspecs) (G: funspecs) {C: compspecs} (fdecs: list (ident * fundef)) (G1: funspecs) : Prop :=
+match_fdecs fdecs G1 /\
+forall ge, prog_contains ge fdecs ->
+      cenv_sub cenv_cs (genv_cenv ge) ->
+      forall n, believe Espec (nofunc_tycontext V G) ge (nofunc_tycontext V G1) n.
+*)
+
+Definition semax_func (V: varspecs) (G: funspecs) {C: compspecs} (ge: Genv.t fundef type)
+       (fdecs: list (ident * fundef)) (G1: funspecs) : Prop :=
+match_fdecs fdecs G1 /\ genv_contains ge fdecs /\
+forall (ge': Genv.t fundef type) (Gfs: forall i,  sub_option (Genv.find_symbol ge i) (Genv.find_symbol ge' i))
+         (Gffp: forall b, sub_option (Genv.find_funct_ptr ge b) (Genv.find_funct_ptr ge' b)) 
+n, believe Espec (nofunc_tycontext V G) (Build_genv ge' (@cenv_cs C)) (nofunc_tycontext V G1) n.
+
+Lemma semax_func_mono CS CS' (CSUB: cspecs_sub CS CS') ge ge'
+  (Gfs: forall i,  sub_option (Genv.find_symbol ge i) (Genv.find_symbol ge' i))
+  (Gffp: forall b, sub_option (Genv.find_funct_ptr ge b) (Genv.find_funct_ptr ge' b))
+  V G fdecs G1 (H: @semax_func  V G CS ge fdecs G1): @semax_func  V G CS' ge' fdecs G1.
+Proof.
+destruct H as [MF [GC B]]; split; [trivial | split].
++ hnf; intros. destruct (GC _ _ H) as [b [Hb1 Hb2]]. exists b; split.
+specialize (Gfs id); rewrite Hb1 in Gfs; apply Gfs.
+specialize (Gffp b); rewrite Hb2 in Gffp; apply Gffp.
++ intros ge2; intros. 
+assert (Q1: forall i, sub_option (Genv.find_symbol ge i) (Genv.find_symbol ge2 i)).
+{ intros. eapply sub_option_trans. apply Gfs. apply Gfs0. }
+assert (Q2: forall b, sub_option (Genv.find_funct_ptr ge b) (Genv.find_funct_ptr ge2 b)).
+{ intros. eapply sub_option_trans. apply Gffp. apply Gffp0. }
+apply (@believe_monoL CS Espec CS' {| genv_genv := ge2; genv_cenv := cenv_cs |} (nofunc_tycontext V G) (nofunc_tycontext V G)).
+intros; apply tycontext_sub_refl. apply CSUB. apply (B _ Q1 Q2 n).
+Qed. 
 
 Definition main_pre (prog: program) : list Type -> (ident->val) -> assert :=
 (fun nil gv => globvars2pred gv (prog_vars prog)).
@@ -83,95 +116,96 @@ Definition main_pre_ext (prog: program) (ora: OK_ty) : list Type -> (ident->val)
 Definition Tint32s := Tint I32 Signed noattr.
 
 Definition main_post (prog: program) : list Type -> (ident->val) -> assert :=
-  (fun nil _ _ => TT).
+(fun nil _ _ => TT).
 
 Definition main_spec' (prog: program) 
-    (post: list Type -> (ident->val) -> environ ->pred rmap): funspec :=
-  mk_funspec (nil, tint) cc_default
-     (ConstType (ident->val)) (main_pre prog) post
-       (const_super_non_expansive _ _) (const_super_non_expansive _ _).
+(post: list Type -> (ident->val) -> environ ->pred rmap): funspec :=
+mk_funspec (nil, tint) cc_default
+ (ConstType (ident->val)) (main_pre prog) post
+   (const_super_non_expansive _ _) (const_super_non_expansive _ _).
 
 Definition main_spec (prog: program): funspec :=
-  mk_funspec (nil, tint) cc_default
-     (ConstType (ident->val)) (main_pre prog) (main_post prog)
-       (const_super_non_expansive _ _) (const_super_non_expansive _ _).
+mk_funspec (nil, tint) cc_default
+ (ConstType (ident->val)) (main_pre prog) (main_post prog)
+   (const_super_non_expansive _ _) (const_super_non_expansive _ _).
 
 Definition main_spec_ext' (prog: program) (ora: OK_ty)
-    (post: list Type -> (ident->val) -> environ ->pred rmap): funspec :=
-  mk_funspec (nil, tint) cc_default
-     (ConstType (ident->val)) (main_pre_ext prog ora) post
-       (const_super_non_expansive _ _) (const_super_non_expansive _ _).
+(post: list Type -> (ident->val) -> environ ->pred rmap): funspec :=
+mk_funspec (nil, tint) cc_default
+ (ConstType (ident->val)) (main_pre_ext prog ora) post
+   (const_super_non_expansive _ _) (const_super_non_expansive _ _).
 
 Definition main_spec_ext (prog: program) (ora: OK_ty): funspec :=
-  mk_funspec (nil, tint) cc_default
-     (ConstType (ident->val)) (main_pre_ext prog ora) (main_post prog)
-       (const_super_non_expansive _ _) (const_super_non_expansive _ _).
+mk_funspec (nil, tint) cc_default
+ (ConstType (ident->val)) (main_pre_ext prog ora) (main_post prog)
+   (const_super_non_expansive _ _) (const_super_non_expansive _ _).
 
 Definition is_Internal (prog : program) (f : ident) :=
-  match Genv.find_symbol (Genv.globalenv prog) f with
-    None => false
-  | Some b =>
-    match Genv.find_funct_ptr (Genv.globalenv prog) b with
-    | None => false
-    | Some f =>
-      match f with
-      | External _ _ _ _ => false
-      | Internal _ => true
-      end
-    end
-  end.
+match Genv.find_symbol (Genv.globalenv prog) f with
+None => false
+| Some b =>
+match Genv.find_funct_ptr (Genv.globalenv prog) b with
+| None => false
+| Some f =>
+  match f with
+  | External _ _ _ _ => false
+  | Internal _ => true
+  end
+end
+end.
 
 Definition semax_prog {C: compspecs}
-           (prog: program)  (V: varspecs) (G: funspecs) : Prop :=
-  compute_list_norepet (prog_defs_names prog) = true  /\
-  all_initializers_aligned prog /\
-  cenv_cs = prog_comp_env prog /\
-  @semax_func V G C (prog_funct prog) G /\
-  match_globvars (prog_vars prog) V = true /\
-  match find_id prog.(prog_main) G with
-  | Some s => exists post, s = main_spec' prog post
-  | None => False
-  end.
+       (prog: program)  (V: varspecs) (G: funspecs) : Prop :=
+compute_list_norepet (prog_defs_names prog) = true  /\
+all_initializers_aligned prog /\
+cenv_cs = prog_comp_env prog /\
+(*  @semax_func V G C (prog_funct prog) G /\*)
+@semax_func V G C (Genv.globalenv prog) (prog_funct prog) G /\
+match_globvars (prog_vars prog) V = true /\
+match find_id prog.(prog_main) G with
+| Some s => exists post, s = main_spec' prog post
+| None => False
+end.
 
 Definition semax_prog_ext {C: compspecs}
-           (prog: program) (ora: OK_ty) (V: varspecs) (G: funspecs) : Prop :=
-  compute_list_norepet (prog_defs_names prog) = true  /\
-  all_initializers_aligned prog /\
-  cenv_cs = prog_comp_env prog /\
-  @semax_func V G C (prog_funct prog) G /\
-  match_globvars (prog_vars prog) V = true /\
-  match find_id prog.(prog_main) G with
-  | Some s => exists post, s = main_spec_ext' prog ora post
-  | None => False
-  end.
+       (prog: program) (ora: OK_ty) (V: varspecs) (G: funspecs) : Prop :=
+compute_list_norepet (prog_defs_names prog) = true  /\
+all_initializers_aligned prog /\
+cenv_cs = prog_comp_env prog /\
+(*  @semax_func V G C (prog_funct prog) G /\*)
+@semax_func V G C (Genv.globalenv prog) (prog_funct prog) G /\
+match_globvars (prog_vars prog) V = true /\
+match find_id prog.(prog_main) G with
+| Some s => exists post, s = main_spec_ext' prog ora post
+| None => False
+end.
 
 Lemma semax_func_nil:
-   forall
-     V G {C: compspecs}, semax_func V G nil nil.
+forall
+ V G {C: compspecs} ge, @semax_func V G C ge nil nil.
 Proof.
-intros; split; auto.
-constructor.
-intros. rename H0 into HGG.
+intros; split. constructor. split; [ hnf; intros; inv H | intros].
+(*rename H0 into HGG.*)
 intros b fsig cc ty P Q w ? ?.
-hnf in H1.
-destruct H1 as [b' [NEP [NEQ [? ?]]]].
-simpl in H1.
-rewrite PTree.gempty in H1. inv H1.
+hnf in H0.
+destruct H0 as [b' [NEP [NEQ [? ?]]]].
+simpl in H0.
+rewrite PTree.gempty in H0. inv H0.
 Qed.
 
 Program Definition HO_pred_eq {T}{agT: ageable T}
-    (A: Type) (P: A -> pred T) (A': Type) (P': A' -> pred T) : pred nat :=
- fun v => exists H: A=A',
-     match H in (_ = A) return (A -> pred T) -> Prop with
-     | refl_equal => fun (u3: A -> pred T) =>
-                                    forall x: A, (P x <=> u3 x) v
-     end P'.
- Next Obligation.
-  intros; intro; intros.
-  destruct H0. exists x.
-  destruct x.
-   intros. specialize (H0 x). eapply pred_hereditary; eauto.
- Qed.
+(A: Type) (P: A -> pred T) (A': Type) (P': A' -> pred T) : pred nat :=
+fun v => exists H: A=A',
+ match H in (_ = A) return (A -> pred T) -> Prop with
+ | refl_equal => fun (u3: A -> pred T) =>
+                                forall x: A, (P x <=> u3 x) v
+ end P'.
+Next Obligation.
+intros; intro; intros.
+destruct H0. exists x.
+destruct x.
+intros. specialize (H0 x). eapply pred_hereditary; eauto.
+Qed.
 
 Lemma laterR_level: forall w w' : rmap, laterR w w' -> (level w > level w')%nat.
 Proof.
@@ -193,9 +227,9 @@ omega.
 Qed.
 
 Lemma HO_pred_eq_i1:
-  forall A P P' m,
-      approx (level m) oo  P = approx (level m) oo P' ->
-    (|> HO_pred_eq A P A  P') m.
+forall A P P' m,
+  approx (level m) oo  P = approx (level m) oo P' ->
+(|> HO_pred_eq A P A  P') m.
 Proof.
 intros.
 unfold HO_pred_eq.
@@ -209,13 +243,13 @@ unfold compose in *.
 apply clos_trans_t1n in H0.
 revert H; induction H0; intros.
 2 : { apply IHclos_trans_1n.
-      unfold age,age1 in H. unfold ag_nat in H. unfold natAge1 in H. destruct x0; inv H.
-      clear - H1.
-      assert (forall w, app_pred (approx (level (S y)) (P x)) w <-> app_pred (approx (level (S y)) (P' x)) w).
-      { intros; rewrite H1; intuition. }
-      apply pred_ext; intros w ?; destruct (H w); simpl in *; intuition.
-      apply H0; auto. clear - H4.  unfold natLevel in *. omega.
-      apply H2; auto. clear - H4.  unfold natLevel in *. omega. }
+  unfold age,age1 in H. unfold ag_nat in H. unfold natAge1 in H. destruct x0; inv H.
+  clear - H1.
+  assert (forall w, app_pred (approx (level (S y)) (P x)) w <-> app_pred (approx (level (S y)) (P' x)) w).
+  { intros; rewrite H1; intuition. }
+  apply pred_ext; intros w ?; destruct (H w); simpl in *; intuition.
+  apply H0; auto. clear - H4.  unfold natLevel in *. omega.
+  apply H2; auto. clear - H4.  unfold natLevel in *. omega. }
 unfold age,age1 in H. unfold ag_nat in H. unfold natAge1 in H. destruct x0; inv H.
 intros z ?.
 split; intros ? ? ?.
@@ -236,12 +270,12 @@ simpl in H3. destruct H3; auto.
 Qed.
 
 Lemma semax_func_cons_aux:
-  forall (psi: genv) id fsig1 cc1 A1 P1 Q1 NEP1 NEQ1 fsig2 cc2 A2 P2 Q2 (V: varspecs) (G': funspecs) {C: compspecs} b fs,
-  Genv.find_symbol psi id = Some b ->
-  ~ In id (map (fst (A:=ident) (B:=fundef)) fs) ->
-   match_fdecs fs G'  ->
-   claims  psi (nofunc_tycontext V ((id, mk_funspec fsig1 cc1 A1 P1 Q1 NEP1 NEQ1) :: G')) (Vptr b Ptrofs.zero) fsig2 cc2 A2 P2 Q2 ->
-    fsig1=fsig2 /\ cc1 = cc2 /\ A1=A2 /\ JMeq P1 P2 /\ JMeq Q1 Q2.
+forall (psi: genv) id fsig1 cc1 A1 P1 Q1 NEP1 NEQ1 fsig2 cc2 A2 P2 Q2 (V: varspecs) (G': funspecs) {C: compspecs} b fs,
+Genv.find_symbol psi id = Some b ->
+~ In id (map (fst (A:=ident) (B:=fundef)) fs) ->
+match_fdecs fs G'  ->
+claims  psi (nofunc_tycontext V ((id, mk_funspec fsig1 cc1 A1 P1 Q1 NEP1 NEQ1) :: G')) (Vptr b Ptrofs.zero) fsig2 cc2 A2 P2 Q2 ->
+fsig1=fsig2 /\ cc1 = cc2 /\ A1=A2 /\ JMeq P1 P2 /\ JMeq Q1 Q2.
 Proof.
 intros until fs. intros H Hin Hmf; intros.
 destruct H0 as [id' [NEP2 [NEQ2 [? ?]]]].
@@ -276,70 +310,90 @@ eapply match_fdecs_in in Hmf; eauto.
 Qed.
 
 Lemma var_block'_cenv_sub {CS CS'} (CSUB: cenv_sub CS CS') sh a
-  (CT: complete_type CS (@snd ident type a) = true):
-  var_block' sh CS a = var_block' sh CS' a.
+(CT: complete_type CS (@snd ident type a) = true):
+var_block' sh CS a = var_block' sh CS' a.
 Proof.
-  extensionality rho.
-  unfold var_block'. rewrite (cenv_sub_sizeof CSUB); trivial.
+extensionality rho.
+unfold var_block'. rewrite (cenv_sub_sizeof CSUB); trivial.
 Qed. 
 
 Lemma stackframe_of'_cenv_sub {CS CS'} (CSUB: cenv_sub CS CS') f
-      (COMPLETE : Forall (fun it : ident * type => complete_type CS (snd it) = true) (fn_vars f)):
-  stackframe_of' CS f = stackframe_of' CS' f .
+  (COMPLETE : Forall (fun it : ident * type => complete_type CS (snd it) = true) (fn_vars f)):
+stackframe_of' CS f = stackframe_of' CS' f .
 Proof.
-  extensionality rho. 
-  unfold stackframe_of'. forget (fn_vars f) as vars.
-  induction vars; simpl; trivial.
-  inv COMPLETE. rewrite (var_block'_cenv_sub CSUB _ _ H1), IHvars; clear IHvars; trivial.
+extensionality rho. 
+unfold stackframe_of'. forget (fn_vars f) as vars.
+induction vars; simpl; trivial.
+inv COMPLETE. rewrite (var_block'_cenv_sub CSUB _ _ H1), IHvars; clear IHvars; trivial.
 Qed.
 
-Lemma semax_func_cons:
-   forall
-         fs id f cc (A: TypeTree) P Q NEP NEQ (V: varspecs) (G G': funspecs) {C: compspecs},
-      andb (id_in_list id (map (@fst _ _) G))
-      (andb (negb (id_in_list id (map (@fst ident fundef) fs)))
-        (semax_body_params_ok f)) = true ->
-      Forall
-         (fun it : ident * type =>
-          complete_type cenv_cs (snd it) =
-          true) (fn_vars f) ->
-       var_sizes_ok cenv_cs (f.(fn_vars)) ->
-       f.(fn_callconv) = cc ->
-       precondition_closed f P ->
-      semax_body V G f (id, mk_funspec (fn_funsig f) cc A P Q NEP NEQ) ->
-      semax_func V G fs G' ->
-      semax_func V G ((id, Internal f)::fs)
-           ((id, mk_funspec (fn_funsig f) cc A P Q NEP NEQ)  :: G').
+Lemma var_block_cenv_sub {CS CS'} (CSUB: cspecs_sub CS CS') sh a
+(CT: complete_type (@cenv_cs CS) (@snd ident type a) = true):
+@var_block sh CS a = @var_block sh CS' a.
+Proof.
+extensionality rho.
+unfold var_block. rewrite (cenv_sub_sizeof CSUB); trivial.
+Qed. 
+
+Lemma stackframe_of_cenv_sub {CS CS'} (CSUB: cspecs_sub CS CS') f
+  (COMPLETE : Forall (fun it : ident * type => complete_type (@cenv_cs CS) (snd it) = true) (fn_vars f)):
+@stackframe_of CS f = @stackframe_of CS' f .
+Proof.
+extensionality rho. 
+unfold stackframe_of. forget (fn_vars f) as vars.
+induction vars; simpl; trivial.
+inv COMPLETE. rewrite (var_block_cenv_sub CSUB _ _ H1), IHvars; clear IHvars; trivial.
+Qed.
+
+Lemma semax_body_cenv_sub {CS CS'} (CSUB: cspecs_sub CS CS') V G f spec
+(COMPLETE : Forall (fun it : ident * type => complete_type (@cenv_cs CS) (snd it) = true) (fn_vars f)):
+@semax_body V G CS f spec -> @semax_body V G CS' f spec.
+Proof.
+destruct spec. simpl. destruct f0; intros.  specialize (H Espec0 ts x).
+rewrite <- (stackframe_of_cenv_sub CSUB); [apply (semax_cssub CSUB); apply H | trivial].
+Qed. 
+
+Lemma semax_func_cons: forall 
+     fs id f cc (A: TypeTree) P Q NEP NEQ (V: varspecs) (G G': funspecs) {C: compspecs} ge,
+  andb (id_in_list id (map (@fst _ _) G))
+  (andb (negb (id_in_list id (map (@fst ident fundef) fs)))
+    (semax_body_params_ok f)) = true ->
+  Forall
+     (fun it : ident * type =>
+      complete_type cenv_cs (snd it) =
+      true) (fn_vars f) ->
+   var_sizes_ok cenv_cs (f.(fn_vars)) ->
+   f.(fn_callconv) = cc ->
+ (*NEW*)  (exists b, Genv.find_symbol ge id = Some b /\ Genv.find_funct_ptr ge b = Some (Internal f)) -> 
+   precondition_closed f P ->
+  semax_body V G f (id, mk_funspec (fn_funsig f) cc A P Q NEP NEQ) ->
+  semax_func V G ge fs G' ->
+  semax_func V G ge ((id, Internal f)::fs)
+       ((id, mk_funspec (fn_funsig f) cc A P Q NEP NEQ)  :: G').
 Proof.
 intros until C.
-intros H' COMPLETE Hvars Hcc Hpclos H3 [Hf' Hf].
+intros ge H' COMPLETE Hvars Hcc [b [Hb1 Hb2]] Hpclos H3 [HfsG' [Hfs HG]].
 apply andb_true_iff in H'.
 destruct H' as [Hin H'].
 apply andb_true_iff in H'.
-destruct H' as [Hni H].
+destruct H' as [Hni H]. 
 split.
-simpl. constructor 2; auto.
+{ simpl. econstructor 2; auto.
 simpl.
-unfold type_of_function. f_equal. auto.
-intros ge H0 HGG n.
-assert (prog_contains ge fs).
-unfold prog_contains in *.
-intros.
-apply H0.
-simpl.
-auto.
-specialize (Hf ge H1 HGG).
-clear H1.
-hnf in Hf|-*.
+unfold type_of_function. f_equal. auto. }
+apply id_in_list_true in Hin. rewrite negb_true_iff in Hni.
+split.
+{ hnf; intros. destruct H0; [ symmetry in H0; inv H0 | apply (Hfs _ _ H0)].
+exists b; split; trivial. } 
+intros ge' H0 HGG n.
+specialize (HG _ H0 HGG).
+hnf in HG |- *. 
 intros v fsig cc' A' P' Q'.
 apply derives_imp.
 clear n.
 intros n ?.
-subst cc.
-specialize (H0 id (Internal f)).
-destruct H0 as [b [? ?]]; [left; auto |].
-rewrite <- Genv.find_funct_find_funct_ptr in H2.
-apply negb_true_iff in Hni.
+subst cc. 
+rewrite <- Genv.find_funct_find_funct_ptr in Hb2.
 apply id_in_list_false in Hni.
 destruct (eq_dec  (Vptr b Ptrofs.zero) v) as [?H|?H].
 * (* Vptr b Ptrofs.zero = v *)
@@ -353,34 +407,30 @@ destruct H as [H H'].
 apply compute_list_norepet_e in H.
 apply compute_list_norepet_e in H'.
 (*split3; auto.*)
-rewrite Genv.find_funct_find_funct_ptr in H2; auto.
+rewrite Genv.find_funct_find_funct_ptr in Hb2; auto.
+split; auto.
+split. { specialize (HGG b). unfold fundef in HGG;  rewrite Hb2 in HGG; simpl in HGG.
+      unfold fundef; simpl. rewrite HGG; trivial. } 
 split; auto.
 split; auto.
 split; auto.
-split; auto.
-split; auto.
-(*
-rewrite HGG; auto.
-split; auto.
-split; auto.
-split.
-rewrite HGG; auto.*)
-(* split; auto.*)
 destruct H1 as [id' [NEP' [NEQ' [? [b' [? ?]]]]]].
-symmetry in H5; inv H5.
+symmetry in H4; inv H4.
 destruct (eq_dec id id').
 subst.
 simpl in H1.
 rewrite PTree.gss in H1.
 inv H1; auto.
-contradiction (Genv.global_addresses_distinct ge n0 H0 H4); auto.
+specialize (H0 id); unfold fundef in H0. simpl in H0.  rewrite Hb1 in H0; simpl in H0.
+simpl in H2. 
+contradiction (Genv.global_addresses_distinct ge' n0 H0 H2); auto.
 +
-  (*destruct H. *) 
+(*destruct H. *) 
 intros Delta' CS' k NK HDelta' w KW CSUB.
 intros ts x.
-simpl in H1.
-pose proof (semax_func_cons_aux ge _ _ _ _ _ _ _ _ _ _ _ _ _ _ _ _ _ H0 Hni Hf' H1).
-destruct H4 as [H4' [H4 [H4a [H4b H4c]]]].
+simpl in H1. specialize (H0 id); unfold fundef in H0; simpl in H0. rewrite Hb1 in H0; simpl in H0.
+pose proof (semax_func_cons_aux (Build_genv ge' cenv_cs) _ _ _ _ _ _ _ _ _ _ _ _ _ _ _ _ _ H0 Hni HfsG' H1).
+destruct H2 as [H4' [H4 [H4a [H4b H4c]]]].
 subst A' fsig cc'.
 apply JMeq_eq in H4b.
 apply JMeq_eq in H4c.
@@ -391,29 +441,16 @@ pose proof I.
 (*specialize (H4 n).*)specialize (H4 k).
 apply now_later. 
 rewrite <- (stackframe_of'_cenv_sub CSUB); trivial.
-apply (semax'_cssub CSUB). Set Printing Implicit.
+apply (semax'_cssub CSUB).
 (*rewrite HGG.*)
 clear - Hpclos H4 NK KW HDelta'.
 rewrite semax_fold_unfold in H4|-*. intros gx DD CS' u WU [SUB GX] v UV BEL.
 assert (HDD: tycontext_sub (func_tycontext f V G nil) DD).
 { unfold func_tycontext, func_tycontext'. simpl.
-  eapply tycontext_sub_trans; eauto. }
+eapply tycontext_sub_trans; eauto. }
 assert (WV: @necR nat ag_nat w v). { eapply necR_trans.  apply WU. apply UV. }
 specialize (H4 gx DD CS' _ KW (conj HDD GX) v WV BEL). 
 revert H4.
-(*{ unfold func_tycontext, func_tycontext'. simpl.
-  apply prop_derives. intros [AA BB]; split; trivial.
-  eapply tycontext_sub_trans. 2: eassumption.
-  unfold make_tycontext; simpl.
-  repeat split; simpl; intros.
-  + destruct ((make_tycontext_t (fn_params f) (fn_temps f)) ! id ); trivial.
-    destruct p. rewrite orb_comm, orb_negb_r; split; trivial.
-  + apply sub_option_refl.
-  + apply sub_option_refl.
-  + rewrite PTree.gempty.
-    unfold Annotation_sub; simpl. destruct (PTree.get id (make_tycontext_a Ann)); trivial. destruct a; trivial.
-} *)
-(*apply imp_derives; auto.*)
 apply allp_derives; intro kk.
 apply allp_derives; intro F.
 apply imp_derives; auto.
@@ -431,38 +468,38 @@ apply andp_left2; auto.
 destruct (Hpclos ts x).
 apply close_precondition_e; auto.
 * (***   Vptr b Ptrofs.zero <> v'  ********)
-apply (Hf n v fsig cc' A' P' Q'); auto.
+apply (HG n v fsig cc' A' P' Q'); auto.
 destruct H1 as [id' [NEP' [NEQ' [? ?]]]].
 simpl in H1.
 destruct (eq_dec id id').
 subst. rewrite PTree.gss in H1.
-destruct H5 as [? [? ?]]. congruence.
+destruct H4 as [? [? ?]]. specialize (H0 id'); unfold fundef in H0; simpl in H0. rewrite Hb1 in H0; simpl in H0. unfold fundef in H4; simpl in H4; congruence.
 rewrite PTree.gso in H1 by auto.
 exists id', NEP', NEQ'; split; auto.
 Qed.
 
 (* EXPERIMENT
 Lemma semax_func_skip:
-   forall
-        V (G: funspecs) {C: compspecs} fs idf (G': funspecs),
-      semax_func V G fs G' ->
-      semax_func V G (idf::fs) G'.
+forall
+    V (G: funspecs) {C: compspecs} fs idf (G': funspecs),
+  semax_func V G fs G' ->
+  semax_func V G (idf::fs) G'.
 Proof.
- intros.
- hnf in H|-*.
- destruct H; split.
- constructor 3. auto.
- intros.
- eapply H0; eauto.
- hnf in H1|-*.
- intros; eapply H1; eauto.
- right; auto.
+intros.
+hnf in H|-*.
+destruct H; split.
+constructor 3. auto.
+intros.
+eapply H0; eauto.
+hnf in H1|-*.
+intros; eapply H1; eauto.
+right; auto.
 Qed.
 *)
 
 Lemma semax_external_FF:
- forall Espec ids ef A n,
-  @semax_external Espec ids ef A (fun _ _ _ => FF) (fun _ _ _ => FF) n.
+forall Espec ids ef A n,
+@semax_external Espec ids ef A (fun _ _ _ => FF) (fun _ _ _ => FF) n.
 intros.
 hnf; intros.
 simpl.
@@ -472,29 +509,30 @@ contradiction.
 Qed.
 
 Lemma semax_func_cons_ext:
-   forall (V: varspecs) (G: funspecs) {C: compspecs} fs id ef argsig retsig A P Q NEP NEQ
-          argsig'
-          (G': funspecs) cc (ids: list ident),
-      ids = map fst argsig' -> (* redundant but useful for the client,
-               to calculate ids by reflexivity *)
-      argsig' = zip_with_tl ids argsig ->
-      ef_sig ef =
-      mksignature
-        (typlist_of_typelist (type_of_params argsig'))
-        (opttyp_of_type retsig) cc ->
-      id_in_list id (map (@fst _ _) fs) = false ->
-      length ids = length (typelist2list argsig) ->
-      (forall gx ts x (ret : option val),
-         (Q ts x (make_ext_rval gx ret)
-            && !!has_opttyp ret (opttyp_of_type retsig)
-            |-- !!tc_option_val retsig ret)) ->
-      (forall n, semax_external Espec ids ef A P Q n) ->
-      semax_func V G fs G' ->
-      semax_func V G ((id, External ef argsig retsig cc)::fs)
-           ((id, mk_funspec (argsig', retsig) cc A P Q NEP NEQ)  :: G').
+forall (V: varspecs) (G: funspecs) {C: compspecs} ge fs id ef argsig retsig A P Q NEP NEQ
+      argsig'
+      (G': funspecs) cc (ids: list ident),
+  ids = map fst argsig' -> (* redundant but useful for the client,
+           to calculate ids by reflexivity *)
+  argsig' = zip_with_tl ids argsig ->
+  ef_sig ef =
+  mksignature
+    (typlist_of_typelist (type_of_params argsig'))
+    (opttyp_of_type retsig) cc ->
+  id_in_list id (map (@fst _ _) fs) = false ->
+  length ids = length (typelist2list argsig) ->
+  (forall gx ts x (ret : option val),
+     (Q ts x (make_ext_rval gx ret)
+        && !!has_opttyp ret (opttyp_of_type retsig)
+        |-- !!tc_option_val retsig ret)) ->
+(*new*)     (exists b : block, Genv.find_symbol ge id = Some b /\ Genv.find_funct_ptr ge b = Some (External ef argsig retsig cc)) ->
+  (forall n, semax_external Espec ids ef A P Q n) ->
+  semax_func V G ge fs G' ->
+  semax_func V G ge ((id, External ef argsig retsig cc)::fs)
+       ((id, mk_funspec (argsig', retsig) cc A P Q NEP NEQ)  :: G').
 Proof.
 intros until ids.
-intros Hids Hargsig Hef Hni Hlen Hretty H [Hf' Hf].
+intros Hids Hargsig Hef Hni Hlen Hretty B H [Hf' [GC Hf]].
 rewrite Hargsig in *.  clear Hids Hargsig argsig'.
 apply id_in_list_false in Hni.
 split.
@@ -506,65 +544,55 @@ revert ids Hlen; induction argsig; simpl; intros; auto.
 destruct ids; auto.
 destruct ids; auto. inv Hlen. simpl. f_equal; auto.
 auto.
-intros ge ? HGG; intros.
-assert (prog_contains ge fs).
-unfold prog_contains in *.
-intros.
-apply H0.
-simpl.
-auto.
-specialize (Hf ge H1 HGG).
-clear H1.
+split; [ clear - B GC; red; intros; destruct H; [ symmetry in H; inv H; apply B | apply GC; trivial] |]. 
+intros ge' GE1 GE2 ?.
+specialize (Hf ge' GE1 GE2). 
 unfold believe.
 intros v' fsig' cc' A' P' Q'.
-apply derives_imp.
-clear n.
-intros n ?.
-unfold prog_contains in H0.
-generalize (H0 id (External ef argsig retsig cc)); clear H0; intro H0.
-destruct H0 as [b [? ?]].
-left; auto.
-rewrite <- Genv.find_funct_find_funct_ptr in H2.
+apply derives_imp. clear n. intros n ?. 
+destruct B as [b [B1 B2]].
+specialize (GE1 id); simpl in GE1. unfold fundef in GE1; rewrite B1 in GE1; simpl in GE1. 
+specialize (GE2 b); simpl in GE2. unfold fundef in GE2; rewrite B2 in GE2; simpl in GE2.
 destruct (eq_dec  (Vptr b Ptrofs.zero) v') as [?H|?H].
-subst v'.
++ subst v'.
 left.
 specialize (H n).
-pose proof (semax_func_cons_aux ge _ _ _ _ _ _ _ _ _ _ _ _ _ _ _ _ _ H0 Hni Hf' H1).
-destruct H3 as [H4' [H4'' [H4 [H4b H4c]]]].
+destruct (semax_func_cons_aux {| genv_genv := ge'; genv_cenv := cenv_cs |} _ _ _ _ _ _ _ _ _ _ _ _ _ _ _ _ _ GE1 Hni Hf' H0)
+as [H4' [H4'' [H4 [H4b H4c]]]].
 subst A' fsig' cc'.
 apply JMeq_eq in H4b.
 apply JMeq_eq in H4c.
 subst P' Q'.
-unfold believe_external.
-rewrite H2.
+unfold believe_external; simpl; rewrite if_true; trivial. 
+unfold fundef in GE2; unfold fundef; simpl; rewrite GE2.
 assert (Hty: map fst (zip_with_tl ids argsig) = ids).
 { clear -Hlen. revert argsig Hlen. induction ids; auto.
-  simpl; intros. destruct argsig; auto. inv Hlen.
-  simpl. f_equal. auto. }
+simpl; intros. destruct argsig; auto. inv Hlen.
+simpl. f_equal. auto. }
 rewrite fst_split. simpl map. rewrite Hty.
 split; auto.
 split; auto. split; auto.
 intros ts x ret phi Hlev Hx Hnec. apply Hretty.
-
++
 (* **   Vptr b Ptrofs.zero <> v'  ********)
 apply (Hf n v' fsig' cc' A' P' Q'); auto.
-destruct H1 as [id' [NEP' [NEQ' [? ?]]]].
-simpl in H1.
+destruct H0 as [id' [NEP' [NEQ' [? ?]]]].
+simpl in H0.
 destruct (eq_dec id id').
-subst. rewrite PTree.gss in H1. inv H1.
-destruct H4 as [? [? ?]]; congruence.
-exists id', NEP', NEQ'; split; auto.
-simpl. rewrite PTree.gso in H1 by auto; auto.
+- subst id'. rewrite PTree.gss in H0. inv H0.
+destruct H2 as [? [? ?]]; subst. unfold fundef in H0; simpl in H0. congruence.
+- exists id', NEP', NEQ'; split; auto.
+simpl. rewrite PTree.gso in H0 by auto; auto.
 Qed.
 
 Definition main_params (ge: genv) start : Prop :=
-  exists b, exists func,
-    Genv.find_symbol ge start = Some b /\
-        Genv.find_funct ge (Vptr b Ptrofs.zero) = Some (Internal func) /\
-        func.(fn_params) = nil.
+exists b, exists func,
+Genv.find_symbol ge start = Some b /\
+    Genv.find_funct ge (Vptr b Ptrofs.zero) = Some (Internal func) /\
+    func.(fn_params) = nil.
 
 Lemma in_prog_funct'_in {F V}:
-  forall i f (g: list (ident * globdef F V)), In (i,f) (prog_funct' g) -> In (i, Gfun f) g.
+forall i f (g: list (ident * globdef F V)), In (i,f) (prog_funct' g) -> In (i, Gfun f) g.
 Proof.
 induction g; intros. inv H. simpl in *.
 destruct a; destruct g0. simpl in H. destruct H; auto. left; congruence.
@@ -572,13 +600,13 @@ right; auto.
 Qed.
 
 Lemma in_prog_funct_in_prog_defs:
-  forall i f prog, In (i,f) (prog_funct prog) -> In (i, Gfun f) (prog_defs prog).
+forall i f prog, In (i,f) (prog_funct prog) -> In (i, Gfun f) (prog_defs prog).
 Proof.
- intros; apply in_prog_funct'_in; auto.
+intros; apply in_prog_funct'_in; auto.
 Qed.
 
 Lemma in_prog_vars_in_prog_defs:
-  forall i v prog, In (i,v) (prog_vars prog) -> In (i, Gvar v) (prog_defs prog).
+forall i v prog, In (i,v) (prog_vars prog) -> In (i, Gvar v) (prog_defs prog).
 Proof.
 unfold prog_vars. intros ? ? ?.
 induction (prog_defs prog); intros. inv H. simpl in *.
@@ -586,17 +614,17 @@ destruct a; destruct g. auto. simpl in H. destruct H; auto. left; congruence.
 Qed.
 
 Lemma find_funct_ptr_exists:
-  forall (p: program) id f,
-  list_norepet (prog_defs_names p) ->
-  In (id, Gfun f) (prog_defs p) ->
-  exists b,
-     Genv.find_symbol (Genv.globalenv p) id = Some b
-  /\ Genv.find_funct_ptr (Genv.globalenv p) b = Some f.
+forall (p: program) id f,
+list_norepet (prog_defs_names p) ->
+In (id, Gfun f) (prog_defs p) ->
+exists b,
+ Genv.find_symbol (Genv.globalenv p) id = Some b
+/\ Genv.find_funct_ptr (Genv.globalenv p) b = Some f.
 Proof.
 intros.
 pose proof (prog_defmap_norepet _ _ _ H H0).
 destruct (proj1 (Genv.find_def_symbol _ _ _) H1)
-  as [b [? ?]].
+as [b [? ?]].
 exists b; split; auto.
 unfold Genv.find_funct_ptr.
 rewrite H3.
@@ -604,77 +632,69 @@ auto.
 Qed.
 
 Lemma funassert_initial_core:
-  forall (prog: program) ve te V G n,
-      list_norepet (prog_defs_names prog) ->
-      match_fdecs (prog_funct prog) G ->
-      app_pred (funassert (nofunc_tycontext V G) (mkEnviron (filter_genv (globalenv prog)) ve te))
-                      (initial_core (Genv.globalenv prog) G n).
+forall (prog: program) ve te V G n,
+  list_norepet (prog_defs_names prog) ->
+  match_fdecs (prog_funct prog) G ->
+  app_pred (funassert (nofunc_tycontext V G) (mkEnviron (filter_genv (globalenv prog)) ve te))
+                  (initial_core (Genv.globalenv prog) G n).
 Proof.
- intros; split.
+intros; split.
+* intros id fs.
+apply prop_imp_i; intros.
+simpl ge_of; simpl fst; simpl snd.
+unfold filter_genv, Map.get.
+assert (exists f, In (id, f) (prog_funct prog)). {
+  simpl in H1.
+  forget (prog_funct prog) as g.
+  clear - H1 H0.
+  revert G H1 H0; induction g; destruct G; intros; simpl in *.
+  elimtype False.
+  rewrite PTree.gempty in H1; inv H1.
+  inv H0.
+  destruct a; simpl in *; subst.
+  destruct (eq_dec i id). subst; eauto.
+  specialize (IHg nil H1). inv H0.
+  destruct a. destruct p.
+  inv H0.
+  simpl in H1.
+  destruct (ident_eq i0 id). subst. eauto.
+  destruct (IHg G); auto. rewrite PTree.gso in H1; auto.
+  eauto.
+}
+destruct H2 as [f ?].
+destruct (find_funct_ptr_exists prog id f) as [b [? ?]]; auto.
+apply in_prog_funct_in_prog_defs; auto.
+exists b. unfold fundef.
+unfold globalenv. simpl. rewrite H3.
+split; auto.
+unfold func_at. destruct fs as [f0 cc0 A a a0].
+unfold initial_core.
+hnf. rewrite resource_at_make_rmap.
+rewrite level_make_rmap.
+unfold initial_core'.
+simpl.
+rewrite (Genv.find_invert_symbol (Genv.globalenv prog) id); auto.
+assert (H9: In (id, mk_funspec f0 cc0 A a a0 P_ne Q_ne) G). {
+  clear - H1.
+  simpl in H1. unfold make_tycontext_g in H1; simpl in H1.
+  induction G; simpl in *.
+  rewrite PTree.gempty in H1; inv H1.
+  destruct (ident_eq (fst a1) id); subst.
+  change (@ptree_set) with (@PTree.set) in *. destruct a1; simpl in *.
+  rewrite PTree.gss in H1; inv H1. left; auto.
+  change (@ptree_set) with (@PTree.set) in *. destruct a1; simpl in *. 
+  rewrite PTree.gso in H1; auto.
+}
+rewrite (find_id_i _ _ _ H9); auto.
+clear - H0 H. unfold prog_defs_names, prog_funct in *.
+eapply match_fdecs_norepet; eauto.
+apply list_norepet_prog_funct'; auto.
 *
- intros id fs.
- apply prop_imp_i; intros.
- simpl ge_of; simpl fst; simpl snd.
- unfold filter_genv, Map.get.
- assert (exists f, In (id, f) (prog_funct prog)). {
- simpl in H1.
- forget (prog_funct prog) as g.
-clear - H1 H0.
-revert G H1 H0; induction g; destruct G; intros; simpl in *.
-elimtype False.
-rewrite PTree.gempty in H1; inv H1.
-inv H0.
-destruct a; simpl in *; subst.
-destruct (eq_dec i id). subst; eauto.
- specialize (IHg nil H1). inv H0.
-(*destruct (IHg). destruct g; simpl; auto.
-constructor. apply match_fdecs_nil.
-eauto. *)
-destruct a. destruct p.
- inv H0.
- simpl in H1.
- destruct (ident_eq i0 id). subst. eauto.
- destruct (IHg G); auto. rewrite PTree.gso in H1; auto.
- eauto.
-(* simpl in H1.
- destruct (IHg ((i0,f0)::G)); auto. eauto.
-*)
- }
- destruct H2 as [f ?].
- destruct (find_funct_ptr_exists prog id f) as [b [? ?]]; auto.
- apply in_prog_funct_in_prog_defs; auto.
- exists b. unfold fundef.
- unfold globalenv. simpl. rewrite H3.
- split; auto.
- unfold func_at. destruct fs as [f0 cc0 A a a0].
- unfold initial_core.
- hnf. rewrite resource_at_make_rmap.
- rewrite level_make_rmap.
- unfold initial_core'.
- simpl.
- rewrite (Genv.find_invert_symbol (Genv.globalenv prog) id); auto.
- assert (H9: In (id, mk_funspec f0 cc0 A a a0 P_ne Q_ne) G). {
-   clear - H1.
-    simpl in H1. unfold make_tycontext_g in H1; simpl in H1.
-    induction G; simpl in *.
-    rewrite PTree.gempty in H1; inv H1.
-    destruct (ident_eq (fst a1) id); subst.
-    change (@ptree_set) with (@PTree.set) in *. destruct a1; simpl in *.
-    rewrite PTree.gss in H1; inv H1. left; auto.
-    change (@ptree_set) with (@PTree.set) in *. destruct a1; simpl in *. 
-    rewrite PTree.gso in H1; auto.
- }
- rewrite (find_id_i _ _ _ H9); auto.
- clear - H0 H. unfold prog_defs_names, prog_funct in *.
- eapply match_fdecs_norepet; eauto.
- apply list_norepet_prog_funct'; auto.
-*
- (*intros loc'  [fsig' cc' A' P' Q' NEP' NEQ']; unfold func_at.*)
- intros loc' fsig' cc'.
- intros w ? ?.
- destruct H2 as [pp ?].
- hnf in H2.
- assert (exists pp, initial_core (Genv.globalenv prog) G n @ (loc',0) = PURE (FUN fsig' cc') pp).
+intros loc' fsig' cc'.
+intros w ? ?.
+destruct H2 as [pp ?].
+hnf in H2.
+assert (exists pp, initial_core (Genv.globalenv prog) G n @ (loc',0) = PURE (FUN fsig' cc') pp).
 case_eq (initial_core (@Genv.globalenv (Ctypes.fundef function) type prog) G n @ (loc', 0)); intros.
 destruct (necR_NO _ _ (loc',0) sh n0 H1) as [? _].
 rewrite H4 in H2 by auto.
@@ -691,7 +711,7 @@ if_tac in H3; [ | inv H3].
 simpl.
 simpl @fst in *. 
 revert H3; case_eq (@Genv.invert_symbol (Ctypes.fundef function) 
-      type (@Genv.globalenv (Ctypes.fundef function) type prog) loc' ); intros;
+                                        type (@Genv.globalenv (Ctypes.fundef function) type prog) loc' ); intros;
   [ | congruence].
 revert H5; case_eq (find_id i G); intros; [| congruence].
 destruct f as [?f ?A ?a ?a]; inv H6.
@@ -699,77 +719,73 @@ apply Genv.invert_find_symbol in H3.
 exists i.
 simpl ge_of. unfold filter_genv, Map.get.
 unfold globalenv; simpl.
- unfold fundef; rewrite H3.
- split; auto.
- assert (exists f, In (i,f) (prog_funct prog)
-              /\ type_of_fundef f = Tfunction (type_of_params (fst fsig')) (snd fsig') cc'). {
- clear - H0 H5.
- forget (prog_funct prog) as g.
- revert G H0 H5; induction g; intros.
- inv H0. inv H5.
- inv H0.
- simpl in H5.
- if_tac in H5. subst i0. inv H5. exists fd; split; auto. left; auto.
- destruct (IHg G0) as [f3 [? ?]]; auto. exists f3; split; auto.
- right; auto.
-(*
- destruct (IHg _ H3 H5) as [f [H4 H4']].
- exists f; split; auto. right; auto.
-*)
- }
- clear H4.
- destruct H6 as [f [H4 H4']].
- destruct (find_funct_ptr_exists prog i f) as [b [? ?]]; auto.
- apply in_prog_funct_in_prog_defs; auto.
- unfold fundef in *.
- inversion2 H3 H6.
- case_eq (Genv.find_var_info (Genv.globalenv prog) loc'); intros.
- elimtype False; clear - H7 H6.
- unfold Genv.find_funct_ptr in H7.
- unfold Genv.find_var_info in H6.
- destruct (Genv.find_def (Genv.globalenv prog) loc'); try destruct g0; congruence.
- apply find_id_e in H5. apply in_map_fst in H5.
- clear - H5.
- revert H5; induction G; simpl; intro. contradiction.
- destruct H5. subst.
- change (@ptree_set) with (@PTree.set) in *. destruct a; simpl in *.
- econstructor; rewrite PTree.gss; reflexivity.
- destruct (IHG H) as [fs ?].
- change (@ptree_set) with (@PTree.set) in *. destruct a; simpl in *.
- destruct (eq_dec i0 i). econstructor; subst; rewrite PTree.gss; eauto.
- econstructor; rewrite PTree.gso by auto; eauto.
+unfold fundef; rewrite H3.
+split; auto.
+assert (exists f, In (i,f) (prog_funct prog)
+                  /\ type_of_fundef f = Tfunction (type_of_params (fst fsig')) (snd fsig') cc'). {
+  clear - H0 H5.
+  forget (prog_funct prog) as g.
+  revert G H0 H5; induction g; intros.
+  inv H0. inv H5.
+  inv H0.
+  simpl in H5.
+  if_tac in H5. subst i0. inv H5. exists fd; split; auto. left; auto.
+  destruct (IHg G0) as [f3 [? ?]]; auto. exists f3; split; auto.
+  right; auto.
+}
+clear H4.
+destruct H6 as [f [H4 H4']].
+destruct (find_funct_ptr_exists prog i f) as [b [? ?]]; auto.
+apply in_prog_funct_in_prog_defs; auto.
+unfold fundef in *.
+inversion2 H3 H6.
+case_eq (Genv.find_var_info (Genv.globalenv prog) loc'); intros.
+elimtype False; clear - H7 H6.
+unfold Genv.find_funct_ptr in H7.
+unfold Genv.find_var_info in H6.
+destruct (Genv.find_def (Genv.globalenv prog) loc'); try destruct g0; congruence.
+apply find_id_e in H5. apply in_map_fst in H5.
+clear - H5.
+revert H5; induction G; simpl; intro. contradiction.
+destruct H5. subst.
+change (@ptree_set) with (@PTree.set) in *. destruct a; simpl in *.
+econstructor; rewrite PTree.gss; reflexivity.
+destruct (IHG H) as [fs ?].
+change (@ptree_set) with (@PTree.set) in *. destruct a; simpl in *.
+destruct (eq_dec i0 i). econstructor; subst; rewrite PTree.gss; eauto.
+econstructor; rewrite PTree.gso by auto; eauto.
 Qed.
 
 Lemma prog_contains_prog_funct: forall prog: program,
-      list_norepet (prog_defs_names prog) ->
-          prog_contains (globalenv prog) (prog_funct prog).
+  list_norepet (prog_defs_names prog) ->
+      prog_contains (globalenv prog) (prog_funct prog).
 Proof.
-  intros; intro; intros.
-  apply (find_funct_ptr_exists prog id f); auto.
-  unfold prog_funct in H0.
-  change (AST.prog_defs prog) with (prog_defs prog).
-  induction (prog_defs prog). inv H0.
-   simpl in H0.  destruct a.
-  destruct g. simpl in H0. destruct H0. inv H0.  left. auto.
-  right; auto.  right; auto.
+intros; intro; intros.
+apply (find_funct_ptr_exists prog id f); auto.
+unfold prog_funct in H0.
+change (AST.prog_defs prog) with (prog_defs prog).
+induction (prog_defs prog). inv H0.
+simpl in H0.  destruct a.
+destruct g. simpl in H0. destruct H0. inv H0.  left. auto.
+right; auto.  right; auto.
 Qed.
 
 Lemma funassert_initial_core_ext:
-  forall (ora : OK_ty) (prog: program) ve te V G n,
-      list_norepet (prog_defs_names prog) ->
-      match_fdecs (prog_funct prog) G ->
-      app_pred (funassert (nofunc_tycontext V G) (mkEnviron (filter_genv (globalenv prog)) ve te))
-                      (initial_core_ext ora (Genv.globalenv prog) G n).
+forall (ora : OK_ty) (prog: program) ve te V G n,
+  list_norepet (prog_defs_names prog) ->
+  match_fdecs (prog_funct prog) G ->
+  app_pred (funassert (nofunc_tycontext V G) (mkEnviron (filter_genv (globalenv prog)) ve te))
+                  (initial_core_ext ora (Genv.globalenv prog) G n).
 Proof.
- intros; split.
+intros; split.
 *
- intros id fs.
- apply prop_imp_i; intros.
- simpl ge_of; simpl fst; simpl snd.
- unfold filter_genv, Map.get.
- assert (exists f, In (id, f) (prog_funct prog)). {
- simpl in H1.
- forget (prog_funct prog) as g.
+intros id fs.
+apply prop_imp_i; intros.
+simpl ge_of; simpl fst; simpl snd.
+unfold filter_genv, Map.get.
+assert (exists f, In (id, f) (prog_funct prog)). {
+simpl in H1.
+forget (prog_funct prog) as g.
 clear - H1 H0.
 revert G H1 H0; induction g; destruct G; intros; simpl in *.
 elimtype False.
@@ -777,55 +793,55 @@ rewrite PTree.gempty in H1; inv H1.
 inv H0.
 destruct a; simpl in *; subst.
 destruct (eq_dec i id). subst; eauto.
- specialize (IHg nil H1). inv H0.
+specialize (IHg nil H1). inv H0.
 (*destruct (IHg). destruct g; simpl; auto.
 constructor. apply match_fdecs_nil.
 eauto. *)
 destruct a. destruct p.
- inv H0.
- simpl in H1.
- destruct (ident_eq i0 id). subst. eauto.
- destruct (IHg G); auto. rewrite PTree.gso in H1; auto.
- eauto.
+inv H0.
+simpl in H1.
+destruct (ident_eq i0 id). subst. eauto.
+destruct (IHg G); auto. rewrite PTree.gso in H1; auto.
+eauto.
 (* simpl in H1.
- destruct (IHg ((i0,f0)::G)); auto. eauto.
+destruct (IHg ((i0,f0)::G)); auto. eauto.
 *)
- }
- destruct H2 as [f ?].
- destruct (find_funct_ptr_exists prog id f) as [b [? ?]]; auto.
- apply in_prog_funct_in_prog_defs; auto.
- exists b. unfold fundef.
- unfold globalenv. simpl. rewrite H3.
- split; auto.
- unfold func_at. destruct fs as [f0 cc0 A a a0].
- unfold initial_core_ext.
- hnf. rewrite resource_at_make_rmap.
- rewrite level_make_rmap.
- unfold initial_core'.
- simpl.
- rewrite (Genv.find_invert_symbol (Genv.globalenv prog) id); auto.
- assert (H9: In (id, mk_funspec f0 cc0 A a a0 P_ne Q_ne) G). {
-   clear - H1.
-    simpl in H1. unfold make_tycontext_g in H1; simpl in H1.
-    induction G; simpl in *.
-    rewrite PTree.gempty in H1; inv H1.
-    destruct (ident_eq (fst a1) id); subst.
-    change (@ptree_set) with (@PTree.set) in *. destruct a1; simpl in *.
-    rewrite PTree.gss in H1; inv H1. left; auto.
-    change (@ptree_set) with (@PTree.set) in *. destruct a1; simpl in *. 
-    rewrite PTree.gso in H1; auto.
- }
- rewrite (find_id_i _ _ _ H9); auto.
- clear - H0 H. unfold prog_defs_names, prog_funct in *.
- eapply match_fdecs_norepet; eauto.
- apply list_norepet_prog_funct'; auto.
+}
+destruct H2 as [f ?].
+destruct (find_funct_ptr_exists prog id f) as [b [? ?]]; auto.
+apply in_prog_funct_in_prog_defs; auto.
+exists b. unfold fundef.
+unfold globalenv. simpl. rewrite H3.
+split; auto.
+unfold func_at. destruct fs as [f0 cc0 A a a0].
+unfold initial_core_ext.
+hnf. rewrite resource_at_make_rmap.
+rewrite level_make_rmap.
+unfold initial_core'.
+simpl.
+rewrite (Genv.find_invert_symbol (Genv.globalenv prog) id); auto.
+assert (H9: In (id, mk_funspec f0 cc0 A a a0 P_ne Q_ne) G). {
+clear - H1.
+simpl in H1. unfold make_tycontext_g in H1; simpl in H1.
+induction G; simpl in *.
+rewrite PTree.gempty in H1; inv H1.
+destruct (ident_eq (fst a1) id); subst.
+change (@ptree_set) with (@PTree.set) in *. destruct a1; simpl in *.
+rewrite PTree.gss in H1; inv H1. left; auto.
+change (@ptree_set) with (@PTree.set) in *. destruct a1; simpl in *. 
+rewrite PTree.gso in H1; auto.
+}
+rewrite (find_id_i _ _ _ H9); auto.
+clear - H0 H. unfold prog_defs_names, prog_funct in *.
+eapply match_fdecs_norepet; eauto.
+apply list_norepet_prog_funct'; auto.
 *
- (*intros loc'  [fsig' cc' A' P' Q' NEP' NEQ']; unfold func_at.*)
- intros loc'  fsig' cc'.
- intros w ? ?.
- destruct H2 as [pp ?].
- hnf in H2.
- assert (exists pp, initial_core_ext ora (Genv.globalenv prog) G n @ (loc',0) = PURE (FUN fsig' cc') pp).
+(*intros loc'  [fsig' cc' A' P' Q' NEP' NEQ']; unfold func_at.*)
+intros loc'  fsig' cc'.
+intros w ? ?.
+destruct H2 as [pp ?].
+hnf in H2.
+assert (exists pp, initial_core_ext ora (Genv.globalenv prog) G n @ (loc',0) = PURE (FUN fsig' cc') pp).
 case_eq (initial_core_ext ora (Genv.globalenv prog) G n @ (loc',0)); intros.
 destruct (necR_NO _ _ (loc',0) sh n0 H1) as [? _].
 rewrite H4 in H2 by auto.
@@ -842,74 +858,74 @@ if_tac in H3; [ | inv H3].
 simpl.
 simpl @fst in *.
 revert H3; case_eq (@Genv.invert_symbol (Ctypes.fundef function) type
-              (@Genv.globalenv (Ctypes.fundef function) type prog) loc'); intros;
-  [ | congruence].
+          (@Genv.globalenv (Ctypes.fundef function) type prog) loc'); intros;
+[ | congruence].
 revert H5; case_eq (find_id i G); intros; [| congruence].
 destruct f as [?f ?A ?a ?a]; inv H6.
 apply Genv.invert_find_symbol in H3.
 exists i.
 simpl ge_of. unfold filter_genv, Map.get.
 unfold globalenv; simpl.
- unfold fundef; rewrite H3.
- split; auto.
- assert (exists f, In (i,f) (prog_funct prog)
-              /\ type_of_fundef f = Tfunction (type_of_params (fst fsig')) (snd fsig') cc'). {
- clear - H0 H5.
- forget (prog_funct prog) as g.
- revert G H0 H5; induction g; intros.
- inv H0. inv H5.
- inv H0.
- simpl in H5.
- if_tac in H5. subst i0. inv H5. exists fd; split; auto. left; auto.
- destruct (IHg G0) as [f3 [? ?]]; auto. exists f3; split; auto.
- right; auto.
+unfold fundef; rewrite H3.
+split; auto.
+assert (exists f, In (i,f) (prog_funct prog)
+          /\ type_of_fundef f = Tfunction (type_of_params (fst fsig')) (snd fsig') cc'). {
+clear - H0 H5.
+forget (prog_funct prog) as g.
+revert G H0 H5; induction g; intros.
+inv H0. inv H5.
+inv H0.
+simpl in H5.
+if_tac in H5. subst i0. inv H5. exists fd; split; auto. left; auto.
+destruct (IHg G0) as [f3 [? ?]]; auto. exists f3; split; auto.
+right; auto.
 (*
- destruct (IHg _ H3 H5) as [f [H4 H4']].
- exists f; split; auto. right; auto.
+destruct (IHg _ H3 H5) as [f [H4 H4']].
+exists f; split; auto. right; auto.
 *)
- }
- clear H4.
- destruct H6 as [f [H4 H4']].
- destruct (find_funct_ptr_exists prog i f) as [b [? ?]]; auto.
- apply in_prog_funct_in_prog_defs; auto.
- unfold fundef in *.
- inversion2 H3 H6.
- case_eq (Genv.find_var_info (Genv.globalenv prog) loc'); intros.
- elimtype False; clear - H7 H6.
- unfold Genv.find_funct_ptr in H7.
- unfold Genv.find_var_info in H6.
- destruct (Genv.find_def (Genv.globalenv prog) loc'); try destruct g0; congruence.
- apply find_id_e in H5. apply in_map_fst in H5.
- clear - H5.
- revert H5; induction G; simpl; intro. contradiction.
- destruct H5. subst.
- change (@ptree_set) with (@PTree.set) in *. destruct a; simpl in *.
- econstructor; rewrite PTree.gss; reflexivity.
- destruct (IHG H) as [fs ?].
- change (@ptree_set) with (@PTree.set) in *. destruct a; simpl in *.
- destruct (eq_dec i0 i). econstructor; subst; rewrite PTree.gss; eauto.
- econstructor; rewrite PTree.gso by auto; eauto.
+}
+clear H4.
+destruct H6 as [f [H4 H4']].
+destruct (find_funct_ptr_exists prog i f) as [b [? ?]]; auto.
+apply in_prog_funct_in_prog_defs; auto.
+unfold fundef in *.
+inversion2 H3 H6.
+case_eq (Genv.find_var_info (Genv.globalenv prog) loc'); intros.
+elimtype False; clear - H7 H6.
+unfold Genv.find_funct_ptr in H7.
+unfold Genv.find_var_info in H6.
+destruct (Genv.find_def (Genv.globalenv prog) loc'); try destruct g0; congruence.
+apply find_id_e in H5. apply in_map_fst in H5.
+clear - H5.
+revert H5; induction G; simpl; intro. contradiction.
+destruct H5. subst.
+change (@ptree_set) with (@PTree.set) in *. destruct a; simpl in *.
+econstructor; rewrite PTree.gss; reflexivity.
+destruct (IHG H) as [fs ?].
+change (@ptree_set) with (@PTree.set) in *. destruct a; simpl in *.
+destruct (eq_dec i0 i). econstructor; subst; rewrite PTree.gss; eauto.
+econstructor; rewrite PTree.gso by auto; eauto.
 Qed.
 
 (* there's a place this lemma should be applied, perhaps in proof of semax_call *)
 Lemma funassert_rho:
-  forall G rho rho', ge_of rho = ge_of rho' -> funassert G rho |-- funassert G rho'.
+forall G rho rho', ge_of rho = ge_of rho' -> funassert G rho |-- funassert G rho'.
 Proof. intros. apply funspecs_assert_rho; trivial. Qed.
 (*Lenb: maybe move to seplog?*)
 
 Lemma core_inflate_initial_mem:
-  forall (m: mem) (prog: program) (G: funspecs) (n: nat)
-     (INIT: Genv.init_mem prog = Some m),
-    match_fdecs (prog_funct prog) G ->
-      list_norepet (prog_defs_names prog) ->
-   core (inflate_initial_mem m (initial_core (Genv.globalenv prog) G n)) =
-         initial_core (Genv.globalenv prog) G n.
+forall (m: mem) (prog: program) (G: funspecs) (n: nat)
+ (INIT: Genv.init_mem prog = Some m),
+match_fdecs (prog_funct prog) G ->
+  list_norepet (prog_defs_names prog) ->
+core (inflate_initial_mem m (initial_core (Genv.globalenv prog) G n)) =
+     initial_core (Genv.globalenv prog) G n.
 Proof.
 intros.
 assert (IOK := initial_core_ok _ _ n _ H0 H INIT).
 apply rmap_ext.
-  unfold inflate_initial_mem, initial_core; simpl.
-  rewrite level_core. do 2 rewrite level_make_rmap; auto.
+unfold inflate_initial_mem, initial_core; simpl.
+rewrite level_core. do 2 rewrite level_make_rmap; auto.
 intro l.
 unfold inflate_initial_mem, initial_core; simpl.
 rewrite <- core_resource_at.
@@ -933,36 +949,36 @@ destruct (find_funct_ptr_exists prog id f) as [b [? ?]]; auto.
 apply in_prog_funct_in_prog_defs; auto.
 inversion2 H1 H4.
 + if_tac.
- - destruct (IOK l) as [_ ?].
-   unfold initial_core in H6. rewrite resource_at_make_rmap in H6.
-   unfold initial_core' in H6. rewrite if_true in H6 by auto.
-   apply Genv.find_invert_symbol in H1.
-   unfold fundef in *; rewrite H1 in *.
-   rewrite H2 in *. destruct fs.
-   destruct H6 as [? [? ?]]. rewrite H7.
-   rewrite core_PURE; auto.
- - destruct (access_at m l); try destruct p; try rewrite core_YES; try rewrite core_NO; auto.
+- destruct (IOK l) as [_ ?].
+unfold initial_core in H6. rewrite resource_at_make_rmap in H6.
+unfold initial_core' in H6. rewrite if_true in H6 by auto.
+apply Genv.find_invert_symbol in H1.
+unfold fundef in *; rewrite H1 in *.
+rewrite H2 in *. destruct fs.
+destruct H6 as [? [? ?]]. rewrite H7.
+rewrite core_PURE; auto.
+- destruct (access_at m l); try destruct p; try rewrite core_YES; try rewrite core_NO; auto.
 + (*unfold fundef in *. rewrite H1,H2 in *.*)
-   if_tac;  destruct (access_at m l); try destruct p; try rewrite core_YES; try rewrite core_NO; auto.
+if_tac;  destruct (access_at m l); try destruct p; try rewrite core_YES; try rewrite core_NO; auto.
 + (*unfold fundef in *; rewrite H1 in *.*)
-  if_tac;   destruct (access_at m l); try destruct p; try rewrite core_YES; try rewrite core_NO; auto.
+if_tac;   destruct (access_at m l); try destruct p; try rewrite core_YES; try rewrite core_NO; auto.
 + rewrite ghost_of_core.
-  unfold inflate_initial_mem, initial_core; rewrite !ghost_of_make_rmap, ghost_core; auto.
+unfold inflate_initial_mem, initial_core; rewrite !ghost_of_make_rmap, ghost_core; auto.
 Qed.
 
 Lemma core_inflate_initial_mem':
-  forall (ora : OK_ty) (m: mem) (prog: program) (G: funspecs) (n: nat)
-     (INIT: Genv.init_mem prog = Some m),
-    match_fdecs (prog_funct prog) G ->
-      list_norepet (prog_defs_names prog) ->
-   core (inflate_initial_mem m (initial_core_ext ora (Genv.globalenv prog) G n)) =
-         initial_core (Genv.globalenv prog) G n.
+forall (ora : OK_ty) (m: mem) (prog: program) (G: funspecs) (n: nat)
+ (INIT: Genv.init_mem prog = Some m),
+match_fdecs (prog_funct prog) G ->
+  list_norepet (prog_defs_names prog) ->
+core (inflate_initial_mem m (initial_core_ext ora (Genv.globalenv prog) G n)) =
+     initial_core (Genv.globalenv prog) G n.
 Proof.
 intros.
 assert (IOK := initial_core_ext_ok ora _ _ n _ H0 H INIT).
 apply rmap_ext.
-  unfold inflate_initial_mem, initial_core, initial_core_ext; simpl.
-  rewrite level_core. rewrite !level_make_rmap; auto.
+unfold inflate_initial_mem, initial_core, initial_core_ext; simpl.
+rewrite level_core. rewrite !level_make_rmap; auto.
 intro l.
 unfold inflate_initial_mem, initial_core, initial_core_ext; simpl.
 rewrite <- core_resource_at.
@@ -986,67 +1002,67 @@ destruct (find_funct_ptr_exists prog id f) as [b [? ?]]; auto.
 apply in_prog_funct_in_prog_defs; auto.
 inversion2 H1 H4.
 + if_tac.
-  - destruct (IOK l) as [_ ?].
-   unfold initial_core_ext in H6. rewrite resource_at_make_rmap in H6.
-   unfold initial_core' in H6. rewrite if_true in H6 by auto.
-   apply Genv.find_invert_symbol in H1.
-   unfold fundef in *; rewrite H1 in *.
-   rewrite H2 in *. destruct fs.
-   destruct H6 as [? [? ?]]. rewrite H7.
-   rewrite core_PURE; auto.
-  - destruct (access_at m l); try destruct p; try rewrite core_YES; try rewrite core_NO; auto.
+- destruct (IOK l) as [_ ?].
+unfold initial_core_ext in H6. rewrite resource_at_make_rmap in H6.
+unfold initial_core' in H6. rewrite if_true in H6 by auto.
+apply Genv.find_invert_symbol in H1.
+unfold fundef in *; rewrite H1 in *.
+rewrite H2 in *. destruct fs.
+destruct H6 as [? [? ?]]. rewrite H7.
+rewrite core_PURE; auto.
+- destruct (access_at m l); try destruct p; try rewrite core_YES; try rewrite core_NO; auto.
 + (*unfold fundef in *; rewrite H1,H2 in *.*)
-  if_tac;  destruct (access_at m l); try destruct p; try rewrite core_YES; try rewrite core_NO; auto.
+if_tac;  destruct (access_at m l); try destruct p; try rewrite core_YES; try rewrite core_NO; auto.
 + (*unfold fundef in *; rewrite H1 in *.*)
-  if_tac;   destruct (access_at m l); try destruct p; try rewrite core_YES; try rewrite core_NO; auto.
+if_tac;   destruct (access_at m l); try destruct p; try rewrite core_YES; try rewrite core_NO; auto.
 + rewrite ghost_of_core.
-  unfold inflate_initial_mem, initial_core; rewrite !ghost_of_make_rmap, ghost_core; auto.
+unfold inflate_initial_mem, initial_core; rewrite !ghost_of_make_rmap, ghost_core; auto.
 Qed.
 
 Definition Delta1 V G {C: compspecs}: tycontext :=
-  make_tycontext ((1%positive,(Tfunction Tnil Tvoid cc_default))::nil) nil nil Tvoid V G nil.
+make_tycontext ((1%positive,(Tfunction Tnil Tvoid cc_default))::nil) nil nil Tvoid V G nil.
 
 Lemma match_globvars_in':
-  forall i t vl vs,
-  match_globvars vl vs = true ->
-  In (i,t) vs ->
-  exists g, In (i,g) vl /\ gvar_info g = t.
+forall i t vl vs,
+match_globvars vl vs = true ->
+In (i,t) vs ->
+exists g, In (i,g) vl /\ gvar_info g = t.
 Proof.
- induction vl; destruct vs; intros. inv H0.
- destruct p; inv H.
- inv H0. destruct p, H0. inv H0.  simpl in *.
- destruct a.
- pose proof (eqb_ident_spec i i0); destruct (eqb_ident i i0).
- assert (i=i0) by (rewrite <- H0; auto). subst i0; clear H0.
- apply andb_true_iff in H; destruct H.
- apply eqb_type_true in H. subst t.
- exists g; split3; auto.
- destruct (IHvl _ H) as [g' [? ?]]. left; auto. exists g'; split; auto.
- simpl in H. destruct a.
- pose proof (eqb_ident_spec i0 i1); destruct (eqb_ident i0 i1).
- apply andb_true_iff in H; destruct H.
- destruct (IHvl _ H2) as [g' [? ?]]; auto. exists g'; split; auto.
- right; auto.
- apply IHvl in H. destruct H as [g' [? ?]]. exists g'; split; auto.
- right; auto.
- right; auto.
+induction vl; destruct vs; intros. inv H0.
+destruct p; inv H.
+inv H0. destruct p, H0. inv H0.  simpl in *.
+destruct a.
+pose proof (eqb_ident_spec i i0); destruct (eqb_ident i i0).
+assert (i=i0) by (rewrite <- H0; auto). subst i0; clear H0.
+apply andb_true_iff in H; destruct H.
+apply eqb_type_true in H. subst t.
+exists g; split3; auto.
+destruct (IHvl _ H) as [g' [? ?]]. left; auto. exists g'; split; auto.
+simpl in H. destruct a.
+pose proof (eqb_ident_spec i0 i1); destruct (eqb_ident i0 i1).
+apply andb_true_iff in H; destruct H.
+destruct (IHvl _ H2) as [g' [? ?]]; auto. exists g'; split; auto.
+right; auto.
+apply IHvl in H. destruct H as [g' [? ?]]. exists g'; split; auto.
+right; auto.
+right; auto.
 Qed.
 
 Lemma match_globvars_in:
-  forall i vl vs, match_globvars vl vs = true -> In i  (map (@fst _ _) vs) -> In i (map (@fst _ _) vl).
+forall i vl vs, match_globvars vl vs = true -> In i  (map (@fst _ _) vs) -> In i (map (@fst _ _) vl).
 Proof.
- intros.
- apply list_in_map_inv in H0. destruct H0 as [t [? ?]]. subst i.
- destruct t as [i t].
- destruct  (match_globvars_in' _ _ _ _ H H1) as [g [? ?]].
- simpl. apply in_map_fst with g; auto.
+intros.
+apply list_in_map_inv in H0. destruct H0 as [t [? ?]]. subst i.
+destruct t as [i t].
+destruct  (match_globvars_in' _ _ _ _ H H1) as [g [? ?]].
+simpl. apply in_map_fst with g; auto.
 Qed.
 
 Lemma match_globvars_norepet:
-  forall vl vs,
-   list_norepet (map (@fst _ _) vl) ->
-   match_globvars vl vs = true ->
-   list_norepet (map (@fst _ _) vs).
+forall vl vs,
+list_norepet (map (@fst _ _) vl) ->
+match_globvars vl vs = true ->
+list_norepet (map (@fst _ _) vs).
 Proof.
 induction vl; destruct vs; simpl; intros.
 constructor. destruct p. inv H0.
@@ -1054,134 +1070,134 @@ constructor.
 destruct p; destruct a.
 simpl in *.
 inv H.
- pose proof (eqb_ident_spec i i0); destruct (eqb_ident i i0).
- assert (i=i0) by (apply H; auto); subst i0; clear H.
- apply andb_true_iff in H0; destruct H0.
- constructor; auto.
- contradict H3.
- eapply match_globvars_in; eauto.
- assert (i<>i0). intro; subst; destruct H. specialize (H1 (eq_refl _)); inv H1.
- clear H.
- specialize (IHvl ((i,t)::vs) H4 H0).
- inv IHvl.
- constructor; auto.
+pose proof (eqb_ident_spec i i0); destruct (eqb_ident i i0).
+assert (i=i0) by (apply H; auto); subst i0; clear H.
+apply andb_true_iff in H0; destruct H0.
+constructor; auto.
+contradict H3.
+eapply match_globvars_in; eauto.
+assert (i<>i0). intro; subst; destruct H. specialize (H1 (eq_refl _)); inv H1.
+clear H.
+specialize (IHvl ((i,t)::vs) H4 H0).
+inv IHvl.
+constructor; auto.
 Qed.
 
 Lemma make_tycontext_g_denote:
-  forall id t l vs G,
-    list_norepet (map fst l) ->
-    match_globvars (prog_vars' l) vs = true ->
-    match_fdecs (prog_funct' l) G ->
-   ((make_tycontext_g vs G) ! id = Some t <->
-    ((exists f, In (id,f) G /\ t = type_of_funspec f) \/ In (id,t) vs)).
+forall id t l vs G,
+list_norepet (map fst l) ->
+match_globvars (prog_vars' l) vs = true ->
+match_fdecs (prog_funct' l) G ->
+((make_tycontext_g vs G) ! id = Some t <->
+((exists f, In (id,f) G /\ t = type_of_funspec f) \/ In (id,t) vs)).
 Proof.
-  intros.
-  assert (list_norepet (map (@fst _ _) (prog_funct' l) ++  (map (@fst _ _) (prog_vars' l)))). {
-   clear - H.
-  induction l; simpl. constructor.
-  destruct a; destruct g; simpl in *; inv H.
-  constructor; auto.
-  clear - H2; contradict H2.
-   induction l. inv H2. destruct a; destruct g; simpl in *. destruct H2; auto.
-   apply in_app in H2. destruct H2. right; apply IHl. apply in_app; auto.
-   destruct H; auto. right; apply IHl; apply in_app; auto.
-   specialize (IHl H3).
-   apply list_norepet_app in IHl. destruct IHl as [? [? ?]].
-   apply list_norepet_app; split3; auto.
-   constructor; auto.
-  clear - H2; contradict H2.
-   induction l. inv H2. destruct a; destruct g. simpl in H2. constructor 2; auto.
-   simpl in H2. destruct H2. subst; left; auto. right. auto.
-  apply list_disjoint_cons_r; auto.
-  clear - H2; contradict H2.
-   induction l. inv H2. destruct a; destruct g. simpl in H2.
-  destruct H2. subst; left; auto. right; auto.
-  simpl in *. right; auto.
+intros.
+assert (list_norepet (map (@fst _ _) (prog_funct' l) ++  (map (@fst _ _) (prog_vars' l)))). {
+clear - H.
+induction l; simpl. constructor.
+destruct a; destruct g; simpl in *; inv H.
+constructor; auto.
+clear - H2; contradict H2.
+induction l. inv H2. destruct a; destruct g; simpl in *. destruct H2; auto.
+apply in_app in H2. destruct H2. right; apply IHl. apply in_app; auto.
+destruct H; auto. right; apply IHl; apply in_app; auto.
+specialize (IHl H3).
+apply list_norepet_app in IHl. destruct IHl as [? [? ?]].
+apply list_norepet_app; split3; auto.
+constructor; auto.
+clear - H2; contradict H2.
+induction l. inv H2. destruct a; destruct g. simpl in H2. constructor 2; auto.
+simpl in H2. destruct H2. subst; left; auto. right. auto.
+apply list_disjoint_cons_r; auto.
+clear - H2; contradict H2.
+induction l. inv H2. destruct a; destruct g. simpl in H2.
+destruct H2. subst; left; auto. right; auto.
+simpl in *. right; auto.
 }
- forget (prog_vars' l) as vl.
- forget (prog_funct' l) as fl.
- clear l H.
- revert G H2 H1; induction fl; intros.
+forget (prog_vars' l) as vl.
+forget (prog_funct' l) as fl.
+clear l H.
+revert G H2 H1; induction fl; intros.
 * (* fl = nil *)
- destruct G; inv H1.
- simpl in H2.
- apply iff_trans with (In (id, t) vs );
-  [ | clear; intuition; destruct H0 as [? [? ?]]; contradiction].
- revert vs H0; induction vl; destruct vs; simpl in *; intros.
+destruct G; inv H1.
+simpl in H2.
+apply iff_trans with (In (id, t) vs );
+[ | clear; intuition; destruct H0 as [? [? ?]]; contradiction].
+revert vs H0; induction vl; destruct vs; simpl in *; intros.
 +(* fl = nil /\ vl = nil /\ vs = nil*)
- rewrite PTree.gempty.
- split; intros. discriminate. contradiction.
+rewrite PTree.gempty.
+split; intros. discriminate. contradiction.
 + (* fl = nil /\ vl = nil /\ vs<>nil *)
- clear H2.
- destruct p. inv H0.
+clear H2.
+destruct p. inv H0.
 + (* fl = nil /\ vl inductive case /\ vs = nil  *)
- clear H0. rewrite PTree.gempty.
-   clear. intuition congruence.
- + (* fl = nil /\ vl inductive case /\ vs <> nil *)
-   destruct p. destruct a. simpl in *. inv H2.
-  specialize (IHvl H4).
-  destruct (ident_eq id i).
- - subst id.
-  rewrite PTree.gss. split; intro. inv H.
-  auto.
- destruct H. inv H. auto.
- pose proof (eqb_ident_spec i i0); destruct (eqb_ident i i0).
- assert (i=i0) by (rewrite <- H1; auto). subst i0; clear H1.
-  apply andb_true_iff in H0; destruct H0.
- contradiction H3.
- eapply match_globvars_in; eauto. apply in_map_fst with t. auto.
- assert (i<>i0). intro; subst. clear - H1. destruct H1. specialize (H0 (eq_refl _)); inv H0.
- clear H1.
- pose proof (match_globvars_norepet _ _ H4 H0).
- inv H1. contradiction H7. apply in_map_fst with t; auto.
- - (* id <> i *)
- rewrite PTree.gso by auto.
- pose proof (eqb_ident_spec i i0).
- destruct (ident_eq i i0).
- subst. destruct H. rewrite H1 in H0 by auto.
- rewrite andb_true_iff in H0; destruct H0.
- apply eqb_type_true in H0. subst t0.
- clear H H1.
- rewrite IHvl; auto.
- clear - n; intuition. inv H0; congruence.
- destruct (eqb_ident i i0). contradict n0; apply H; auto.
- eapply iff_trans; [ | apply (IHvl ((i,t0)::vs))]; clear IHvl.
- simpl;  rewrite PTree.gso by auto. apply iff_refl.
- auto.
+clear H0. rewrite PTree.gempty.
+clear. intuition congruence.
++ (* fl = nil /\ vl inductive case /\ vs <> nil *)
+destruct p. destruct a. simpl in *. inv H2.
+specialize (IHvl H4).
+destruct (ident_eq id i).
+- subst id.
+rewrite PTree.gss. split; intro. inv H.
+auto.
+destruct H. inv H. auto.
+pose proof (eqb_ident_spec i i0); destruct (eqb_ident i i0).
+assert (i=i0) by (rewrite <- H1; auto). subst i0; clear H1.
+apply andb_true_iff in H0; destruct H0.
+contradiction H3.
+eapply match_globvars_in; eauto. apply in_map_fst with t. auto.
+assert (i<>i0). intro; subst. clear - H1. destruct H1. specialize (H0 (eq_refl _)); inv H0.
+clear H1.
+pose proof (match_globvars_norepet _ _ H4 H0).
+inv H1. contradiction H7. apply in_map_fst with t; auto.
+- (* id <> i *)
+rewrite PTree.gso by auto.
+pose proof (eqb_ident_spec i i0).
+destruct (ident_eq i i0).
+subst. destruct H. rewrite H1 in H0 by auto.
+rewrite andb_true_iff in H0; destruct H0.
+apply eqb_type_true in H0. subst t0.
+clear H H1.
+rewrite IHvl; auto.
+clear - n; intuition. inv H0; congruence.
+destruct (eqb_ident i i0). contradict n0; apply H; auto.
+eapply iff_trans; [ | apply (IHvl ((i,t0)::vs))]; clear IHvl.
+simpl;  rewrite PTree.gso by auto. apply iff_refl.
+auto.
 *
- inv H1.
- +
-   inv H2.
-   specialize (IHfl _ H5 H6).
-   destruct (ident_eq id i). subst.
-  simpl; rewrite PTree.gss.
-  split; intro.
-  left; exists fspec.  inv H; auto.
-  f_equal.
-  destruct H as [[f [? ?]]| ?].
-  destruct H. inv H. auto.
-  elimtype False; clear - H3 H H6.
-  apply H3; apply in_app_iff. left; eapply match_fdecs_in; eauto.
-  apply in_map_fst in H; auto.
-  contradiction H3. apply in_app_iff; right.
-  subst.
-  eapply match_globvars_in; eauto.
-  apply in_map_fst in H; auto.
-  simpl; rewrite PTree.gso; auto.
-  rewrite IHfl. clear IHfl.
-  split; intros [[f [? ?]]| ?]; subst.
-  left; eauto. right; eauto.
-  left; eauto. destruct H. congruence.
-  exists f; eauto.
-  right; eauto.
+inv H1.
++
+inv H2.
+specialize (IHfl _ H5 H6).
+destruct (ident_eq id i). subst.
+simpl; rewrite PTree.gss.
+split; intro.
+left; exists fspec.  inv H; auto.
+f_equal.
+destruct H as [[f [? ?]]| ?].
+destruct H. inv H. auto.
+elimtype False; clear - H3 H H6.
+apply H3; apply in_app_iff. left; eapply match_fdecs_in; eauto.
+apply in_map_fst in H; auto.
+contradiction H3. apply in_app_iff; right.
+subst.
+eapply match_globvars_in; eauto.
+apply in_map_fst in H; auto.
+simpl; rewrite PTree.gso; auto.
+rewrite IHfl. clear IHfl.
+split; intros [[f [? ?]]| ?]; subst.
+left; eauto. right; eauto.
+left; eauto. destruct H. congruence.
+exists f; eauto.
+right; eauto.
 (*+
-  simpl in H2; inv H2.
-  apply (IHfl G); auto.
+simpl in H2; inv H2.
+apply (IHfl G); auto.
 *)
 Qed.
 
 Lemma tc_ge_denote_initial:
-  forall vs G (prog: program),
+forall vs G (prog: program),
 list_norepet (prog_defs_names prog) ->
 match_globvars (prog_vars prog) vs = true->
 match_fdecs (prog_funct prog) G ->
@@ -1211,23 +1227,23 @@ apply IHl; auto.
 destruct (find_funct_ptr_exists prog id fd) as [b [? ?]]; auto.
 exists b; auto.
 *
- unfold filter_genv.
- destruct (match_globvars_in' _ _ _ _ H0 H2) as [g [? ?]].
- apply in_prog_vars_in_prog_defs in H3.
- pose proof (prog_defmap_norepet _ _ _ H H3).
+unfold filter_genv.
+destruct (match_globvars_in' _ _ _ _ H0 H2) as [g [? ?]].
+apply in_prog_vars_in_prog_defs in H3.
+pose proof (prog_defmap_norepet _ _ _ H H3).
 destruct (proj1 (Genv.find_def_symbol _ _ _) H5)
-  as [b [? ?]].
- exists b; auto.
+as [b [? ?]].
+exists b; auto.
 Qed.
 
 Lemma semax_prog_typecheck_aux:
-  forall vs G {C: compspecs} (prog: program) b,
-   list_norepet (prog_defs_names prog) ->
-   match_globvars (prog_vars prog) vs = true ->
-   match_fdecs (prog_funct prog) G ->
-   typecheck_environ
-      (Delta1 vs G) (construct_rho (filter_genv (globalenv prog)) empty_env
-        (PTree.set 1 (Vptr b Ptrofs.zero) (PTree.empty val))) .
+forall vs G {C: compspecs} (prog: program) b,
+list_norepet (prog_defs_names prog) ->
+match_globvars (prog_vars prog) vs = true ->
+match_fdecs (prog_funct prog) G ->
+typecheck_environ
+  (Delta1 vs G) (construct_rho (filter_genv (globalenv prog)) empty_env
+    (PTree.set 1 (Vptr b Ptrofs.zero) (PTree.empty val))) .
 Proof.
 unfold Delta1; intros.
 unfold construct_rho.
@@ -1261,655 +1277,677 @@ Qed.
 
 Lemma in_map_sig {A B} (E:forall b b' : B, {b=b'}+{b<>b'}) y (f : A -> B) l : In y (map f l) -> {x : A | f x = y /\ In x l }.
 Proof.
-  induction l; intros HI.
-  - inversion HI.
-  - simpl in HI.
-    destruct (E (f a) y).
-    + exists a; intuition.
-    + destruct IHl. tauto. exists x; intuition.
+induction l; intros HI.
+- inversion HI.
+- simpl in HI.
+destruct (E (f a) y).
++ exists a; intuition.
++ destruct IHl. tauto. exists x; intuition.
 Qed.
 
 Lemma find_symbol_funct_ptr_ex_sig V ge id f :
-  (exists b : block,
-      Genv.find_symbol ge id = Some b /\
-      Genv.find_funct_ptr ge b = Some f) ->
-  {b : block |
-   Genv.find_symbol ge id = Some b /\
-   @Genv.find_funct_ptr (Ctypes.fundef function) V ge b = Some f}.
+(exists b : block,
+  Genv.find_symbol ge id = Some b /\
+  Genv.find_funct_ptr ge b = Some f) ->
+{b : block |
+Genv.find_symbol ge id = Some b /\
+@Genv.find_funct_ptr (Ctypes.fundef function) V ge b = Some f}.
 Proof.
-  intros Ex.
-  apply (decidable_countable_ex_sig Pos.of_nat); auto.
-  now intro; eexists; symmetry; apply Pos2Nat.id.
-  intros p.
-  assert (group : forall {A} {B} (a a':A) (b b':B), (a = a' /\ b = b') <-> ((a, b) = (a', b')))
-    by (intros;split; [ intros [<- <-]; reflexivity | intros E; injection E; auto]).
-  assert (sumbool_iff_left : forall (A A' B : Prop), (A -> A') -> {A}+{B} -> {A'}+{B}) by tauto.
-  assert (sumbool_iff_right : forall (A B B' : Prop), (B -> B') -> {A}+{B} -> {A}+{B'}) by tauto.
-  eapply sumbool_iff_left. apply group.
-  eapply sumbool_iff_right. rewrite group. apply (fun x => x).
-  pose proof type_eq.
-  pose proof eq_dec_statement.
-  repeat (hnf; decide equality; auto).
+intros Ex.
+apply (decidable_countable_ex_sig Pos.of_nat); auto.
+now intro; eexists; symmetry; apply Pos2Nat.id.
+intros p.
+assert (group : forall {A} {B} (a a':A) (b b':B), (a = a' /\ b = b') <-> ((a, b) = (a', b')))
+by (intros;split; [ intros [<- <-]; reflexivity | intros E; injection E; auto]).
+assert (sumbool_iff_left : forall (A A' B : Prop), (A -> A') -> {A}+{B} -> {A'}+{B}) by tauto.
+assert (sumbool_iff_right : forall (A B B' : Prop), (B -> B') -> {A}+{B} -> {A}+{B'}) by tauto.
+eapply sumbool_iff_left. apply group.
+eapply sumbool_iff_right. rewrite group. apply (fun x => x).
+pose proof type_eq.
+pose proof eq_dec_statement.
+repeat (hnf; decide equality; auto).
 Qed.
 
 Lemma initial_jm_funassert V (prog : Clight.program) m G n H H1 H2 :
-  (funassert (nofunc_tycontext V G) (empty_environ (globalenv prog)))
-    (m_phi (initial_jm prog m G n H H1 H2)).
+(funassert (nofunc_tycontext V G) (empty_environ (globalenv prog)))
+(m_phi (initial_jm prog m G n H H1 H2)).
 Proof.
-  unfold initial_jm.
-  assert (FA: app_pred (funassert (nofunc_tycontext V G) (empty_environ (globalenv prog)))
-    (initial_world.initial_core (Genv.globalenv prog) G n)
-         ).
-  apply funassert_initial_core; auto.
-  revert FA.
-  pose proof corable_funassert (nofunc_tycontext V G) (empty_environ (globalenv prog)) as CO.
-  rewrite corable_spec in CO. apply CO.
-  pose proof initial_mem_core as E.
-  unfold juicy_mem_core in *. erewrite E; try reflexivity.
+unfold initial_jm.
+assert (FA: app_pred (funassert (nofunc_tycontext V G) (empty_environ (globalenv prog)))
+(initial_world.initial_core (Genv.globalenv prog) G n)
+     ).
+apply funassert_initial_core; auto.
+revert FA.
+pose proof corable_funassert (nofunc_tycontext V G) (empty_environ (globalenv prog)) as CO.
+rewrite corable_spec in CO. apply CO.
+pose proof initial_mem_core as E.
+unfold juicy_mem_core in *. erewrite E; try reflexivity.
 Qed.
 
 Lemma initial_jm_ext_funassert (ora : OK_ty) V (prog : Clight.program) m G n H H1 H2 :
-  (funassert (nofunc_tycontext V G) (empty_environ (globalenv prog)))
-    (m_phi (initial_jm_ext ora prog m G n H H1 H2)).
+(funassert (nofunc_tycontext V G) (empty_environ (globalenv prog)))
+(m_phi (initial_jm_ext ora prog m G n H H1 H2)).
 Proof.
-  unfold initial_jm_ext.
-  assert (FA: app_pred (funassert (nofunc_tycontext V G) (empty_environ (globalenv prog)))
-    (initial_world.initial_core_ext ora (Genv.globalenv prog) G n)
-         ).
-  apply funassert_initial_core_ext; auto.
-  revert FA. 
-  pose proof corable_funassert (nofunc_tycontext V G) (empty_environ (globalenv prog)) as CO.
-  rewrite corable_spec in CO. apply CO.
-  pose proof initial_mem_core as E.
-  unfold juicy_mem_core in *. erewrite E; try reflexivity.
+unfold initial_jm_ext.
+assert (FA: app_pred (funassert (nofunc_tycontext V G) (empty_environ (globalenv prog)))
+(initial_world.initial_core_ext ora (Genv.globalenv prog) G n)
+     ).
+apply funassert_initial_core_ext; auto.
+revert FA. 
+pose proof corable_funassert (nofunc_tycontext V G) (empty_environ (globalenv prog)) as CO.
+rewrite corable_spec in CO. apply CO.
+pose proof initial_mem_core as E.
+unfold juicy_mem_core in *. erewrite E; try reflexivity.
 Qed.
 
 Lemma semax_prog_rule' {CS: compspecs} :
-  forall V G prog m h,
-     @semax_prog CS prog V G ->
-     Genv.init_mem prog = Some m ->
-     { b : block & { q : corestate &
-       (Genv.find_symbol (globalenv prog) (prog_main prog) = Some b) *
-       (forall jm, m_dry jm = m -> exists jm', semantics.initial_core (juicy_core_sem (cl_core_sem (globalenv prog))) h
-                    jm q jm' (Vptr b Ptrofs.zero) nil) *
-       forall n z,
-         { jm |
-           m_dry jm = m /\ level jm = n /\
-           nth_error (ghost_of (m_phi jm)) 0 = Some (Some (ext_ghost z, NoneP)) /\
-           jsafeN (@OK_spec Espec) (globalenv prog) n z q jm /\
-           no_locks (m_phi jm) /\
-           matchfunspecs (globalenv prog) G (m_phi jm) /\
-           (funassert (nofunc_tycontext V G) (empty_environ (globalenv prog))) (m_phi jm)
-     } } }%type.
+forall V G prog m h,
+ @semax_prog CS prog V G ->
+ Genv.init_mem prog = Some m ->
+ { b : block & { q : corestate &
+   (Genv.find_symbol (globalenv prog) (prog_main prog) = Some b) *
+   (forall jm, m_dry jm = m -> exists jm', semantics.initial_core (juicy_core_sem (cl_core_sem (globalenv prog))) h
+                jm q jm' (Vptr b Ptrofs.zero) nil) *
+   forall n z,
+     { jm |
+       m_dry jm = m /\ level jm = n /\
+       nth_error (ghost_of (m_phi jm)) 0 = Some (Some (ext_ghost z, NoneP)) /\
+       jsafeN (@OK_spec Espec) (globalenv prog) n z q jm /\
+       no_locks (m_phi jm) /\
+       matchfunspecs (globalenv prog) G (m_phi jm) /\
+       (funassert (nofunc_tycontext V G) (empty_environ (globalenv prog))) (m_phi jm)
+ } } }%type.
 Proof.
-  intros until m.
-  pose proof I; intros.
-  destruct H0 as [? [AL [HGG [[? ?] [GV ?]]]]].
-  assert (CSUBmain: cenv_sub  (@cenv_cs CS) (@prog_comp_env function prog)).
-  { rewrite HGG; apply cenv_sub_refl. }
-  destruct (find_id (prog_main prog) G) as [fspec|] eqn:Hfind; try contradiction.
-  assert (H4': exists post, In (prog_main prog, main_spec' prog post) G /\ fspec = main_spec' prog post). {
-    destruct (find_id (prog_main prog) G) eqn:?.
-    apply find_id_e in Heqo. destruct H4 as [post ?]. exists post.
-    subst. split; auto. inv Hfind. auto. inv Hfind.
-  } clear H4. rename H4' into H4.
-  assert ({ f | In (prog_main prog, f) (prog_funct prog)}).
-  forget (prog_main prog) as id.
-  assert (H4': In id (map fst G)). {
-  destruct H4 as [? [H4 _]].
-  apply in_map_fst in H4. auto.
-  }
-  pose proof (match_fdecs_in _ _ _ H4' H2).
-  apply in_map_sig in H5. 2:decide equality.
-  destruct H5 as [[? ?] [? ?]]; subst.
-  eauto.
-  destruct H5 as [f ?].
-  apply compute_list_norepet_e in H0.
-  assert (indefs: In (prog_main prog, Gfun f) (AST.prog_defs prog))
-    by (apply in_prog_funct_in_prog_defs; auto).
-  pose proof (find_funct_ptr_exists prog (prog_main prog) f) as EXx.
-  (* Genv.find_funct_ptr_exists is a Prop existential, we use constructive epsilon and
-     decidability on a countable set to transform it to a Type existential *)
-  apply find_symbol_funct_ptr_ex_sig in EXx; auto.
+intros until m.
+pose proof I; intros.
+destruct H0 as [? [AL [HGG [[? [Gcontains ?]] [GV ?]]]]].
+assert (CSUBmain: cenv_sub  (@cenv_cs CS) (@prog_comp_env function prog)).
+{ rewrite HGG; apply cenv_sub_refl. }
+destruct (find_id (prog_main prog) G) as [fspec|] eqn:Hfind; try contradiction.
+assert (H4': exists post, In (prog_main prog, main_spec' prog post) G /\ fspec = main_spec' prog post). {
+destruct (find_id (prog_main prog) G) eqn:?.
+apply find_id_e in Heqo. destruct H4 as [post ?]. exists post.
+subst. split; auto. inv Hfind. auto. inv Hfind.
+} clear H4. rename H4' into H4.
+assert ({ f | In (prog_main prog, f) (prog_funct prog)}).
+forget (prog_main prog) as id.
+assert (H4': In id (map fst G)). {
+destruct H4 as [? [H4 _]].
+apply in_map_fst in H4. auto.
+}
+pose proof (match_fdecs_in _ _ _ H4' H2).
+apply in_map_sig in H5. 2:decide equality.
+destruct H5 as [[? ?] [? ?]]; subst.
+eauto.
+destruct H5 as [f ?].
+apply compute_list_norepet_e in H0.
+assert (indefs: In (prog_main prog, Gfun f) (AST.prog_defs prog))
+by (apply in_prog_funct_in_prog_defs; auto).
+pose proof (find_funct_ptr_exists prog (prog_main prog) f) as EXx.
+(* Genv.find_funct_ptr_exists is a Prop existential, we use constructive epsilon and
+ decidability on a countable set to transform it to a Type existential *)
+apply find_symbol_funct_ptr_ex_sig in EXx; auto.
 
-  pose proof I.
-  destruct EXx as [b [? ?]]; auto.
-  assert (E: type_of_fundef f = Tfunction Tnil tint cc_default). {
-     destruct H4 as [post [? ?]].
-      destruct (match_fdecs_exists_Gfun
-                  prog G (prog_main prog)
-                  (main_spec' prog post))
-        as (fd, (Ifd, sametypes)); auto.
-      {
-        apply find_id_i; auto.
-        eapply match_fdecs_norepet; eauto.
-        clear -H0; revert H0.
-        apply sublist_norepet.
-        unfold prog_funct, prog_funct', prog_defs_names.
-        replace (AST.prog_defs prog) with (prog_defs prog) by reflexivity.
-        generalize (prog_defs prog); intros l; induction l as [|(i,[g|]) l];
-          constructor; auto.
-      }
-      assert (fd = f).
-      cut (Gfun fd = @Gfun _ type f); [ intros E; injection E; auto | ].
-      apply (list_norepet_In_In (prog_main prog) _ _ (prog_defs prog)); auto.
-      subst fd.
-      auto.
-    }
-  exists b.
-  unfold semantics.initial_core, juicy_core_sem.
-  unfold j_initial_core, semantics.initial_core, cl_core_sem, cl_initial_core.
-  eexists.
-  unfold fundef in *.
-  change (Genv.globalenv prog) with (genv_genv (globalenv prog)) in *.
-  rewrite H6, H7.
-  rewrite if_true by auto.
-  repeat split; eauto.
+pose proof I.
+destruct EXx as [b [? ?]]; auto.
+assert (E: type_of_fundef f = Tfunction Tnil tint cc_default). {
+ destruct H4 as [post [? ?]].
+  destruct (match_fdecs_exists_Gfun
+              prog G (prog_main prog)
+              (main_spec' prog post))
+    as (fd, (Ifd, sametypes)); auto.
   {
-    intros. eexists; split. reflexivity.
-    rewrite E.  
-    repeat split; eauto; try solve [constructor].
+    apply find_id_i; auto.
+    eapply match_fdecs_norepet; eauto.
+    clear -H0; revert H0.
+    apply sublist_norepet.
+    unfold prog_funct, prog_funct', prog_defs_names.
+    replace (AST.prog_defs prog) with (prog_defs prog) by reflexivity.
+    generalize (prog_defs prog); intros l; induction l as [|(i,[g|]) l];
+      constructor; auto.
   }
-  intros n z.
-  exists (initial_jm_ext z _ _ _ n H1 H0 H2).
-  repeat split.
-  - simpl.
-    rewrite inflate_initial_mem_level.
-    unfold initial_core_ext. rewrite level_make_rmap; auto.
+  assert (fd = f).
+  cut (Gfun fd = @Gfun _ type f); [ intros E; injection E; auto | ].
+  apply (list_norepet_In_In (prog_main prog) _ _ (prog_defs prog)); auto.
+  subst fd.
+  auto.
+}
+exists b.
+unfold semantics.initial_core, juicy_core_sem.
+unfold j_initial_core, semantics.initial_core, cl_core_sem, cl_initial_core.
+eexists.
+unfold fundef in *.
+change (Genv.globalenv prog) with (genv_genv (globalenv prog)) in *.
+rewrite H6, H7.
+rewrite if_true by auto.
+repeat split; eauto.
+{
+intros. eexists; split. reflexivity.
+rewrite E.  
+repeat split; eauto; try solve [constructor].
+}
+intros n z.
+exists (initial_jm_ext z _ _ _ n H1 H0 H2).
+repeat split.
+- simpl.
+rewrite inflate_initial_mem_level.
+unfold initial_core_ext. rewrite level_make_rmap; auto.
 
-  - unfold initial_jm_ext; simpl.
+- unfold initial_jm_ext; simpl.
+unfold inflate_initial_mem; rewrite ghost_of_make_rmap.
+unfold initial_core_ext; rewrite ghost_of_make_rmap.
+reflexivity.
+
+- specialize (H3 (globalenv prog)).
+spec H3; [ intros; apply sub_option_refl |].
+spec H3; [ intros; apply sub_option_refl |]. 
+destruct H4 as [post [? ?]].
+unfold temp_bindings. simpl length. simpl typed_params. simpl type_of_params.
+pattern n at 1; replace n with (level (m_phi (initial_jm_ext z prog m G n H1 H0 H2))).
+pose (rho1 := mkEnviron (filter_genv (globalenv prog)) (Map.empty (block * type))
+                       (Map.set 1 (Vptr b Ptrofs.zero) (Map.empty val))).
+pose (post' := fun rho => TT * EX rv:val, post nil (globals_of_env rho1) (env_set (globals_only rho) ret_temp rv)).
+eapply (semax_call_aux (Delta1 V G) (ConstType (ident->val))
+          _ post _ (const_super_non_expansive _ _) (const_super_non_expansive _ _)
+          nil (globals_of_env rho1) (fun _ => TT) (fun _ => TT)
+          None (nil, tint) cc_default _ _ (normal_ret_assert post') _ _ _ _
+          (construct_rho (filter_genv (globalenv prog)) empty_env
+             (PTree.set 1 (Vptr b Ptrofs.zero) (PTree.empty val)))
+          _ _ b (prog_main prog));
+  try apply H3; try eassumption; auto.
++ simpl.
     unfold inflate_initial_mem; rewrite ghost_of_make_rmap.
     unfold initial_core_ext; rewrite ghost_of_make_rmap.
-    reflexivity.
-
-  - specialize (H3 (globalenv prog) (prog_contains_prog_funct _ H0)).
-    destruct H4 as [post [? ?]].
-    unfold temp_bindings. simpl length. simpl typed_params. simpl type_of_params.
-    pattern n at 1; replace n with (level (m_phi (initial_jm_ext z prog m G n H1 H0 H2))).
-    pose (rho1 := mkEnviron (filter_genv (globalenv prog)) (Map.empty (block * type))
-                           (Map.set 1 (Vptr b Ptrofs.zero) (Map.empty val))).
-    pose (post' := fun rho => TT * EX rv:val, post nil (globals_of_env rho1) (env_set (globals_only rho) ret_temp rv)).
-    eapply (semax_call_aux (Delta1 V G) (ConstType (ident->val))
-              _ post _ (const_super_non_expansive _ _) (const_super_non_expansive _ _)
-              nil (globals_of_env rho1) (fun _ => TT) (fun _ => TT)
-              None (nil, tint) cc_default _ _ (normal_ret_assert post') _ _ _ _
-              (construct_rho (filter_genv (globalenv prog)) empty_env
-                 (PTree.set 1 (Vptr b Ptrofs.zero) (PTree.empty val)))
-              _ _ b (prog_main prog));
-      try apply H3; try eassumption; auto.
-    + simpl.
-        unfold inflate_initial_mem; rewrite ghost_of_make_rmap.
-        unfold initial_core_ext; rewrite ghost_of_make_rmap.
-        exists (Some (ext_both z, NoneP) :: nil); repeat constructor.
-    + simpl.
-      exists (Vptr b Ptrofs.zero).
-      split; auto.
-    + simpl snd.
-      replace (params_of_fundef f) with (@nil type). simpl; auto. clear -E.
-      destruct f as [[? ? [ | [] ]] | e [|] ? c] ; compute in *; congruence.
-    + clear - GV H2 H0.
-      split.
-      eapply semax_prog_typecheck_aux; eauto.
-      simpl.
-      auto.
-    + hnf; intros; intuition.
-    + (*hnf; intros; intuition.
-      unfold normal_ret_assert; simpl.
-      extensionality rho'.
-      normalize.
-      unfold post'.
-      apply pred_ext.
-           normalize. intro rv. do 2 apply exp_right with rv; auto.
-           normalize. intro rv. apply exp_right with rv; auto. *)
-      intros rho' u U y UY k YK K.
-      unfold normal_ret_assert; simpl.
-      destruct K as [v [a1 [a2 [J [A1 [w A2]]]]]]. exists a1, a2; intuition. exists w; trivial.
-    + rewrite (corable_funassert _ _).
-      simpl m_phi.
-      rewrite core_inflate_initial_mem'; auto.
-      do 3 (pose proof I).
-      replace (funassert (Delta1 V G)) with
-      (funassert (@nofunc_tycontext V G)).
-      unfold rho1; apply funassert_initial_core; auto.
-      apply same_glob_funassert.
-      reflexivity.
-    + apply now_later.
-      intros ek vl tx' vx'.
-      cbv zeta. rewrite proj_frame_ret_assert. simpl seplog.sepcon.
-      subst post'. cbv beta.
-      destruct ek; simpl proj_ret_assert; normalize.
-      apply derives_subp.
-      normalize. intro rv.
-      simpl.
-      eapply derives_trans, own.bupd_intro.
-      intros ? ? ? ? Hora _ ?.
-      destruct H9 as [[? [H10' [H11 ?]]] ?].
-      hnf in H10', H11.
-      destruct H9.
-      subst a.
-      change Clight_new.true_expr with true_expr.
-      change (level (m_phi jm)) with (level jm).
-      apply safe_loop_skip.
-    + unfold glob_types, Delta1. simpl @snd.
-      forget (prog_main prog) as main.
-      instantiate (1:= post).
-      instantiate (1:= main_pre prog).
-      assert (H8': list_norepet (map (@fst _ _) (prog_funct prog))). {
-      clear - H0.
-      unfold prog_defs_names in H0. unfold prog_funct.
-      change (AST.prog_defs prog) with (prog_defs prog) in H0.
-      induction (prog_defs prog); auto. inv H0.
-      destruct a; destruct g; simpl; auto. constructor; auto.
-      clear - H2; simpl in H2; contradict H2; induction l; simpl in *; auto.
-      destruct a; destruct g; simpl in *; auto. destruct H2; auto.
-      }
-      forget (prog_funct prog) as fs.
-      clear - H4 H8' H2. rename H8' into H8.
-      fold (main_spec prog).
-      forget (main_spec prog) as fd.
-      revert G H2 H4 H8; induction fs; intros; inv H2.
-      contradiction H4.
-      simpl in *.
-      destruct (ident_eq i main). subst. rewrite PTree.gss.
-      destruct H4. inv H; auto.
-      inv H8.
-      contradiction H3.
-      eapply match_fdecs_in; eauto.
-      apply in_map_fst in H; auto.
-      rewrite PTree.gso by auto.
-      destruct H4; try congruence.
-      inv H8.
-      eapply IHfs; eauto.
-    + intros.
-      intros ? ?.
-      split; apply derives_imp; auto.
-    + unfold main_pre.
-      apply now_later.
-      rewrite TT_sepcon_TT.
-      rewrite sepcon_comm.
-      eexists; eexists; split; [apply initial_jm_ext_eq|].
-      split; auto.
-     match goal with |- app_pred (globvars2pred (globals_of_env ?A) _ ?B) _ => 
-       change (globals_of_env A) with (globals_of_env B)
-      end.
-      apply global_initializers; auto.
-    + simpl.
-      rewrite inflate_initial_mem_level.
-      unfold initial_core.
-      apply level_make_rmap.
-  - apply initial_jm_ext_without_locks.
-  - apply initial_jm_ext_matchfunspecs. 
-  -  destruct (initial_jm_ext_funassert z V prog m G n H1 H0 H2). auto.
-  -  destruct (initial_jm_ext_funassert z V prog m G n H1 H0 H2). auto.
+    exists (Some (ext_both z, NoneP) :: nil); repeat constructor.
++ simpl.
+  exists (Vptr b Ptrofs.zero).
+  split; auto.
++ simpl snd.
+  replace (params_of_fundef f) with (@nil type). simpl; auto. clear -E.
+  destruct f as [[? ? [ | [] ]] | e [|] ? c] ; compute in *; congruence.
++ clear - GV H2 H0.
+  split.
+  eapply semax_prog_typecheck_aux; eauto.
+  simpl.
+  auto.
++ hnf; intros; intuition.
++ (*hnf; intros; intuition.
+  unfold normal_ret_assert; simpl.
+  extensionality rho'.
+  normalize.
+  unfold post'.
+  apply pred_ext.
+       normalize. intro rv. do 2 apply exp_right with rv; auto.
+       normalize. intro rv. apply exp_right with rv; auto. *)
+  intros rho' u U y UY k YK K.
+  unfold normal_ret_assert; simpl.
+  destruct K as [v [a1 [a2 [J [A1 [w A2]]]]]]. exists a1, a2; intuition. exists w; trivial.
++ rewrite (corable_funassert _ _).
+  simpl m_phi.
+  rewrite core_inflate_initial_mem'; auto.
+  do 3 (pose proof I).
+  replace (funassert (Delta1 V G)) with
+  (funassert (@nofunc_tycontext V G)).
+  unfold rho1; apply funassert_initial_core; auto.
+  apply same_glob_funassert.
+  reflexivity.
++ apply now_later.
+  intros ek vl tx' vx'.
+  cbv zeta. rewrite proj_frame_ret_assert. simpl seplog.sepcon.
+  subst post'. cbv beta.
+  destruct ek; simpl proj_ret_assert; normalize.
+  apply derives_subp.
+  normalize. intro rv.
+  simpl.
+  eapply derives_trans, own.bupd_intro.
+  intros ? ? ? ? Hora _ ?.
+  destruct H9 as [[? [H10' [H11 ?]]] ?].
+  hnf in H10', H11.
+  destruct H9.
+  subst a.
+  change Clight_new.true_expr with true_expr.
+  change (level (m_phi jm)) with (level jm).
+  apply safe_loop_skip.
++ unfold glob_types, Delta1. simpl @snd.
+  forget (prog_main prog) as main.
+  instantiate (1:= post).
+  instantiate (1:= main_pre prog).
+  assert (H8': list_norepet (map (@fst _ _) (prog_funct prog))). {
+  clear - H0.
+  unfold prog_defs_names in H0. unfold prog_funct.
+  change (AST.prog_defs prog) with (prog_defs prog) in H0.
+  induction (prog_defs prog); auto. inv H0.
+  destruct a; destruct g; simpl; auto. constructor; auto.
+  clear - H2; simpl in H2; contradict H2; induction l; simpl in *; auto.
+  destruct a; destruct g; simpl in *; auto. destruct H2; auto.
+  }
+  forget (prog_funct prog) as fs.
+  clear - H4 H8' H2. rename H8' into H8.
+  fold (main_spec prog).
+  forget (main_spec prog) as fd.
+  revert G H2 H4 H8; induction fs; intros; inv H2.
+  contradiction H4.
+  simpl in *.
+  destruct (ident_eq i main). subst. rewrite PTree.gss.
+  destruct H4. inv H; auto.
+  inv H8.
+  contradiction H3.
+  eapply match_fdecs_in; eauto.
+  apply in_map_fst in H; auto.
+  rewrite PTree.gso by auto.
+  destruct H4; try congruence.
+  inv H8.
+  eapply IHfs; eauto.
++ intros.
+  intros ? ?.
+  split; apply derives_imp; auto.
++ unfold main_pre.
+  apply now_later.
+  rewrite TT_sepcon_TT.
+  rewrite sepcon_comm.
+  eexists; eexists; split; [apply initial_jm_ext_eq|].
+  split; auto.
+ match goal with |- app_pred (globvars2pred (globals_of_env ?A) _ ?B) _ => 
+   change (globals_of_env A) with (globals_of_env B)
+  end.
+  apply global_initializers; auto.
++ simpl.
+  rewrite inflate_initial_mem_level.
+  unfold initial_core.
+  apply level_make_rmap.
+- apply initial_jm_ext_without_locks.
+- apply initial_jm_ext_matchfunspecs. 
+-  destruct (initial_jm_ext_funassert z V prog m G n H1 H0 H2). auto.
+-  destruct (initial_jm_ext_funassert z V prog m G n H1 H0 H2). auto.
 Qed.
 
 (* This version works if we don't need to know anything about the external state. *)
 Lemma semax_prog_rule {CS: compspecs} :
-  OK_ty = unit -> 
-  forall V G prog m h,
-     @semax_prog CS prog V G ->
-     Genv.init_mem prog = Some m ->
-     { b : block & { q : corestate &
-       (Genv.find_symbol (globalenv prog) (prog_main prog) = Some b) *
-       (forall jm, m_dry jm = m -> exists jm', semantics.initial_core (juicy_core_sem (cl_core_sem (globalenv prog))) h
-                    jm q jm' (Vptr b Ptrofs.zero) nil) *
-       forall n,
-         { jm |
-           m_dry jm = m /\ level jm = n /\
-           (forall z, jsafeN (@OK_spec Espec) (globalenv prog) n z q jm) /\
-           no_locks (m_phi jm) /\
-           matchfunspecs (globalenv prog) G (m_phi jm) /\
-           (funassert (nofunc_tycontext V G) (empty_environ (globalenv prog))) (m_phi jm)
-     } } }%type.
+OK_ty = unit -> 
+forall V G prog m h,
+ @semax_prog CS prog V G ->
+ Genv.init_mem prog = Some m ->
+ { b : block & { q : corestate &
+   (Genv.find_symbol (globalenv prog) (prog_main prog) = Some b) *
+   (forall jm, m_dry jm = m -> exists jm', semantics.initial_core (juicy_core_sem (cl_core_sem (globalenv prog))) h
+                jm q jm' (Vptr b Ptrofs.zero) nil) *
+   forall n,
+     { jm |
+       m_dry jm = m /\ level jm = n /\
+       (forall z, jsafeN (@OK_spec Espec) (globalenv prog) n z q jm) /\
+       no_locks (m_phi jm) /\
+       matchfunspecs (globalenv prog) G (m_phi jm) /\
+       (funassert (nofunc_tycontext V G) (empty_environ (globalenv prog))) (m_phi jm)
+ } } }%type.
 Proof.
-  intro OKunit; intros.
-  destruct (semax_prog_rule' V G prog m h H H0) as [b [q [[?H ?H] ?H]]].
-  clear H H0.
-  destruct Espec. simpl in *.
-  exists b, q; split; auto.
-  clear H1 H2.
-  intros n. specialize (H3 n).
-  subst OK_ty. specialize (H3 tt).
- destruct H3 as [jm [? [? ?]]]; exists jm; split3; auto.
- destruct H1 as [? [? [? [? ?]]]]. split3; auto.
- intro. destruct z. auto.
+intro OKunit; intros.
+destruct (semax_prog_rule' V G prog m h H H0) as [b [q [[?H ?H] ?H]]].
+clear H H0.
+destruct Espec. simpl in *.
+exists b, q; split; auto.
+clear H1 H2.
+intros n. specialize (H3 n).
+subst OK_ty. specialize (H3 tt).
+destruct H3 as [jm [? [? ?]]]; exists jm; split3; auto.
+destruct H1 as [? [? [? [? ?]]]]. split3; auto.
+intro. destruct z. auto.
 Qed.
 
 Definition Delta_types V G {C: compspecs} (tys : list type) : tycontext :=
-  make_tycontext
-    (params_of_types
-       1 ((Tfunction (type_of_params (params_of_types 2 tys)) Tvoid cc_default) :: tys))
-    nil nil Tvoid V G nil.
+make_tycontext
+(params_of_types
+   1 ((Tfunction (type_of_params (params_of_types 2 tys)) Tvoid cc_default) :: tys))
+nil nil Tvoid V G nil.
 
 Lemma semax_prog_typecheck_aux_types:
-  forall vs G {C: compspecs} (prog: program) b (typed_args : list (val * type)),
-   list_norepet (prog_defs_names prog) ->
-   match_globvars (prog_vars prog) vs = true ->
-   match_fdecs (prog_funct prog) G ->
-   Forall (fun x => tc_val (snd x) (fst x)) typed_args ->
-   typecheck_environ
-     (Delta_types vs G (map snd typed_args))
-     (construct_rho
-        (filter_genv (globalenv prog)) empty_env
-        (PTree.set 1 (Vptr b Ptrofs.zero)
-                   (temp_bindings 2 (map fst typed_args)))).
+forall vs G {C: compspecs} (prog: program) b (typed_args : list (val * type)),
+list_norepet (prog_defs_names prog) ->
+match_globvars (prog_vars prog) vs = true ->
+match_fdecs (prog_funct prog) G ->
+Forall (fun x => tc_val (snd x) (fst x)) typed_args ->
+typecheck_environ
+ (Delta_types vs G (map snd typed_args))
+ (construct_rho
+    (filter_genv (globalenv prog)) empty_env
+    (PTree.set 1 (Vptr b Ptrofs.zero)
+               (temp_bindings 2 (map fst typed_args)))).
 Proof.
-  intros vs G C prog b typed_args NR MG MF TYP.
-  repeat split.
-  - unfold te_of, construct_rho.
-    intros i ty.
-    unfold make_tycontext, temp_types.
-    intros Found.
-    assert (make_tycontext_t_cons1 : forall i i' t l1 l2, (make_tycontext_t ((i, t) :: l1) l2) ! i' =
-      if peq i' i then Some t else (make_tycontext_t l1 l2) ! i')
-    by (clear; intros i i' t l1 l2; simpl; rewrite PTree.gsspec; reflexivity).
-    unfold Delta_types, make_tycontext in Found.
-    simpl params_of_types in Found.
+intros vs G C prog b typed_args NR MG MF TYP.
+repeat split.
+- unfold te_of, construct_rho.
+intros i ty.
+unfold make_tycontext, temp_types.
+intros Found.
+assert (make_tycontext_t_cons1 : forall i i' t l1 l2, (make_tycontext_t ((i, t) :: l1) l2) ! i' =
+  if peq i' i then Some t else (make_tycontext_t l1 l2) ! i')
+by (clear; intros i i' t l1 l2; simpl; rewrite PTree.gsspec; reflexivity).
+unfold Delta_types, make_tycontext in Found.
+simpl params_of_types in Found.
+rewrite make_tycontext_t_cons1 in Found.
+rewrite <-map_ptree_rel, Map.gsspec.
+if_tac; if_tac in Found; subst; try tauto.
++ injection Found as <-.
+  exists (Vptr b Ptrofs.zero); split; auto.
+  apply tc_val_tc_val'; simpl; auto.
++ revert Found; generalize (2%positive).
+  induction typed_args; intros p Found.
+  * rewrite PTree.gempty in Found.
+    discriminate.
+  * simpl (params_of_types _ _ ) in Found.
     rewrite make_tycontext_t_cons1 in Found.
+    simpl (map _ _).
+    change (exists v : val, Map.get (make_tenv (PTree.set p (fst a) (temp_bindings (p+1)
+      (map fst typed_args)))) i = Some v /\ tc_val' ty v).
     rewrite <-map_ptree_rel, Map.gsspec.
-    if_tac; if_tac in Found; subst; try tauto.
-    + injection Found as <-.
-      exists (Vptr b Ptrofs.zero); split; auto.
-      apply tc_val_tc_val'; simpl; auto.
-    + revert Found; generalize (2%positive).
-      induction typed_args; intros p Found.
-      * rewrite PTree.gempty in Found.
-        discriminate.
-      * simpl (params_of_types _ _ ) in Found.
-        rewrite make_tycontext_t_cons1 in Found.
-        simpl (map _ _).
-        change (exists v : val, Map.get (make_tenv (PTree.set p (fst a) (temp_bindings (p+1)
-          (map fst typed_args)))) i = Some v /\ tc_val' ty v).
-        rewrite <-map_ptree_rel, Map.gsspec.
-        inversion TYP.
-        { if_tac; if_tac in Found; subst; try tauto.
-          - injection Found as <-. apply tc_val_tc_val' in H3; eauto.
-          - apply IHtyped_args; auto. }
-  - simpl.
-    rewrite PTree.gempty.
-    intro; discriminate.
-  - simpl.
-    unfold make_venv, Map.get, empty_env.
-    rewrite PTree.gempty.
-    intros [? ?]; discriminate.
-  - eapply tc_ge_denote_initial; eauto.
+    inversion TYP.
+    { if_tac; if_tac in Found; subst; try tauto.
+      - injection Found as <-. apply tc_val_tc_val' in H3; eauto.
+      - apply IHtyped_args; auto. }
+- simpl.
+rewrite PTree.gempty.
+intro; discriminate.
+- simpl.
+unfold make_venv, Map.get, empty_env.
+rewrite PTree.gempty.
+intros [? ?]; discriminate.
+- eapply tc_ge_denote_initial; eauto.
 Qed.
 
 Lemma find_id_maketycontext_s G id : (make_tycontext_s G) ! id = find_id id G.
 Proof.
-  induction G as [|(i,t) G]; simpl.
-  - destruct id; reflexivity.
-  - rewrite PTree.gsspec.
-    do 2 if_tac; congruence.
+induction G as [|(i,t) G]; simpl.
+- destruct id; reflexivity.
+- rewrite PTree.gsspec.
+do 2 if_tac; congruence.
 Qed.
 
 Lemma semax_prog_entry_point {CS: compspecs} V G prog b id_fun id_arg arg A 
-   (P Q: forall ts : list Type, (dependent_type_functor_rec ts (AssertTT A)) mpred)
-   NEP NEQ h:
-  @semax_prog CS prog V G ->
-  Genv.find_symbol (globalenv prog) id_fun = Some b ->
-  find_id id_fun G =
-    Some (mk_funspec ((id_arg, Tpointer Tvoid noattr) :: nil, tptr Tvoid)
-                     cc_default A P Q NEP NEQ) ->
-  is_pointer_or_null arg ->
-  (* initial environment *)
-  let rho0 : environ :=
+(P Q: forall ts : list Type, (dependent_type_functor_rec ts (AssertTT A)) mpred)
+NEP NEQ h:
+@semax_prog CS prog V G ->
+Genv.find_symbol (globalenv prog) id_fun = Some b ->
+find_id id_fun G =
+Some (mk_funspec ((id_arg, Tpointer Tvoid noattr) :: nil, tptr Tvoid)
+                 cc_default A P Q NEP NEQ) ->
+is_pointer_or_null arg ->
+(* initial environment *)
+let rho0 : environ :=
+  construct_rho
+    (filter_genv (globalenv prog)) empty_env
+    (PTree.set 1 (Vptr b Ptrofs.zero)
+               (PTree.set id_arg arg (PTree.empty val))) in
+
+(* initial environment without the function => to check jm |= P a *)
+let rho1 : environ :=
+  construct_rho
+    (filter_genv (globalenv prog)) empty_env
+    ((* PTree.set 1 (Vptr b Ptrofs.zero) *)
+      (PTree.set id_arg arg (PTree.empty val))) in
+
+{ q : corestate |
+(forall jm, Val.inject (Mem.flat_inj (nextblock (m_dry jm))) arg arg ->
+  exists jm', semantics.initial_core
+  (juicy_core_sem (cl_core_sem (globalenv prog))) h
+  jm q jm' (Vptr b Ptrofs.zero) (arg :: nil)) /\
+
+forall (jm : juicy_mem) ts a,
+  app_pred (P ts a rho1) (m_phi jm) ->
+(*      (forall rho, app_pred (! (Q ts a rho >=> !!False)) (m_phi jm)) ->*)
+  app_pred (funassert (Delta_types V G (Tpointer Tvoid noattr::nil)) rho0) (m_phi jm) ->
+  forall z, app_pred (ext_compat z) (m_phi jm) -> jsafeN (@OK_spec Espec) (globalenv prog) (level jm) z q jm }.
+Proof.
+intros SP Findb id_in_G arg_p.
+assert (CSUBmain: cenv_sub (@cenv_cs CS) (globalenv prog)).
+{ destruct SP as [_ [_ [CSEQ _]]]. rewrite CSEQ; apply cenv_sub_refl. }
+destruct ((fun x => x) SP) as (_ & _ & _ & (MatchFdecs & (Gcontains & Believe)) & _).
+specialize (Believe (globalenv prog)).
+spec Believe; [ intros; apply sub_option_refl |].
+spec Believe; [ intros; apply sub_option_refl |]. (*
+spec Believe. now apply prog_contains_prog_funct, compute_list_norepet_e, SP.
+spec Believe. (*now symmetry; apply SP.*) apply CSUBmain. *)
+pose proof Believe as Believe_.
+specialize (Believe 5%nat).
+unfold claims in *.
+unfold nofunc_tycontext in *.
+simpl glob_specs in Believe.
+rewrite <-find_id_maketycontext_s in id_in_G.
+
+specialize (Believe (Vptr b Ptrofs.zero)
+                  ((id_arg, Tpointer Tvoid noattr) :: nil, tptr Tvoid)
+                  cc_default A P Q _ (necR_refl _)).
+spec Believe.
+{ exists id_fun, NEP, NEQ. split; auto. exists b; split; auto. }
+simpl (semantics.initial_core _). unfold j_initial_core.
+simpl (semantics.initial_core _). unfold cl_initial_core.
+if_tac [_|?]. 2:solve[tauto].
+
+destruct (Genv.find_funct_ptr (globalenv prog) b) as [f|] eqn:Eb; swap 1 2.
+{ exfalso.
+destruct Believe as [H | (b' & fu & (? & WOB & ASD) & WOBk)].
++ unfold believe_external in *.
+  unfold Genv.find_funct in *. rewrite if_true in H by trivial.
+  simpl in Eb, H. rewrite Eb in H. auto. 
++ assert (b' = b) by congruence. simpl in WOB, Eb. subst b'. congruence.
+}
+assert (Ef : type_of_fundef f = Tfunction (Tcons (Tpointer Tvoid noattr) Tnil) (tptr Tvoid) cc_default). {
+(* I think this can be proved using believe_internal / believe_external ? *)
+destruct Believe as [BE|BI].
+- unfold believe_external in *.
+  simpl in BE. if_tac [_|?] in BE. 2:tauto.
+  replace (Genv.find_funct_ptr (globalenv prog)) with
+  (Genv.find_funct_ptr (Genv.globalenv prog)) in *
+    by reflexivity.
+  unfold fundef in BE.
+  rewrite Eb in BE.
+  destruct f as [ | ef sigargs sigret c'']. tauto.
+  simpl.
+  destruct BE as [((Es & -> & ASD & LEN) & ?) _]. injection Es as Es <-. f_equal.
+  destruct sigargs as [ | ? [ | ]]; simpl in Es.
+  + congruence.
+  + congruence.
+  + (* in believe_external, zip_with_tl throws away arguments if they are not named *)
+    simpl in LEN. disc.
+
+- destruct BI as (b' & fu & (? & WOB & ? & ? & ? & ? & wob & ?) & WOBk).
+  unfold fn_funsig in *. injection wob as Hpar Hret.
+  assert (b' = b) by congruence. subst b'.
+  simpl in Eb, WOB. assert (f = Internal fu) by congruence. subst f.
+  simpl.
+  unfold type_of_function.
+  destruct fu as [? ? [ | [] [ | [] ]] ? ?]; simpl in *; congruence.
+}
+rewrite Ef.
+eexists. split.
+intros. eexists; repeat split; eauto.
+repeat constructor.
+{clear - arg_p.
+destruct arg; try contradiction.
+first [apply val_casted_long_ptr |  apply val_casted_int_ptr]; reflexivity.
+apply val_casted_ptr_ptr. }
+{ clear - arg_p. destruct arg; try contradiction; simpl in *.
+  unfold Tptr. destruct Archi.ptr64; try contradiction; auto.
+  unfold Tptr. destruct Archi.ptr64; auto.
+}
+{ unfold arg_well_formed. constructor; auto. } 
+
+intros jm ts a m_sat_Pa m_funassert.
+
+assert (Pf : params_of_fundef f = Tpointer Tvoid noattr :: nil).
+{ clear -Ef.
+destruct f as [f|f]. simpl in *.
+unfold type_of_function in *.
+destruct f as [? ? [ | [] [ | [] ]] ? ?]; simpl in *; congruence.
+simpl in *. injection Ef; intros; subst. reflexivity. }
+
+pose (rho3 :=
       construct_rho
         (filter_genv (globalenv prog)) empty_env
         (PTree.set 1 (Vptr b Ptrofs.zero)
-                   (PTree.set id_arg arg (PTree.empty val))) in
+                   (temp_bindings 2 (map fst ((arg, Tpointer Tvoid noattr) :: nil))))).
+pose proof I.
+intros z HZ.
+set (R:= fun rho' => EX _ : val,
+       (EX x : val, emp * Q ts a (env_set (globals_only rho') ret_temp x))).
+eapply
+(semax_call_aux
+   (Delta_types V G (Tpointer Tvoid noattr::nil)) A P
+   (fun _ _ => Q ts a) Q NEP NEQ
+   ts a (fun _ => emp) (fun _ => emp)
+   None ((id_arg, Tpointer Tvoid noattr)::nil, tptr Tvoid) cc_default _ _
+   (normal_ret_assert R)
+   _ _ _ _ rho3
+   _ _ b id_fun);
+try apply H3; try eassumption; auto.
 
-  (* initial environment without the function => to check jm |= P a *)
-  let rho1 : environ :=
-      construct_rho
-        (filter_genv (globalenv prog)) empty_env
-        ((* PTree.set 1 (Vptr b Ptrofs.zero) *)
-          (PTree.set id_arg arg (PTree.empty val))) in
+(* tc_expr *)
 
-  { q : corestate |
-    (forall jm, Val.inject (Mem.flat_inj (nextblock (m_dry jm))) arg arg ->
-      exists jm', semantics.initial_core
-      (juicy_core_sem (cl_core_sem (globalenv prog))) h
-      jm q jm' (Vptr b Ptrofs.zero) (arg :: nil)) /\
+simpl. exists (Vptr b Ptrofs.zero); auto.
 
-    forall (jm : juicy_mem) ts a,
-      app_pred (P ts a rho1) (m_phi jm) ->
-(*      (forall rho, app_pred (! (Q ts a rho >=> !!False)) (m_phi jm)) ->*)
-      app_pred (funassert (Delta_types V G (Tpointer Tvoid noattr::nil)) rho0) (m_phi jm) ->
-      forall z, app_pred (ext_compat z) (m_phi jm) -> jsafeN (@OK_spec Espec) (globalenv prog) (level jm) z q jm }.
-Proof.
-  intros SP Findb id_in_G arg_p.
-  assert (CSUBmain: cenv_sub (@cenv_cs CS) (globalenv prog)).
-  { destruct SP as [_ [_ [CSEQ _]]]. rewrite CSEQ; apply cenv_sub_refl. }
-  destruct ((fun x => x) SP) as (_ & _ & _ & (MatchFdecs & Believe) & _).
-  specialize (Believe (globalenv prog)).
-  spec Believe. now apply prog_contains_prog_funct, compute_list_norepet_e, SP.
-  spec Believe. (*now symmetry; apply SP.*) apply CSUBmain. 
-  pose proof Believe as Believe_.
-  specialize (Believe 5%nat).
-  unfold claims in *.
-  unfold nofunc_tycontext in *.
-  simpl glob_specs in Believe.
-  rewrite <-find_id_maketycontext_s in id_in_G.
+(* tc_exprlist *)
+rewrite Pf. simpl. exists arg; simpl; auto.
 
-  specialize (Believe (Vptr b Ptrofs.zero)
-                      ((id_arg, Tpointer Tvoid noattr) :: nil, tptr Tvoid)
-                      cc_default A P Q _ (necR_refl _)).
-  spec Believe.
-  { exists id_fun, NEP, NEQ. split; auto. exists b; split; auto. }
-  simpl (semantics.initial_core _). unfold j_initial_core.
-  simpl (semantics.initial_core _). unfold cl_initial_core.
-  if_tac [_|?]. 2:tauto.
+(* guard_environ *)
+split; try apply I.
+eapply semax_prog_typecheck_aux_types; eauto.
+apply compute_list_norepet_e. apply SP. apply SP.
 
-  destruct (Genv.find_funct_ptr (globalenv prog) b) as [f|] eqn:Eb; swap 1 2.
-  { exfalso.
-    destruct Believe as [H | (b' & fu & (? & WOB & ASD) & WOBk)].
-    unfold believe_external in *.
-    unfold Genv.find_funct in *.
-    if_tac [_|?] in H. rewrite Eb in H. auto. tauto.
-    assert (b' = b) by congruence. subst b'. congruence.
-  }
-  assert (Ef : type_of_fundef f = Tfunction (Tcons (Tpointer Tvoid noattr) Tnil) (tptr Tvoid) cc_default). {
-    (* I think this can be proved using believe_internal / believe_external ? *)
-    destruct Believe as [BE|BI].
-    - unfold believe_external in *.
-      simpl in BE. if_tac [_|?] in BE. 2:tauto.
-      replace (Genv.find_funct_ptr (globalenv prog)) with
-      (Genv.find_funct_ptr (Genv.globalenv prog)) in *
-        by reflexivity.
-      unfold fundef in BE.
-      rewrite Eb in BE.
-      destruct f as [ | ef sigargs sigret c'']. tauto.
-      simpl.
-      destruct BE as [((Es & -> & ASD & LEN) & ?) _]. injection Es as Es <-. f_equal.
-      destruct sigargs as [ | ? [ | ]]; simpl in Es.
-      + congruence.
-      + congruence.
-      + (* in believe_external, zip_with_tl throws away arguments if they are not named *)
-        simpl in LEN. disc.
+(* closed_wrt_modvars *)
+intro.
+reflexivity.
 
-    - destruct BI as (b' & fu & (? & WOB & ? & ? & ? & ? & wob & ?) & WOBk).
-      unfold fn_funsig in *. injection wob as Hpar Hret.
-      assert (b' = b) by congruence. subst b'.
-      assert (f = Internal fu) by congruence. subst f.
-      simpl.
-      unfold type_of_function.
-      destruct fu as [? ? [ | [] [ | [] ]] ? ?]; simpl in *; congruence.
-  }
-  rewrite Ef.
-  eexists. split.
-  intros. eexists; repeat split; eauto.
-  repeat constructor.
-  {clear - arg_p.
-   destruct arg; try contradiction.
-   first [apply val_casted_long_ptr |  apply val_casted_int_ptr]; reflexivity.
-   apply val_casted_ptr_ptr. }
-  { clear - arg_p. destruct arg; try contradiction; simpl in *.
-      unfold Tptr. destruct Archi.ptr64; try contradiction; auto.
-      unfold Tptr. destruct Archi.ptr64; auto.
-  }
-  { unfold arg_well_formed. constructor; auto. } 
+(* equality of normal_ret_assert 
+unfold R.
+unfold normal_ret_assert; simpl.
+extensionality rho'.
+normalize.
+reflexivity.*)
 
-  intros jm ts a m_sat_Pa m_funassert.
+(*entailment of  normal_ret_assert *)
+rewrite <- box_all. apply now_later. unfold R.
+unfold normal_ret_assert. simpl. intros. destruct H2 as [v [a1 [a2 [J [HY [w HQ]]]]]].
+exists v, w, a1, a2; auto.
 
-  assert (Pf : params_of_fundef f = Tpointer Tvoid noattr :: nil).
-  { clear -Ef.
-    destruct f as [f|f]. simpl in *.
-    unfold type_of_function in *.
-    destruct f as [? ? [ | [] [ | [] ]] ? ?]; simpl in *; congruence.
-    simpl in *. injection Ef; intros; subst. reflexivity. }
+(* globalenv prog = cenv_cs *)
+(*destruct SP as [? [AL [HGG [[H2 H3] [GV _]]]]].
+rewrite HGG. reflexivity.*)
 
-  pose (rho3 :=
-          construct_rho
-            (filter_genv (globalenv prog)) empty_env
-            (PTree.set 1 (Vptr b Ptrofs.zero)
-                       (temp_bindings 2 (map fst ((arg, Tpointer Tvoid noattr) :: nil))))).
-  pose proof I.
-  intros z HZ.
-  set (R:= fun rho' => EX _ : val,
-           (EX x : val, emp * Q ts a (env_set (globals_only rho') ret_temp x))).
-  eapply
-    (semax_call_aux
-       (Delta_types V G (Tpointer Tvoid noattr::nil)) A P
-       (fun _ _ => Q ts a) Q NEP NEQ
-       ts a (fun _ => emp) (fun _ => emp)
-       None ((id_arg, Tpointer Tvoid noattr)::nil, tptr Tvoid) cc_default _ _
-       (normal_ret_assert R)
-       _ _ _ _ rho3
-       _ _ b id_fun);
-    try apply H3; try eassumption; auto.
+(* safety: we conclude as we add an infinite loop at the end *)
+apply now_later.
+intros ek ret te env phi lev phi' necr [[Guard FrameRA] FunAssert].
+apply own.bupd_intro; intros ora jm0 Hora Heq <-.
+rewrite proj_frame_ret_assert in FrameRA. simpl seplog.sepcon in FrameRA.
+destruct ek; simpl proj_ret_assert in FrameRA;
+try solve [elimtype False; clear - FrameRA; destruct FrameRA as [? [? [? [[? ?] ?]]]]; contradiction];
+try solve [elimtype False; clear - FrameRA; destruct FrameRA as [? [? [? [? ?]]]]; contradiction].
+apply safe_loop_skip.
+(* equivalence between Q and Q' *)
+intros vl; split; apply derives_imp; apply derives_refl'; reflexivity.
 
-  (* tc_expr *)
-
-  simpl. exists (Vptr b Ptrofs.zero); auto.
-
-  (* tc_exprlist *)
-  rewrite Pf. simpl. exists arg; simpl; auto.
-
-  (* guard_environ *)
-  split; try apply I.
-  eapply semax_prog_typecheck_aux_types; eauto.
-  apply compute_list_norepet_e. apply SP. apply SP.
-
-  (* closed_wrt_modvars *)
-  intro.
-  reflexivity.
-
-  (* equality of normal_ret_assert 
-  unfold R.
-  unfold normal_ret_assert; simpl.
-  extensionality rho'.
-  normalize.
-  reflexivity.*)
-  
-  (*entailment of  normal_ret_assert *)
-  rewrite <- box_all. apply now_later. unfold R.
-  unfold normal_ret_assert. simpl. intros. destruct H2 as [v [a1 [a2 [J [HY [w HQ]]]]]].
-  exists v, w, a1, a2; auto.
-
-  (* globalenv prog = cenv_cs *)
-  (*destruct SP as [? [AL [HGG [[H2 H3] [GV _]]]]].
-  rewrite HGG. reflexivity.*)
-
-  (* safety: we conclude as we add an infinite loop at the end *)
-  apply now_later.
-  intros ek ret te env phi lev phi' necr [[Guard FrameRA] FunAssert].
-  apply own.bupd_intro; intros ora jm0 Hora Heq <-.
-  rewrite proj_frame_ret_assert in FrameRA. simpl seplog.sepcon in FrameRA.
-  destruct ek; simpl proj_ret_assert in FrameRA;
-   try solve [elimtype False; clear - FrameRA; destruct FrameRA as [? [? [? [[? ?] ?]]]]; contradiction];
-   try solve [elimtype False; clear - FrameRA; destruct FrameRA as [? [? [? [? ?]]]]; contradiction].
-   apply safe_loop_skip.
-  (* equivalence between Q and Q' *)
-  intros vl; split; apply derives_imp; apply derives_refl'; reflexivity.
-
-  (* precondition *)
-  refine (derives_e _ _ _ _ m_sat_Pa).
-  normalize.
-  eapply derives_trans; [|apply now_later].
-  apply derives_refl'; f_equal.
-  rewrite Pf.
-  simpl.
-  unfold globals_only, env_set, construct_rho.
-  simpl.
-  f_equal.
-  extensionality i; destruct i; reflexivity.
-  unfold make_tenv, force_val, sem_cast_pointer, eval_id.
-  extensionality i.
-  rewrite PTree.gsspec.
-  unfold Map.set.
-  if_tac; if_tac; try congruence; subst.
-  unfold liftx, lift; simpl.
-  now destruct arg; inversion arg_p; auto.
-  now destruct i; reflexivity.
+(* precondition *)
+refine (derives_e _ _ _ _ m_sat_Pa).
+normalize.
+eapply derives_trans; [|apply now_later].
+apply derives_refl'; f_equal.
+rewrite Pf.
+simpl.
+unfold globals_only, env_set, construct_rho.
+simpl.
+f_equal.
+extensionality i; destruct i; reflexivity.
+unfold make_tenv, force_val, sem_cast_pointer, eval_id.
+extensionality i.
+rewrite PTree.gsspec.
+unfold Map.set.
+if_tac; if_tac; try congruence; subst.
+unfold liftx, lift; simpl.
+now destruct arg; inversion arg_p; auto.
+now destruct i; reflexivity.
 Qed.
 
 Lemma match_fdecs_length funs K:
-      match_fdecs funs K -> length funs = length K.
+  match_fdecs funs K -> length funs = length K.
 Proof. induction 1; trivial. 
 simpl; rewrite IHmatch_fdecs; trivial.
 Qed.
 
 Lemma match_fdecs_nil_iff funs K (M: match_fdecs funs K):
- (funs = nil) <-> (K=nil).
+(funs = nil) <-> (K=nil).
 Proof. apply match_fdecs_length in M. 
- split; intros; subst; simpl in M.
- destruct K; trivial; inv M.
- destruct funs; trivial; inv M.
+split; intros; subst; simpl in M.
+destruct K; trivial; inv M.
+destruct funs; trivial; inv M.
 Qed.
 
 Lemma match_fdecs_cons_D f funs k K (M: match_fdecs (cons f funs) (cons k K)):
-  exists i fd fspec, f=(i,fd) /\ k=(i,fspec) /\ 
-         type_of_fundef fd = type_of_funspec fspec /\
-         match_fdecs funs K.
+exists i fd fspec, f=(i,fd) /\ k=(i,fspec) /\ 
+     type_of_fundef fd = type_of_funspec fspec /\
+     match_fdecs funs K.
 Proof. inv M. exists i, fd, fspec; intuition. Qed.
 
 Lemma match_fdecs_cons_D1 f funs K (M: match_fdecs (cons f funs) K):
-  exists i fd fspec G, f=(i,fd) /\ K=cons (i,fspec) G /\ 
-         type_of_fundef fd = type_of_funspec fspec /\
-         match_fdecs funs G.
+exists i fd fspec G, f=(i,fd) /\ K=cons (i,fspec) G /\ 
+     type_of_fundef fd = type_of_funspec fspec /\
+     match_fdecs funs G.
 Proof. inv M. exists i, fd, fspec, G; intuition. Qed.
 
 Lemma match_fdecs_cons_D2 funs k K (M: match_fdecs funs (cons k K)):
-  exists i fd fspec fs, funs=cons (i,fd) fs /\ k=(i,fspec) /\ 
-         type_of_fundef fd = type_of_funspec fspec /\
-         match_fdecs fs K.
+exists i fd fspec fs, funs=cons (i,fd) fs /\ k=(i,fspec) /\ 
+     type_of_fundef fd = type_of_funspec fspec /\
+     match_fdecs fs K.
 Proof. inv M. exists i, fd, fspec, fs; intuition. Qed.
 
-Lemma semax_func_length V G {C: compspecs} funs K (M: semax_func V G funs K):
-     length funs = length K.
+(*Lemma semax_func_length V G {C: compspecs} funs K (M: semax_func V G funs K):
+ length funs = length K.
+Proof. destruct M as [M _]. apply match_fdecs_length in M; trivial. Qed.*)
+Lemma semax_func_length ge V G {C: compspecs} funs K (M: semax_func V G ge funs K):
+ length funs = length K.
 Proof. destruct M as [M _]. apply match_fdecs_length in M; trivial. Qed.
 
 Lemma match_fdecs_app: forall vl G vl' G',
-  match_fdecs vl G -> match_fdecs vl' G' -> match_fdecs (vl ++ vl') (G ++ G').
+match_fdecs vl G -> match_fdecs vl' G' -> match_fdecs (vl ++ vl') (G ++ G').
 Proof. induction vl; simpl; intros; inv H; simpl in *; trivial; econstructor; eauto. Qed.
 
 Lemma prog_contains_nil ge: prog_contains ge nil.
 Proof. red; intros. inv H. Qed.
 Lemma prog_contains_app_inv ge: forall funs1 funs2, prog_contains ge (funs1 ++ funs2) ->
-      prog_contains ge funs1 /\ prog_contains ge funs2.
+  prog_contains ge funs1 /\ prog_contains ge funs2.
 Proof. induction funs1; simpl; intros; split; trivial.
 + apply prog_contains_nil.
 + red; intros. apply (H id f).
-  destruct H0; [ left; trivial | right; apply in_or_app; left; trivial].
+destruct H0; [ left; trivial | right; apply in_or_app; left; trivial].
 + red; intros. apply (H id f).
-  right; apply in_or_app; right; trivial.
+right; apply in_or_app; right; trivial.
 Qed.
 
+Lemma genv_contains_nil ge: genv_contains ge nil.
+Proof. red; intros. inv H. Qed.
+Lemma genv_contains_app_inv ge: forall funs1 funs2, genv_contains ge (funs1 ++ funs2) ->
+  genv_contains ge funs1 /\ genv_contains ge funs2.
+Proof. induction funs1; simpl; intros; split; trivial.
++ apply genv_contains_nil.
++ red; intros. apply (H id f).
+destruct H0; [ left; trivial | right; apply in_or_app; left; trivial].
++ red; intros. apply (H id f).
+right; apply in_or_app; right; trivial.
+Qed.
+Lemma genv_contains_app ge funs1 funs2 (G1:genv_contains ge funs1) (G2: genv_contains ge funs2):
+genv_contains ge (funs1 ++ funs2).
+Proof. red; intros. apply in_app_or in H; destruct H; [apply G1 | apply G2]; trivial. Qed. 
+
 Lemma find_id_app i fs: forall (G1 G2: funspecs) (G: find_id i (G1 ++ G2) = Some fs),
-  find_id i G1 = Some fs \/ find_id i G2 = Some fs.
+find_id i G1 = Some fs \/ find_id i G2 = Some fs.
 Proof. induction G1; simpl; intros. right; trivial. 
 destruct a. destruct (eq_dec i i0); [ left; trivial | eauto].
 Qed.
 
 Lemma make_tycontext_s_app_inv i fs G1 G2 (G: (make_tycontext_s (G1 ++ G2)) ! i = Some fs):
-      (make_tycontext_s G1) ! i = Some fs \/ (make_tycontext_s G2) ! i = Some fs.
+  (make_tycontext_s G1) ! i = Some fs \/ (make_tycontext_s G2) ! i = Some fs.
 Proof. rewrite ! find_id_maketycontext_s  in *. apply find_id_app; trivial. Qed.
- 
-Lemma believe_app_inv {cs} ge V H G1 G2 n 
-  (B1: @believe cs Espec (nofunc_tycontext V H) ge (nofunc_tycontext V G1) n)
-  (B2: @believe cs Espec (nofunc_tycontext V H) ge (nofunc_tycontext V G2) n):
-  @believe cs Espec (nofunc_tycontext V H) ge (nofunc_tycontext V (G1 ++ G2)) n.
+
+Lemma believe_app {cs} ge V H G1 G2 n 
+(B1: @believe cs Espec (nofunc_tycontext V H) ge (nofunc_tycontext V G1) n)
+(B2: @believe cs Espec (nofunc_tycontext V H) ge (nofunc_tycontext V G2) n):
+@believe cs Espec (nofunc_tycontext V H) ge (nofunc_tycontext V (G1 ++ G2)) n.
 Proof. 
 intros v fsig cc A P Q k NEC CL.
 destruct CL as [i [HP [HQ [G B]]]].
@@ -1918,628 +1956,325 @@ simpl in G. apply make_tycontext_s_app_inv in G; destruct G.
 + apply B2; trivial. exists i, HP, HQ; simpl; split; trivial.
 Qed.
 
-Lemma semax_func_app cs V H: forall funs1 funs2 G1 G2
-   (SF1: @semax_func V H cs funs1 G1) (SF2: @semax_func V H cs funs2 G2)
-   (L:length funs1 = length G1),
-   @semax_func V H cs (funs1 ++ funs2) (G1++G2).
+Lemma semax_func_app ge cs V H: forall funs1 funs2 G1 G2
+(SF1: @semax_func V H cs ge funs1 G1) (SF2: @semax_func V H cs ge funs2 G2)
+(L:length funs1 = length G1),
+@semax_func V H cs ge (funs1 ++ funs2) (G1++G2).
 Proof.
-intros. destruct SF1 as [MF1 B1]. destruct SF2 as [MF2 B2]. 
+intros. destruct SF1 as [MF1 [GC1 B1]]. destruct SF2 as [MF2 [GC2 B2]]. 
 split; [ apply match_fdecs_app; trivial | intros; subst].
-apply prog_contains_app_inv in H0; destruct H0 as [PG1 PG2].
-specialize (B1 ge PG1 H1 n). specialize (B2 ge PG2 H1 n).
-clear -B1 B2.
-apply believe_app_inv; eauto.
+split; [ apply genv_contains_app; trivial | intros].
+apply believe_app; [ apply B1 | apply B2]; trivial.
 Qed.
 
-Lemma semax_func_subsumption cs V V' F F'
-      (SUB: tycontext_sub (nofunc_tycontext V F) (nofunc_tycontext V F'))
-      (HV: forall id, sub_option (make_tycontext_g V F) ! id (make_tycontext_g V' F') ! id):
-  forall funs G (SF: @semax_func V F cs funs G),  @semax_func V' F' cs funs G.
+Lemma semax_func_subsumption ge cs V V' F F'
+  (SUB: tycontext_sub (nofunc_tycontext V F) (nofunc_tycontext V F'))
+  (HV: forall id, sub_option (make_tycontext_g V F) ! id (make_tycontext_g V' F') ! id):
+forall funs G (SF: @semax_func V F cs ge funs G),  @semax_func V' F' cs ge funs G.
 Proof.
-  intros. destruct SF as [MF B]. split; [trivial | intros]. specialize (B _ H H0 n).
-  assert (TS: forall f, tycontext_sub (func_tycontext' f (nofunc_tycontext V F)) (func_tycontext' f (nofunc_tycontext V' F'))).
-  { clear - SUB HV.
-    destruct SUB as [SUBa [SUBb [SUBc [SUBd [SUBe SUBf]]]]]; simpl in *.
-    unfold func_tycontext'; split; simpl; intuition.
-    destruct ((make_tycontext_t (fn_params f) (fn_temps f)) ! id); trivial. }
-  eapply believe_monoL; [eassumption | apply cspecs_sub_refl | eassumption]. 
-Qed.
-            
-Lemma semax_func_join cs V1 H1 V2 H2 V funs1 funs2 G1 G2 H
-      (SF1: @semax_func V1 H1 cs funs1 G1) (SF2: @semax_func V2 H2 cs funs2 G2)
-      
-      (K1: forall i, sub_option ((make_tycontext_g V1 H1) ! i) ((make_tycontext_g V1 H) ! i))
-      (K2: forall i, subsumespec ((make_tycontext_s H1) ! i) ((make_tycontext_s H) ! i))
-      (K3: forall i, sub_option ((make_tycontext_g V1 H) ! i) ((make_tycontext_g V H) ! i))
-      
-      (N1: forall i, sub_option ((make_tycontext_g V2 H2) ! i) ((make_tycontext_g V2 H) ! i))
-      (N2: forall i, subsumespec ((make_tycontext_s H2) ! i) ((make_tycontext_s H) ! i))
-      (N3: forall i, sub_option ((make_tycontext_g V2 H) ! i) ((make_tycontext_g V H) ! i)):
-  @semax_func V H cs (funs1 ++ funs2) (G1++G2).
-Proof.
-  apply semax_func_app.
-  + eapply semax_func_subsumption; [ | | apply SF1].
-  - hnf; simpl. intuition.
-    * rewrite PTree.gempty; trivial.
-    * rewrite PTree.gempty. simpl; trivial.
-  - intros. specialize (K1 id). eapply sub_option_trans. apply K1. trivial.
-  + eapply semax_func_subsumption; [ | | apply SF2].
-  - hnf; simpl. intuition.
-    * rewrite PTree.gempty; trivial.
-    * rewrite PTree.gempty. simpl; trivial.
-  - intros. specialize (N1 id). eapply sub_option_trans. apply N1. trivial.
-  + clear - SF1. eapply semax_func_length. apply SF1.
+intros. destruct SF as [MF [GC B]]. split; [trivial | split; [ trivial | intros]]. specialize (B _ Gfs Gffp n). 
+assert (TS: forall f, tycontext_sub (func_tycontext' f (nofunc_tycontext V F)) (func_tycontext' f (nofunc_tycontext V' F'))).
+{ clear - SUB HV.
+destruct SUB as [SUBa [SUBb [SUBc [SUBd [SUBe SUBf]]]]]; simpl in *.
+unfold func_tycontext'; split; simpl; intuition.
+destruct ((make_tycontext_t (fn_params f) (fn_temps f)) ! id); trivial. }
+eapply believe_monoL; [eassumption | apply cspecs_sub_refl | eassumption]. 
 Qed.
 
-Lemma semax_func_join_sameV cs H1 H2 V funs1 funs2 G1 G2 H
-      (SF1: @semax_func V H1 cs funs1 G1) (SF2: @semax_func V H2 cs funs2 G2)
-      
-      (K1: forall i, sub_option ((make_tycontext_g V H1) ! i) ((make_tycontext_g V H) ! i))
-      (K2: forall i, subsumespec ((make_tycontext_s H1) ! i) ((make_tycontext_s H) ! i))
-      
-      (N1: forall i, sub_option ((make_tycontext_g V H2) ! i) ((make_tycontext_g V H) ! i))
-      (N2: forall i, subsumespec ((make_tycontext_s H2) ! i) ((make_tycontext_s H) ! i)):
-  @semax_func V H cs (funs1 ++ funs2) (G1++G2).
+Lemma semax_func_join {cs ge V1 H1 V2 H2 V funs1 funs2 G1 G2 H}
+  (SF1: @semax_func V1 H1 cs ge funs1 G1) (SF2: @semax_func V2 H2 cs ge funs2 G2)
+
+  (K1: forall i, sub_option ((make_tycontext_g V1 H1) ! i) ((make_tycontext_g V1 H) ! i))
+  (K2: forall i, subsumespec ((make_tycontext_s H1) ! i) ((make_tycontext_s H) ! i))
+  (K3: forall i, sub_option ((make_tycontext_g V1 H) ! i) ((make_tycontext_g V H) ! i))
+
+  (N1: forall i, sub_option ((make_tycontext_g V2 H2) ! i) ((make_tycontext_g V2 H) ! i))
+  (N2: forall i, subsumespec ((make_tycontext_s H2) ! i) ((make_tycontext_s H) ! i))
+  (N3: forall i, sub_option ((make_tycontext_g V2 H) ! i) ((make_tycontext_g V H) ! i)):
+@semax_func V H cs ge (funs1 ++ funs2) (G1++G2).
 Proof.
-  eapply semax_func_join; try eassumption.
-  intros. apply sub_option_refl.
-  intros. apply sub_option_refl.
+apply semax_func_app.
++ eapply semax_func_subsumption; [ | | apply SF1].
+- hnf; simpl. intuition.
+* rewrite PTree.gempty; trivial.
+* rewrite PTree.gempty. simpl; trivial.
+- intros. specialize (K1 id). eapply sub_option_trans. apply K1. trivial.
++ eapply semax_func_subsumption; [ | | apply SF2].
+- hnf; simpl. intuition.
+* rewrite PTree.gempty; trivial.
+* rewrite PTree.gempty. simpl; trivial.
+- intros. specialize (N1 id). eapply sub_option_trans. apply N1. trivial.
++ clear - SF1. eapply semax_func_length. apply SF1.
 Qed.
+
+Lemma semax_func_join_sameV {cs ge H1 H2 V funs1 funs2 G1 G2 H}
+  (SF1: @semax_func V H1 cs ge funs1 G1) (SF2: @semax_func V H2 cs ge funs2 G2)
+
+  (K1: forall i, sub_option ((make_tycontext_g V H1) ! i) ((make_tycontext_g V H) ! i))
+  (K2: forall i, subsumespec ((make_tycontext_s H1) ! i) ((make_tycontext_s H) ! i))
+
+  (N1: forall i, sub_option ((make_tycontext_g V H2) ! i) ((make_tycontext_g V H) ! i))
+  (N2: forall i, subsumespec ((make_tycontext_s H2) ! i) ((make_tycontext_s H) ! i)):
+@semax_func V H cs ge (funs1 ++ funs2) (G1++G2).
+Proof. apply (semax_func_join SF1 SF2); try eassumption; intros; apply sub_option_refl. Qed.
 
 Lemma sub_option_subsumespec x1 x2 (H:sub_option x1 x2): subsumespec x1 x2.
 Proof.
-  destruct x1 as [fs1 |]; destruct x2 as [fs2 |]; trivial; inv H.
-  apply subsumespec_refl.
+destruct x1 as [fs1 |]; destruct x2 as [fs2 |]; trivial; inv H.
+apply subsumespec_refl.
 Qed.
 
 Lemma make_tycontext_g_nilV_elim G i t: (make_tycontext_g nil G) ! i = Some t ->
-      exists fs, find (fun x => ident_eq i (fst x)) G = Some (i,fs) /\ t=type_of_funspec fs.
+  exists fs, find (fun x => ident_eq i (fst x)) G = Some (i,fs) /\ t=type_of_funspec fs.
 Proof.
-  induction G; simpl; intros. rewrite PTree.gempty in H. congruence.
-  destruct a as [j fs]; unfold ident_eq; simpl in *.
-  rewrite PTree.gsspec in H. destruct (peq i j); subst; simpl; eauto.
-  inv H. exists fs; split; trivial.
+induction G; simpl; intros. rewrite PTree.gempty in H. congruence.
+destruct a as [j fs]; unfold ident_eq; simpl in *.
+rewrite PTree.gsspec in H. destruct (peq i j); subst; simpl; eauto.
+inv H. exists fs; split; trivial.
 Qed.
 
 Fixpoint find_idV (id : ident) (G : varspecs) {struct G} : option type:=
-  match G with
-  | nil => None
-  | (id', f) :: G' => if peq id id' then Some f else find_idV id G'
-  end.
-(*
-Lemma find_id_maketycontext_g V G id : (make_tycontext_g V G) ! id =
-                                       match find_idV id V with
-                                         None => find_id id G | Some t => Some  t
-                                       end.
-Proof.
-  induction G as [|(i,t) G]; simpl.
-  - destruct id; reflexivity.
-  - rewrite PTree.gsspec.
-    do 2 if_tac; congruence.
-Qed.*)
+match G with
+| nil => None
+| (id', f) :: G' => if peq id id' then Some f else find_idV id G'
+end.
 
 Lemma make_tycontext_s_g V H i fs (HH: (make_tycontext_s H) ! i = Some fs):
-      (make_tycontext_g V H) ! i = Some (type_of_funspec fs).
+  (make_tycontext_g V H) ! i = Some (type_of_funspec fs).
 Proof.
-  induction H; simpl in *.  rewrite PTree.gempty in HH; congruence.
-  destruct a as [j gs]; simpl in *.  rewrite PTree.gsspec.
-  destruct (peq i j); subst.
-  + rewrite PTree.gss in HH; inv HH; trivial.
-  + rewrite PTree.gso in HH; auto.
+induction H; simpl in *.  rewrite PTree.gempty in HH; congruence.
+destruct a as [j gs]; simpl in *.  rewrite PTree.gsspec.
+destruct (peq i j); subst.
++ rewrite PTree.gss in HH; inv HH; trivial.
++ rewrite PTree.gso in HH; auto.
 Qed.
 
 Lemma make_tycontext_g_consV_elim:
-  forall i t v vs G (HV: list_norepet ((map fst (v::vs)) ++ (map fst G))),
-   (make_tycontext_g (v::vs) G) ! i = Some t ->
-   if peq i (fst v) then t=snd v else (make_tycontext_g vs G) ! i = Some t.
+forall i t v vs G (HV: list_norepet ((map fst (v::vs)) ++ (map fst G))),
+(make_tycontext_g (v::vs) G) ! i = Some t ->
+if peq i (fst v) then t=snd v else (make_tycontext_g vs G) ! i = Some t.
 Proof.
-  intros. destruct v as [j u]. induction G; simpl in *.
+intros. destruct v as [j u]. induction G; simpl in *.
 + rewrite PTree.gsspec in H. destruct (peq i j); subst; trivial. inv H; trivial.
 + destruct a as [k s]; simpl in *.  rewrite PTree.gsspec in *.
-  destruct (peq i k); subst.
-  - inv H. destruct (peq k j); trivial; subst. clear - HV. inv HV.
-    elim H1; clear. apply in_or_app.  right; left; trivial.
-  - apply IHG; trivial.  clear - HV. inv HV. apply list_norepet_append_inv in H2.
-    destruct H2 as [? [? ?]]. constructor.
-    * intros N. apply H1; clear - N.  apply in_app_or in N. apply in_or_app.
-      destruct N; [left; trivial | right; right; trivial].
-    * inv H0. apply list_norepet_append; trivial.
-      clear - H2. hnf; intros. apply H2; trivial.  right; trivial.
+destruct (peq i k); subst.
+- inv H. destruct (peq k j); trivial; subst. clear - HV. inv HV.
+elim H1; clear. apply in_or_app.  right; left; trivial.
+- apply IHG; trivial.  clear - HV. inv HV. apply list_norepet_append_inv in H2.
+destruct H2 as [? [? ?]]. constructor.
+* intros N. apply H1; clear - N.  apply in_app_or in N. apply in_or_app.
+  destruct N; [left; trivial | right; right; trivial].
+* inv H0. apply list_norepet_append; trivial.
+  clear - H2. hnf; intros. apply H2; trivial.  right; trivial.
 Qed.
 Lemma make_tycontext_g_consV_mk:
-  forall i t v vs G (HV: list_norepet ((map fst (v::vs)) ++ (map fst G))),
-   (if peq i (fst v) then t=snd v else (make_tycontext_g vs G) ! i = Some t) ->
-   (make_tycontext_g (v::vs) G) ! i = Some t.
+forall i t v vs G (HV: list_norepet ((map fst (v::vs)) ++ (map fst G))),
+(if peq i (fst v) then t=snd v else (make_tycontext_g vs G) ! i = Some t) ->
+(make_tycontext_g (v::vs) G) ! i = Some t.
 Proof.
-  intros. destruct v as [j u]. simpl in *. induction G; simpl in *. rewrite app_nil_r in HV.
+intros. destruct v as [j u]. simpl in *. induction G; simpl in *. rewrite app_nil_r in HV.
 + rewrite PTree.gsspec. destruct (peq i j); subst; trivial.
 + destruct a as [k s]; simpl in *. rewrite PTree.gsspec in *.
-  destruct (peq i k); subst.
-  - destruct (peq k j); trivial; subst. clear - HV. inv HV.
-    elim H1; clear. apply in_or_app.  right; left; trivial.
-  - apply IHG; trivial.  clear - HV. inv HV. apply list_norepet_append_inv in H2.
-    destruct H2 as [? [? ?]]. constructor.
-    * intros N. apply H1; clear - N.  apply in_app_or in N. apply in_or_app.
-      destruct N; [left; trivial | right; right; trivial].
-    * inv H0. apply list_norepet_append; trivial.
-      clear - H2. hnf; intros. apply H2; trivial.  right; trivial.
+destruct (peq i k); subst.
+- destruct (peq k j); trivial; subst. clear - HV. inv HV.
+elim H1; clear. apply in_or_app.  right; left; trivial.
+- apply IHG; trivial.  clear - HV. inv HV. apply list_norepet_append_inv in H2.
+destruct H2 as [? [? ?]]. constructor.
+* intros N. apply H1; clear - N.  apply in_app_or in N. apply in_or_app.
+  destruct N; [left; trivial | right; right; trivial].
+* inv H0. apply list_norepet_append; trivial.
+  clear - H2. hnf; intros. apply H2; trivial.  right; trivial.
 Qed.
 
 Lemma make_tycontext_g_nilG_findV V i: (make_tycontext_g V nil) ! i = find_idV i V.
 Proof.
-  induction V; simpl. apply PTree.gempty.
-  destruct a as [j t]; simpl.
-  rewrite PTree.gsspec. destruct (peq i j); subst; simpl; eauto.
+induction V; simpl. apply PTree.gempty.
+destruct a as [j t]; simpl.
+rewrite PTree.gsspec. destruct (peq i j); subst; simpl; eauto.
 Qed.
 
 Lemma make_tycontext_g_consG_elim i t V g G (HG: (make_tycontext_g V (g::G)) ! i = Some t):
-   if peq i (fst g) then t=type_of_funspec (snd g) else (make_tycontext_g V G) ! i = Some t.
+if peq i (fst g) then t=type_of_funspec (snd g) else (make_tycontext_g V G) ! i = Some t.
 Proof.
-  destruct g as [j fs]; simpl in *.
-  rewrite PTree.gsspec in HG. destruct (peq i j); subst; auto. inv HG; trivial.
+destruct g as [j fs]; simpl in *.
+rewrite PTree.gsspec in HG. destruct (peq i j); subst; auto. inv HG; trivial.
 Qed.
 Lemma make_tycontext_g_consG_mk i t V g G
-      (HG: if peq i (fst g) then t=type_of_funspec (snd g) else (make_tycontext_g V G) ! i = Some t):
-  (make_tycontext_g V (g::G)) ! i = Some t.
+  (HG: if peq i (fst g) then t=type_of_funspec (snd g) else (make_tycontext_g V G) ! i = Some t):
+(make_tycontext_g V (g::G)) ! i = Some t.
 Proof.
-  destruct g as [j fs]; simpl in *.
-  rewrite PTree.gsspec. destruct (peq i j); subst; auto.
+destruct g as [j fs]; simpl in *.
+rewrite PTree.gsspec. destruct (peq i j); subst; auto.
 Qed.
 
 Lemma find_idV_In_map_fst i t: forall V (Hi: find_idV i V = Some t), In i (map fst V).
 Proof.
-  induction V; simpl; intros. inv Hi.
-  destruct a as [j u]; simpl. destruct (peq i j); subst; [left | right]; auto.
+induction V; simpl; intros. inv Hi.
+destruct a as [j u]; simpl. destruct (peq i j); subst; [left | right]; auto.
 Qed.
 
-Lemma list_norepet_cit_middle {A:Set} l1 l2 (a:A) (Ha: list_norepet (l1 ++ (a :: l2))): list_norepet (l1 ++ l2).
+Lemma list_norepet_cut_middle {A:Set} l1 l2 (a:A) (Ha: list_norepet (l1 ++ (a :: l2))): list_norepet (l1 ++ l2).
 Proof.
-  apply list_norepet_append_inv in Ha. destruct Ha as [VH1 [VH2 D]]. inv VH2.
-  apply list_norepet_append; trivial.
-  intros x y X Y. apply D; [ trivial | right; trivial].
+apply list_norepet_append_inv in Ha. destruct Ha as [VH1 [VH2 D]]. inv VH2.
+apply list_norepet_append; trivial.
+intros x y X Y. apply D; [ trivial | right; trivial].
 Qed.
 
 Lemma make_context_g_mk_findV_mk: forall H V (VH:list_norepet (map fst V ++ map fst H)) i t
-  (Heqd : find_idV i V = Some t), (make_tycontext_g V H) ! i = Some t.
+(Heqd : find_idV i V = Some t), (make_tycontext_g V H) ! i = Some t.
 Proof.
-  induction H; intros.
-  + rewrite make_tycontext_g_nilG_findV; trivial.
-  + apply make_tycontext_g_consG_mk. destruct a as [j fs]; simpl in *.
-    destruct (peq i j); subst; simpl.
-  - apply list_norepet_append_inv in VH. destruct VH as [_ [_ VH]].
-    elim (VH j j); trivial.
-    apply (find_idV_In_map_fst _ _ _ Heqd). left; trivial.
-  - apply list_norepet_cit_middle in VH. apply IHlist; trivial.
+induction H; intros.
++ rewrite make_tycontext_g_nilG_findV; trivial.
++ apply make_tycontext_g_consG_mk. destruct a as [j fs]; simpl in *.
+destruct (peq i j); subst; simpl.
+- apply list_norepet_append_inv in VH. destruct VH as [_ [_ VH]].
+elim (VH j j); trivial.
+apply (find_idV_In_map_fst _ _ _ Heqd). left; trivial.
+- apply list_norepet_cut_middle in VH. apply IHlist; trivial.
 Qed.
 
 Lemma make_context_g_char:
-  forall H V (VH:list_norepet (map fst V ++ map fst H)) i,
-    (make_tycontext_g V H) ! i = match (make_tycontext_s H)!i with
-                                   None => find_idV i V
-                                 | Some fs => Some (type_of_funspec fs)
-                                 end.
+forall H V (VH:list_norepet (map fst V ++ map fst H)) i,
+(make_tycontext_g V H) ! i = match (make_tycontext_s H)!i with
+                               None => find_idV i V
+                             | Some fs => Some (type_of_funspec fs)
+                             end.
 Proof.
-  induction H; intros.
-  + rewrite make_tycontext_g_nilG_findV.
-    simpl; rewrite PTree.gleaf; trivial.
-  + apply list_norepet_cit_middle in VH.
-    remember ((make_tycontext_g V (a :: H)) ! i) as d; symmetry in Heqd; destruct d. 
-  - apply make_tycontext_g_consG_elim in Heqd. destruct a as [j fs]; simpl in *. rewrite PTree.gsspec.
-    destruct (peq i j); subst; simpl in *; trivial. rewrite <- IHlist, Heqd; trivial.
-  - destruct a as [j fs]; simpl in *; rewrite PTree.gsspec in *.
-    destruct (peq i j); subst; simpl in *. congruence.
-    rewrite <- IHlist, Heqd; trivial.
+induction H; intros.
++ rewrite make_tycontext_g_nilG_findV.
+simpl; rewrite PTree.gleaf; trivial.
++ apply list_norepet_cut_middle in VH.
+remember ((make_tycontext_g V (a :: H)) ! i) as d; symmetry in Heqd; destruct d. 
+- apply make_tycontext_g_consG_elim in Heqd. destruct a as [j fs]; simpl in *. rewrite PTree.gsspec.
+destruct (peq i j); subst; simpl in *; trivial. rewrite <- IHlist, Heqd; trivial.
+- destruct a as [j fs]; simpl in *; rewrite PTree.gsspec in *.
+destruct (peq i j); subst; simpl in *. congruence.
+rewrite <- IHlist, Heqd; trivial.
 Qed.
 
 Lemma suboption_make_tycontext_s_g V G H 
-      (GH: forall i : positive, sub_option (make_tycontext_s G) ! i (make_tycontext_s H) ! i)
-      (VH: list_norepet (map fst V ++ map fst H))
-      (LNR : list_norepet (map fst G)) i:
-  sub_option (make_tycontext_g V G) ! i (make_tycontext_g V H) ! i.
+  (GH: forall i : positive, sub_option (make_tycontext_s G) ! i (make_tycontext_s H) ! i)
+  (VH: list_norepet (map fst V ++ map fst H))
+  (LNR : list_norepet (map fst G)) i:
+sub_option (make_tycontext_g V G) ! i (make_tycontext_g V H) ! i.
 Proof.
-  remember ((make_tycontext_g V G) ! i) as d; destruct d; simpl; trivial; symmetry in Heqd.
-  rewrite make_context_g_char in *; trivial.
-  - remember ((make_tycontext_s G) ! i) as q; destruct q.
-    * specialize (GH i). rewrite <- Heqq in GH; simpl in GH. rewrite GH; trivial.
-    * rewrite Heqd, find_id_maketycontext_s. apply find_idV_In_map_fst in Heqd.
-      remember (find_id i H) as w; destruct w; trivial. symmetry in Heqw; apply find_id_e in Heqw.
-      apply list_norepet_append_inv in VH. destruct VH as [_ [_ D]].
-      elim (D i i); trivial. eapply in_map_fst in Heqw; apply Heqw.
-  - clear Heqd i t. apply list_norepet_append_inv in VH. destruct VH as [LNRV [LNRH D]].
-    apply list_norepet_append; trivial.
-    intros x y ? ?. apply D; trivial.  specialize (GH y). clear - GH H1 LNR.
-    hnf in GH. rewrite 2 find_id_maketycontext_s in GH. apply list_in_map_inv in H1.
-    destruct H1 as [[i fs] [? ?]]; subst.
-    erewrite find_id_i in GH; [| apply H1 | trivial]. apply find_id_e in GH. apply in_map_fst in GH. apply GH.
+remember ((make_tycontext_g V G) ! i) as d; destruct d; simpl; trivial; symmetry in Heqd.
+rewrite make_context_g_char in *; trivial.
+- remember ((make_tycontext_s G) ! i) as q; destruct q.
+* specialize (GH i). rewrite <- Heqq in GH; simpl in GH. rewrite GH; trivial.
+* rewrite Heqd, find_id_maketycontext_s. apply find_idV_In_map_fst in Heqd.
+  remember (find_id i H) as w; destruct w; trivial. symmetry in Heqw; apply find_id_e in Heqw.
+  apply list_norepet_append_inv in VH. destruct VH as [_ [_ D]].
+  elim (D i i); trivial. eapply in_map_fst in Heqw; apply Heqw.
+- clear Heqd i t. apply list_norepet_append_inv in VH. destruct VH as [LNRV [LNRH D]].
+apply list_norepet_append; trivial.
+intros x y ? ?. apply D; trivial.  specialize (GH y). clear - GH H1 LNR.
+hnf in GH. rewrite 2 find_id_maketycontext_s in GH. apply list_in_map_inv in H1.
+destruct H1 as [[i fs] [? ?]]; subst.
+erewrite find_id_i in GH; [| apply H1 | trivial]. apply find_id_e in GH. apply in_map_fst in GH. apply GH.
 Qed.
 
-Lemma semax_func_join_sameV' cs H1 H2 V funs1 funs2 G1 G2 H
-      (SF1: @semax_func V H1 cs funs1 G1) (SF2: @semax_func V H2 cs funs2 G2)
-      
-      (K1: forall i, sub_option ((make_tycontext_s H1) ! i) ((make_tycontext_s H) ! i))
-      (K2: forall i, sub_option ((make_tycontext_s H2) ! i) ((make_tycontext_s H) ! i))
-      
-      (LNR: list_norepet ((map fst V)++(map fst H)))
-      (LNR1: list_norepet (map fst H1)) (LNR2: list_norepet (map fst H2)):
-  @semax_func V H cs (funs1 ++ funs2) (G1++G2).
+Lemma semax_func_join_sameV' {cs ge H1 H2 V funs1 funs2 G1 G2 H}
+  (SF1: @semax_func V H1 cs ge funs1 G1) (SF2: @semax_func V H2 cs ge funs2 G2)
+
+  (K1: forall i, sub_option ((make_tycontext_s H1) ! i) ((make_tycontext_s H) ! i))
+  (K2: forall i, sub_option ((make_tycontext_s H2) ! i) ((make_tycontext_s H) ! i))
+
+  (LNR: list_norepet ((map fst V)++(map fst H)))
+  (LNR1: list_norepet (map fst H1)) (LNR2: list_norepet (map fst H2)):
+@semax_func V H cs ge (funs1 ++ funs2) (G1++G2).
 Proof.
-  eapply semax_func_join_sameV; try eassumption.
-  + apply suboption_make_tycontext_s_g; eauto.
-  + intros. apply sub_option_subsumespec; auto.
-  + apply suboption_make_tycontext_s_g; eauto.
-  + intros. apply sub_option_subsumespec; auto.
+apply (semax_func_join_sameV SF1 SF2); try eassumption.
++ apply suboption_make_tycontext_s_g; eauto.
++ intros; apply sub_option_subsumespec; auto.
++ apply suboption_make_tycontext_s_g; eauto.
++ intros; apply sub_option_subsumespec; auto.
 Qed.
 
 Lemma find_id_firstn i fs: forall n G (N: find_id i (firstn n G) = Some fs), find_id i G = Some fs.
 Proof.
-  induction n; simpl; intros. inv N.
-  destruct G; simpl in *. inv N.
-  destruct p as [j gs]; simpl in *.
-  destruct (eq_dec i j); subst; trivial. auto.
+induction n; simpl; intros. inv N.
+destruct G; simpl in *. inv N.
+destruct p as [j gs]; simpl in *.
+destruct (eq_dec i j); subst; trivial. auto.
 Qed.
 
 Lemma find_id_skipn i fs: forall n G (HG: list_norepet (map fst G))
-                                 (N: find_id i (skipn n G) = Some fs), find_id i G = Some fs.
+                             (N: find_id i (skipn n G) = Some fs), find_id i G = Some fs.
 Proof.
-  induction n; simpl; intros; trivial.
-  destruct G; simpl in *; trivial.
-  destruct p as [j gs]; simpl in *. inv HG.
-  destruct (eq_dec i j); [ subst | auto].
-  apply IHn in N; [clear IHn; exfalso| trivial].
-  apply find_id_e in N. apply in_map_fst in N; auto.
+induction n; simpl; intros; trivial.
+destruct G; simpl in *; trivial.
+destruct p as [j gs]; simpl in *. inv HG.
+destruct (eq_dec i j); [ subst | auto].
+apply IHn in N; [clear IHn; exfalso| trivial].
+apply find_id_e in N. apply in_map_fst in N; auto.
 Qed.
 
 Lemma In_firstn {A} (a:A): forall n l, In a (firstn n l) -> In a l.
 Proof.
-  induction n; simpl; intros. contradiction.
-  destruct l; inv H. left; trivial. right; auto.
+induction n; simpl; intros. contradiction.
+destruct l; inv H. left; trivial. right; auto.
 Qed.
 Lemma In_skipn {A} (a:A): forall n l, In a (skipn n l) -> In a l.
 Proof.
-  induction n; simpl; intros. trivial. 
-  destruct l. inv H. right; auto.
+induction n; simpl; intros. trivial. 
+destruct l. inv H. right; auto.
 Qed.
 
-Definition semax_prefunc ge V G (cs : compspecs) (fdecs : list (ident * fundef)) (G1 : funspecs) :=
-  match_fdecs fdecs G1 /\ prog_contains ge fdecs /\ (*cenv_sub cenv_cs (genv_cenv ge) /\*)
-  forall n : nat, (believe Espec (nofunc_tycontext V G) ge (nofunc_tycontext V G1)) n.
-
-Lemma semax_prefunc_cspecs_sub {CS CS'} (CSUB: cspecs_sub CS CS') ge V G fdecs G1:
-  semax_prefunc ge V G CS fdecs G1 -> semax_prefunc ge V G CS' fdecs G1 .
+Lemma semax_func_firstn {cs ge H V n funs G}:
+  forall (SF: @semax_func V H cs ge funs G),
+    @semax_func V H cs ge (firstn n funs) (firstn n G).
 Proof.
-  intros [MF [PC B]]. split3; [ trivial | trivial | intros ].
-  eapply (@believe_monoL CS Espec CS' ge); [ intros f; apply tycontext_sub_refl | assumption | apply (B n)].
-Qed. 
-
-Lemma semax_prefunc_firstn ge cs H V:
-  forall n funs G (SF: @semax_prefunc ge V H cs funs G),
-    @semax_prefunc ge V H cs (firstn n funs) (firstn n G).
-Proof.
-  intros. destruct SF as [SF1 [SF2 SF3]]; split; [|split].
-  + clear SF2 SF3. specialize (match_fdecs_length _ _ SF1); intros.
-    generalize dependent G. generalize dependent funs. induction n; simpl; intros. constructor.
-    destruct funs; simpl in *. destruct G; simpl in *. constructor. congruence.
-    destruct G; simpl in *. congruence. inv SF1. inv H0. constructor; auto.
-  + clear SF1 SF3. red; intros. apply SF2. eapply In_firstn; eauto. 
-  + clear SF1 SF2 funs; intros k v fsig cc A P Q p KP HP. apply (SF3 k v fsig cc A P Q p KP).
-    hnf; hnf in HP. destruct HP as [i [HP [HQ [GS B]]]].
-    exists i, HP, HQ; split; trivial.
-    clear B SF3. simpl in*. rewrite find_id_maketycontext_s.
-    rewrite find_id_maketycontext_s in GS. apply find_id_firstn in GS; trivial.
+intros. destruct SF as [SF1 [SF2 SF3]]; split; [|split].
++ clear SF2 SF3. specialize (match_fdecs_length _ _ SF1); intros. (*clear PC.*)
+generalize dependent G. generalize dependent funs. induction n; simpl; intros. constructor.
+destruct funs; simpl in *. destruct G; simpl in *. constructor. congruence.
+destruct G; simpl in *. congruence. inv SF1. inv H0. constructor; auto.
++ clear SF1 SF3. red; intros. apply SF2. eapply In_firstn; eauto.
++ clear SF2. intros ? ? ? k v fsig cc A P Q p KP HP.
+apply (SF3 ge' Gfs Gffp k v fsig cc A P Q p KP); clear SF3.
+hnf; hnf in HP. destruct HP as [i [HP [HQ [GS B]]]].
+exists i, HP, HQ; split; trivial.
+clear -GS. simpl in*. rewrite find_id_maketycontext_s.
+rewrite find_id_maketycontext_s in GS. apply find_id_firstn in GS; trivial.
 Qed.
 
-Lemma semax_prefunc_skipn ge cs H V funs (HV:list_norepet (map fst funs)) G (SF: @semax_prefunc ge V H cs funs G):
-  forall n ,
-    @semax_prefunc ge V H cs (skipn n funs) (skipn n G).
+Lemma semax_func_skipn {cs ge H V funs G} (HV:list_norepet (map fst funs)) (SF: @semax_func V H cs ge funs G):
+forall n ,
+@semax_func V H cs ge (skipn n funs) (skipn n G).
 Proof.
-  destruct SF as [SF1 [SF2 SF3]]; split; [|split].
-  + clear SF2 SF3. specialize (match_fdecs_length _ _ SF1); intros.
-    generalize dependent G. generalize dependent funs. induction n; simpl; intros; trivial.
-    destruct funs; simpl in *. inv SF1; constructor. destruct G; simpl in *; inv SF1. inv H0. inv HV. auto.
-  + clear SF1 SF3; red; intros. apply SF2. eapply In_skipn; eauto.
-  + clear SF2; intros k v fsig cc A P Q p KP HP. eapply match_fdecs_norepet in HV; [| eassumption ].
-    apply (SF3 k v fsig cc A P Q p KP).
-    hnf; hnf in HP. destruct HP as [i [HP [HQ [GS B]]]].
-    exists i, HP, HQ; split; trivial.
-    clear B SF1 SF3. simpl in *. rewrite find_id_maketycontext_s.
-    rewrite find_id_maketycontext_s in GS. apply find_id_skipn in GS; trivial.
+intros. destruct SF as [SF1 [SF2 SF3]]; split; [|split].
++ clear SF2 SF3. specialize (match_fdecs_length _ _ SF1); intros.
+generalize dependent G. generalize dependent funs. induction n; simpl; intros; trivial.
+destruct funs; simpl in *. inv SF1; constructor. destruct G; simpl in *; inv SF1. inv H0. inv HV. auto.
++ clear SF1 SF3. red; intros. apply SF2. eapply In_skipn; eauto.
++ clear SF2. intros ? ? ? k v fsig cc A P Q p KP HP.
+apply (SF3 ge' Gfs Gffp k v fsig cc A P Q p KP); clear SF3. 
+eapply match_fdecs_norepet in HV; [|eassumption ].
+hnf; hnf in HP. destruct HP as [i [HP [HQ [GS B]]]].
+exists i, HP, HQ; split; trivial.
+clear - GS HV. simpl in *. rewrite find_id_maketycontext_s.
+rewrite find_id_maketycontext_s in GS. apply find_id_skipn in GS; trivial.
 Qed.
-
-Lemma semax_func_firstn cs H V:
-  forall n funs G (SF: @semax_func V H cs funs G) (*(PC: prog_contains (expr_lemmas3.empty_genv cenv_cs) funs)*),
-    @semax_func V H cs (firstn n funs) (firstn n G).
+Lemma semax_func_cenv_sub {CS CS'} (CSUB: cenv_sub (@cenv_cs CS) (@cenv_cs CS')) V H ge funs G:
+@semax_func V H CS ge funs G -> @semax_func V H CS' ge funs G.
+Proof. apply semax_func_mono; [ apply CSUB | | ]; intros ?; apply sub_option_refl. Qed. 
+(*
+Lemma semax_func_loeb V G C (prog:program):
+@semax_func V G C (Genv.globalenv prog) (prog_funct prog) G ->
+@semax_func V nil C (Genv.globalenv prog) (prog_funct prog) G.
 Proof.
-  intros. destruct SF as [SF1 SF2]; split.
-  + clear SF2. specialize (match_fdecs_length _ _ SF1); intros. (*clear PC.*)
-    generalize dependent G. generalize dependent funs. induction n; simpl; intros. constructor.
-    destruct funs; simpl in *. destruct G; simpl in *. constructor. congruence.
-    destruct G; simpl in *. congruence. inv SF1. inv H0. constructor; auto.
-  + intros ? ? ? k. specialize (SF2 ge).
-    assert (PCC: prog_contains ge funs). admit. 
-    intros v fsig cc A P Q p KP HP. apply (SF2 PCC H1 k v fsig cc A P Q p KP); clear SF2.
-    hnf; hnf in HP. destruct HP as [i [HP [HQ [GS B]]]].
-    exists i, HP, HQ; split; trivial.
-    clear B. simpl in*. rewrite find_id_maketycontext_s.
-    rewrite find_id_maketycontext_s in GS. apply find_id_firstn in GS; trivial.
-Admitted.
-
-Lemma semax_func_skipn cs H V funs (HV:list_norepet (map fst funs)) G (SF: @semax_func V H cs funs G):
-  forall n ,
-    @semax_func V H cs (skipn n funs) (skipn n G).
-Proof.
-  destruct SF as [SF1 SF2]; split.
-  + clear SF2. specialize (match_fdecs_length _ _ SF1); intros.
-    generalize dependent G. generalize dependent funs. induction n; simpl; intros; trivial.
-    destruct funs; simpl in *. inv SF1; constructor. destruct G; simpl in *; inv SF1. inv H0. inv HV. auto.
-  + intros ? ? ? k. specialize (SF2 ge). eapply match_fdecs_norepet in HV; [| eassumption ].
-    assert (PCC: prog_contains ge funs). admit.
-    intros v fsig cc A P Q p KP HP. apply (SF2 PCC H1 k v fsig cc A P Q p KP).
-    hnf; hnf in HP. destruct HP as [i [HP [HQ [GS B]]]].
-    exists i, HP, HQ; split; trivial.
-    clear B SF2. simpl in *. rewrite find_id_maketycontext_s.
-    rewrite find_id_maketycontext_s in GS. apply find_id_skipn in GS; trivial.
-Admitted.
-
-Lemma semax_func_cenv_sub {CS CS'} (CSUB: cenv_sub (@cenv_cs CS) (@cenv_cs CS')) V H funs G:
-  @semax_func V H CS funs G -> @semax_func V H CS' funs G.
-Proof.
-  unfold semax_func; intros [? ?]. split; trivial. intros.
-  assert (X: cenv_sub (@cenv_cs CS) ge) by (eapply cenv_sub_trans; trivial). 
-  specialize (H1 _ H2 X n).
-  eapply (@believe_monoL CS Espec CS'); [ intros f; apply tycontext_sub_refl | apply CSUB | apply H1].
-Qed.
+intros [MFD [GC GE]].
+split. trivial. split. trivial. intros. specialize (GE _ Gfs Gffp n).
+eapply believe_monoL. 3: apply GE. 2: apply cspecs_sub_refl.
+intros. red; simpl. intuition; intros.
++ remember ((make_tycontext_t (fn_params f) (fn_temps f)) ! id) as x; destruct x; trivial.
++ red; intros. Search make_tycontext_g.
+    *)
 
 End semax_prog.
-(*
-Goal forall Espec ge V H cs fdecs G, @semax_prefunc Espec ge V H cs fdecs G -> prog_contains ge fdecs ->
-                               @semax_func Espec V H cs fdecs G.
-Proof.
-  intros. destruct H0. split; [ trivial | ].
-*)
- 
 
-
-      (*Fixpoint merge {A} (*(eqd: forall (a a':A), {a = a'} + {a <> a'})*)(eqd : A -> A -> bool) (l1 l2: list (ident * A)): option (list (ident * A)) :=
-  match l1 with
-    nil => Some l2
-  | (i,a)::t => match merge eqd t l2 with
-                  None => None
-                | Some m => match find (fun x=> eqb_ident i (fst x)) m with
-                              None => Some ((i,a)::m)
-                            | Some b => if eqd a (snd b) then Some m else None
-                            end
-                end
-  end.
-
-Definition VarSpec_merge (V1 V2:varspecs): option varspecs := merge eqb_type V1 V2.
-(*
-Definition identtype_eqdec: forall (x y : ident * type), {x = y}+{x <> y}.
-Proof.
-  destruct x as [i1 t1]. destruct y as [i2 t2].
-  destruct (ident_eq i1 i2); [ subst i2|].
-  + destruct (type_eq t1 t2); [ left; subst t2; reflexivity | right ].
-    intros N. inv N. apply n; reflexivity.
-  + right. intros N. inv N. apply n; reflexivity.
-Defined.
-
-Definition funsig_eqdec: forall (x y : funsig), {x = y}+{x <> y}.
-Proof.
-  destruct x as [args1 ret1]. destruct y as [args2 ret2].
-  destruct (type_eq ret1 ret2).
-+ subst. destruct (list_eq_dec identtype_eqdec args1 args2). left; subst; reflexivity.
-  right; intros N; inv N. apply n; reflexivity.
-+ right. intros N; inv N. apply n; reflexivity.
-Defined.
-(*
-Definition funspec_combine (fs1 fs2 fs:funspec):Prop.
-Proof.
-  destruct fs1 as [sig1 cc1 A1 P1 Q1 P_ne1 Q_ne1].
-  destruct fs2 as [sig2 cc2 A2 P2 Q2 P_ne2 Q_ne2].
-  destruct fs as [sig cc A P Q P_ne Q_ne].
-  Print TypeTree.
-  apply (sig1 = sig2 /\ sig1=sig /\ cc1=cc2 /\ cc1=cc /\ A = PiType bool (fun b => if b then A1 else A2)).
-         forall ts, P ts = *)
-Fixpoint Funspecs_insert fs (fspecs: funspecs) : funspecs:=
-  match funspecs with
-    nil => [fs]
-  | (i,s)::t => if ideqnt_eq i (fst fs) then (i, 
-*)
-                 
-
-Definition varspecs_sub (V1 V2:varspecs):=
-  forall i, sub_option (find_idV i V1) (find_idV i V2).
-
-Lemma X: forall H H', tycontext_sub (nofunc_tycontext nil H) (nofunc_tycontext nil H') -> 
-      forall V i, sub_option ((make_tycontext_g V H) ! i) ((make_tycontext_g V H') ! i).
-Proof.
-  intros H H' HH'. induction V; intros. apply HH'.
-  hnf. remember ((make_tycontext_g (a :: V) H) ! i). destruct o; trivial.
-  specialize (IHV i). destruct a as [j u]. unfold make_tycontext_g in *. simpl in *.
-  remember (fun v : ident * type => PTree.set (fst v) (snd v)) as f.
-  remember (fun var : ident * funspec => PTree.set (fst var) (type_of_funspec (snd var))) as g.
-  clear Heqf Heqg.
-  remember  (fold_right f (PTree.empty type) V) as GG. clear HeqGG.
-  Search PTree.fold. Search fold_left fold_right.
-  Check fold_symmetric.
-  remember ().
-  rewrite PTree.gsspec. ; simpl in *. apply H1.
-  Lemma make_tycontext_g_consD a V G i t: (make_tycontext_g (a :: V) G) ! i = Some t ->
-                                        (make_tycontext_g V G) ! i = Some t.
-Proof.
-  intros. hnf. hnf in H. unfold make_tycontext_g in H.
-  remember simpl in H.
-  erewrite <- fold_symmetric in H.
-  Search fold_right.
-Lemma make_tycontext_g_nil_up G i t: forall V U (HU: (make_tycontext_g U G) ! i = Some t),
-  (make_tycontext_g (V++U) G) ! i = Some t.
-Proof.
-  induction V; simpl. trivial.
-  intros.
-
-  Lemma make_tycontext_g_nil_up G i t U (HU: (make_tycontext_g U G) ! i = Some t):
-  forall V, (make_tycontext_g (V++U) G) ! i = Some t.
-Proof.
- induction V; simpl. trivial. 
- unfold make_tycontext_g. simpl. rewrite PTree.gsspec. Search fold_right cons.
- Lemma make_tycontext_mono1 V1 V2 G (V:  varspecs_sub V1 V2) i:
-  sub_option ((make_tycontext_g V1 G)!i) ((make_tycontext_g V2 G)!i).
-Proof.
-  hnf. hnf in V. remember ((make_tycontext_g V1 G) ! i) as d; destruct d; symmetry in Heqd; trivial.
-  induction V1; simpl in *. Search make_tycontext_g nil.
-  unfold make_tycontext_g in *. hnf.
-Definition specs_sub (V1 V2:varspecs):=
-  forall i, sub_option (find_idV i V1) (find_idV i V2).
-
-Lemma make_tycontext_mono2 V G1 G2 (G: tycontext_sub G1 G2) i:
-  sub_option ((make_tycontext_g V G1)!i) ((make_tycontext_g V G2)!i).
-                                              
-Lemma semax_func_join' cs V1 H1 V2 H2 V funs1 funs2 G1 G2 H
-      (SF1: @semax_func V1 H1 cs funs1 G1) (SF2: @semax_func V2 H2 cs funs2 G2)
-      (K1: tycontext_sub (nofunc_tycontext V1 H) (nofunc_tycontext V H)) 
-      (K2: tycontext_sub (nofunc_tycontext V2 H2) (nofunc_tycontext V H))
-      (HV1: varspecs_sub V1 V)  (HV2: varspecs_sub V2 V): 
-  @semax_func V H cs (funs1 ++ funs2) (G1++G2).
-Proof.
-  destruct K1 as [Q1 [Q2 [Q3 [Q4 [Q5 Q6]]]]]; simpl in *.
-  destruct K2 as [P1 [P2 [P3 [P4 [P5 P6]]]]]; simpl in *.
-  apply semax_func_app.
-  + eapply semax_func_subsumption; [ | | apply SF1].
-  - hnf; simpl. intuition.
-    intros. eapply sub_option_trans. apply Q4. Print find_id. hnf.
-    Print make_tycontext_g. trivial.
-  + eapply semax_func_subsumption; [ | | apply SF2].
-  - hnf; simpl. intuition.
-    * rewrite PTree.gempty; trivial.
-    * rewrite PTree.gempty. simpl; trivial.
-  - intros. specialize (N1 id). eapply sub_option_trans. apply N1. trivial.
-  + clear - SF1. eapply semax_func_length. apply SF1.
-Qed.
-Lemma semax_func_join cs V1 H1 V2 H2: forall funs1 funs2 G1 G2
-   (SF1: @semax_func V1 H1 cs funs1 G1) (SF2: @semax_func V2 H2 cs funs2 G2),
-   @semax_func (mergeV H cs (funs1 ++ funs2) (G1++G2).
-Proof.
-intros. destruct SF1 as [MF1 B1]. destruct SF2 as [MF2 B2]. 
-split; [ apply match_fdecs_app; trivial | intros; subst].
-apply prog_contains_app_inv in H0; destruct H0 as [PG1 PG2].
-specialize (B1 ge PG1 H1 n). specialize (B2 ge PG2 H1 n).
-clear -B1 B2.
-apply believe_app_inv; eauto.
-Qed.
-End semax_prog.
-(*
-Definition external_specification_sub {Z Z'}
-           (spec:  external_specification juicy_mem external_function Z)
-           (spec': external_specification juicy_mem external_function Z'):Prop :=
-  match spec, spec' with
-    Build_external_specification es_type es_pre es_post es_exit,
-    Build_external_specification es_type' es_pre' es_post' es_exit' =>
-    forall e t x typs args z m, es_pre e t x typs args z m ->
-              exists t' z', es_pre' e t' x typs args z' m /\
-                          ((forall ot ov mm, es_post' e t' x ot ov z' mm -> es_post e t x ot ov z mm)
-                           /\ (forall ov mm, es_exit' ov z' mm -> es_exit ov z mm))
-  end.
-           
-Definition  juicy_ext_spec_sub {Z Z'} (spec: juicy_ext_spec Z) (spec': juicy_ext_spec Z') :=
-  external_specification_sub (JE_spec _ spec) (JE_spec _ spec').
-
-Definition OracleKind_sub (Espec Espec': OracleKind): Prop :=
-        match Espec, Espec' with
-          Build_OracleKind ty spec, Build_OracleKind ty' spec' => juicy_ext_spec_sub spec spec'
-        end.
-
-Check Build_OracleKind. Print juicy_ext_spec. Print external_specification. add_funspecs_rec.
-Lemma believe_external_subsumption {Espec Espec'} (OSUB : OracleKind_sub Espec Espec')
-  (ge : genv) b sig cc A P Q m (B: (believe_external Espec ge b sig cc A P Q) m):
-  (believe_external Espec' ge b sig cc A P Q) m.
-Proof.
-  do 3 red in B. do 3 red.
-  destruct Espec as [OKty JExtSpec]. destruct Espec' as [OKty' JExtSpec']. simpl in *.
-  remember (Genv.find_funct ge b) as p; destruct p; [ | trivial].
-  destruct f; [ trivial | destruct B as [[B1 B2] B3]].
-  split; [ split; [ trivial | ] | trivial]. clear B1 B3. hnf in OSUB, B2. unfold  ext_spec_type in B2.
-Locate OK_ty. Print semax_external. Print semax_. Print _guard. Print believepred.
- Print believe_external. Locate semax_ext. pred.  remember (JE_spec OKty JExtSpec) as JES; destruct JES as [es_type es_pre es_post es_exit].
-  remember (JE_spec OKty' JExtSpec') as JES'; destruct JES' as [es_type' es_pre' es_post' es_exit']. simpl in *.
-  intros g ts x k MK F ts' args w KW a WA Ha.
-  specialize (B2 g ts x k MK F ts' args w KW a WA Ha).
-  destruct B2 as [u [U1 U2]]. subst. rewrite <- HeqJES in u. simpl in u, U1, U2; unfold ext_spec_type in u. (*exists u. type error in implicit arg*)
-  destruct Espec as [OKty JExtSpec]. destruct Espec' as [OKty' JExtSpec']. (* simpl in *.*)
-  hnf in OSUB.
-  remember (JE_spec OKty JExtSpec) as JES; destruct JES as [es_type es_pre es_post es_exit].
-  remember (JE_spec OKty' JExtSpec') as JES'; destruct JES' as [es_type' es_pre' es_post' es_exit'].
-  remember (JE_spec OK_ty OK_spec) as JESS; destruct JESS as [es_typeX es_preX es_postX es_exitX].
-  simpl in u. unfold ext_spec_type in u.
-  specialize (OSUB e). simpl in OSUB. destruct Ha as [Ha1 Ha2]. simpl in u. Print ext_compat. Set Printing All. None. as [es_type es_pre es_post es_exit]. destruct (JE_spec OK_ty0 OK_spec0).
-
-exists u. split. 2: apply B3. split; trivial. hnf in B. admit. in B. red in B. destruct B. hnf in B. remember (believe_external Espec ge b sig cc A P Q). destruct p.
-       simpl in *.
-       
-       destruct B. intros.
-
-  Qed.
-
-  Lemma semax_func_externalsubsumption {Espec Espec' cs V F}
-      (OSUB:  OracleKind_sub Espec Espec'):
-  forall funs G (SF: @semax_func Espec V F cs funs G),  @semax_func Espec' V F cs funs G.
-Proof. intros. destruct SF as [MF B].
-  split; [trivial | intros; specialize (B _ H H0 n); clear - OSUB B].
-  intros b sig cc A P Q m NEC Claim.
-  destruct (B b sig cc A P Q _ NEC Claim) as [HB | HB]; [ left | right]; clear Claim B.
-+ (*believe_externalEpsec_sub*)
-  hnf. Print believe_external. destruct B. hnf in B. eapply allp_derives.  simpl in B. specialize (B _ H H0 n b). hnf in B.
-  clear - OSUB B. hnf; intros. specialize apply B.
-  eapply believe_monoL; [| eassumption]; intros.
-  clear - SUB HV.
-  destruct SUB as [SUBa [SUBb [SUBc [SUBd [SUBe SUBf]]]]]; simpl in *.
-  unfold func_tycontext'; split; simpl; intuition.
-  destruct ((make_tycontext_t (fn_params f) (fn_temps f)) ! id); trivial.
-Qed.
-
-Definition funspecs_sub V (G1 G2:funspecs) :=
-(forall i s, (make_tycontext_s G1) ! i = Some s -> (make_tycontext_s G2) ! i = Some s) /\
-(forall i t, (make_tycontext_g V G1) ! i = Some t -> (make_tycontext_g V G2) ! i = Some t).
-
-Lemma funspecs_sub_sub_option_s V G1 G2 (F: funspecs_sub V G1 G2) id:
-  sub_option ((make_tycontext_s G1) ! id) ((make_tycontext_s G2) ! id).
-Proof.
-red. remember ((make_tycontext_s G1) ! id) as t; symmetry in Heqt.
-destruct t; trivial. apply F in Heqt; trivial. 
-Qed.
-
-Lemma funspecs_sub_sub_option_g V G1 G2 (F: funspecs_sub V G1 G2) id:
-  sub_option ((make_tycontext_g V G1) ! id) ((make_tycontext_g V G2) ! id).
-Proof.
-red. remember ((make_tycontext_g V G1) ! id) as t; symmetry in Heqt.
-destruct t; trivial. apply F in Heqt; trivial. 
-Qed.
-
-Lemma funspecs_sub_refl V G: funspecs_sub V G G.
-Proof. split; intros; trivial. Qed.
-
-Lemma funspecs_sub_trans V G1 G2 G3: funspecs_sub V G1 G2 ->
-  funspecs_sub V G2 G3 -> funspecs_sub V G1 G3.
-Proof. intros. destruct H as [A1 A2]. destruct H0 as [B1 B2]. 
-split; intros; eauto.
-Qed.
-
-Lemma funspecs_sub_nofunctycontext_sub {V} G1 G2 (HSUB: funspecs_sub V G1 G2) f:
-tycontext_sub (func_tycontext' f (nofunc_tycontext V G1))
-  (func_tycontext' f (nofunc_tycontext V G2)).
-Proof. red. unfold func_tycontext; simpl; intuition.
-+ destruct ((make_tycontext_t (fn_params f) (fn_temps f)) ! id); trivial.
-+ apply funspecs_sub_sub_option_g; trivial.
-+ eapply funspecs_sub_sub_option_s; eauto.
-+ apply Annotation_sub_refl.
-Qed.
-
-Lemma funspecs_sub_functycontext_sub {V} G1 G2 (HSUB: funspecs_sub V G1 G2) f K:
-tycontext_sub (func_tycontext f V G1 K) (func_tycontext f V G2 K).
-Proof. red. unfold func_tycontext; simpl; intuition.
-+ destruct ((make_tycontext_t (fn_params f) (fn_temps f)) ! id); trivial.
-+ apply funspecs_sub_sub_option_g; trivial.
-+ eapply funspecs_sub_sub_option_s; eauto.
-+ apply Annotation_sub_refl.
-Qed.
+      (*
 
 (*We may always add unused assumptions to G - intuitively, this context weakening rule 
   is sound since one could have done the proof of f wrt the larger gprog in the first place. *)
@@ -2571,5 +2306,4 @@ Definition match_fdecs_sub funs G funs' G' :=
 Definition hide_auxiliary_functions {cs} V K funs G := 
    exists funs' G', match_fdecs_sub funs G funs' G' /\
                     @semax_func V K cs funs' G'.
-*)
 *)
